@prefix          rdf: <http://www.w3.org/1999/02/22-rdf-syntax-ns#> .
@prefix         rdfs: <http://www.w3.org/2000/01/rdf-schema#> .
@prefix          xsd: <http://www.w3.org/2001/XMLSchema#> .
@prefix          owl: <http://www.w3.org/2002/07/owl#> .
@prefix             : <http://iec.ch/TC57/CIM-generic#> .
@prefix          cim: <https://cim.ucaiug.io/ns#> .
@prefix       entsoe: <http://entsoe.eu/CIM/SchemaExtension/3/1#> .
@prefix           md: <http://iec.ch/TC57/61970-552/ModelDescription/1#> .
@prefix        model: <http://iec.ch/TC57/61970-552/ModelDescription/1#> .
@prefix         next: <http://der.edf.fr/mire/MSite-v3.1.a#> .
@prefix        next2: <http://edf.fr/draft/cim17-ext#> .
@prefix        next3: <http://edf.fr/draft/cim17-info#> .
@prefix          uml: <http://iec.ch/TC57/NonStandard/UML#> .

<http://iec.ch/TC57/CIM-generic> a owl:Ontology .

:ModelingAuthority a owl:Class ;
  rdfs:label "ModelingAuthority" ;
  rdfs:comment "A Modeling Authority is an entity responsible for supplying and maintaining the data defining a specific set of objects in a network model."@en ;
  rdfs:isDefinedBy :Package_ModelAuthority ;
  uml:id "EAID_C2D644C3_20C1_408d_86F0_738AD512C121" .

:ModelingAuthoritySet a owl:Class ;
  rdfs:label "ModelingAuthoritySet" ;
  rdfs:comment """A Modeling Authority Set is a group of objects in a network model where the data is supplied and maintained by the same Modeling Authority.
This class is typically not included in instance data exchange as this information is tracked by other mechanisms in the exchange."""@en ;
  rdfs:isDefinedBy :Package_ModelAuthority ;
  uml:id "EAID_6D6E62ED_DCB6_4e54_9159_8469729C9828" .

:PowerSystemProjectSchedule a owl:Class ;
  rdfs:label "PowerSystemProjectSchedule" ;
  rdfs:isDefinedBy :Package_PowerSystemProject ;
  uml:id "EAID_7DC6B4C8_C974_401f_939A_39C1DD101122" .

:PowerSystemSubProject a owl:Class ;
  rdfs:label "PowerSystemSubProject" ;
  rdfs:comment "A collection of dependent projects."@en ;
  rdfs:isDefinedBy :Package_PowerSystemProject ;
  uml:id "EAID_42771878_2F05_4bc6_BC00_E9068AA3EDD3" .

:ProjectStep a owl:Class ;
  rdfs:label "ProjectStep" ;
  rdfs:comment "The ProjectSteps are ordered by the actualStart and actualEnds so that  a dependent ProjectStep will have a actualStart after an actualEnd."@en ;
  rdfs:isDefinedBy :Package_PowerSystemProject ;
  uml:id "EAID_7CD8163C_EE75_49cd_9305_8882E4110723" .

:ProjectStepStatusKind a owl:Class ;
  rdfs:label "ProjectStepStatusKind" ;
  rdfs:isDefinedBy :Package_PowerSystemProject ;
  uml:hasStereotype uml:enum, uml:enumeration ;
  uml:id "EAID_9A16A0EF_917D_4824_BA55_8833EB4D8E0E" .

:StepKind a owl:Class ;
  rdfs:label "StepKind" ;
  rdfs:comment "First phase investigation and planning."@en, "Project is approved for realisation and the construction is starting, under construction or in the state of being realist."@en, "State of the project"@en, "The project is commissioned and added to the network model."@en ;
  rdfs:isDefinedBy :Package_PowerSystemProject ;
  uml:hasStereotype uml:enum, uml:enumeration ;
  uml:id "EAID_E73576D6_ABD2_4dde_B7AB_71996C8B33A2" .

cim:ACDCConverter a owl:Class ;
  rdfs:label "ACDCConverter" ;
  rdfs:comment "A unit with valves for three phases, together with unit control equipment, essential protective and switching devices, DC storage capacitors, phase reactors and auxiliaries, if any, used for conversion."@en ;
  rdfs:isDefinedBy :Package_Standard ;
  rdfs:subClassOf cim:ConductingEquipment ;
  uml:id "EAID_E4B8FEDD_411B_4c05_87D7_966230B8DA6F" .

cim:ACDCTerminal a owl:Class ;
  rdfs:label "ACDCTerminal" ;
  rdfs:comment "An electrical connection point (AC or DC) to a piece of conducting equipment. Terminals are connected at physical connection points called connectivity nodes."@en ;
  rdfs:isDefinedBy :Package_Standard ;
  rdfs:subClassOf cim:IdentifiedObject ;
  uml:id "EAID_73962937_D47A_4edc_93AC_C1455DD3B3D1" .

cim:ACLineSegment a owl:Class ;
  rdfs:label "ACLineSegment" ;
  rdfs:comment """A wire or combination of wires, with consistent electrical characteristics, building a single electrical system, used to carry alternating current between points in the power system.
For symmetrical, transposed 3ph lines, it is sufficient to use ACLineSegment attributes, which describe sequence impedances and admittances for the entire length of the segment.
If per lenght impedance data is available from a library of standard types, impedances and admittances can be calculated in one of the following ways:
- calculate electrical parameters from asset data, using associated ConductorInfo, with values then multiplied by Conductor.length to produce a matrix model.
- calculate unbalanced electrical parameters from associated PerLengthPhaseImpedance, then multiplied by Conductor.length to produce a matrix model.
- calculate transposed electrical parameters from associated PerLengthSequenceImpedance, then multiplied by Conductor.length to produce a sequence model."""@en ;
  rdfs:isDefinedBy :Package_Standard ;
  rdfs:subClassOf cim:Conductor ;
  uml:id "EAID_1D2E31F3_43A4_4892_9784_A678056A767F" .

cim:Accumulator a owl:Class ;
  rdfs:label "Accumulator" ;
  rdfs:comment "Accumulator represents an accumulated (counted) Measurement, e.g. an energy value."@en ;
  rdfs:isDefinedBy :Package_Standard ;
  rdfs:subClassOf cim:Measurement ;
  uml:id "EAID_E1E8BA41_5B74_4377_B3F6_D703C2D2B551" .

cim:AccumulatorLimit a owl:Class ;
  rdfs:label "AccumulatorLimit" ;
  rdfs:comment "Limit values for Accumulator measurements."@en ;
  rdfs:isDefinedBy :Package_Standard ;
  rdfs:subClassOf cim:Limit ;
  uml:id "EAID_E4999D4A_210C_4447_841A_41D996D602E8" .

cim:AccumulatorLimitSet a owl:Class ;
  rdfs:label "AccumulatorLimitSet" ;
  rdfs:comment "An AccumulatorLimitSet specifies a set of Limits that are associated with an Accumulator measurement."@en ;
  rdfs:isDefinedBy :Package_Standard ;
  rdfs:subClassOf cim:LimitSet ;
  uml:id "EAID_1C8D58C4_FCF2_492c_89A4_83BAF41BAA18" .

cim:AccumulatorReset a owl:Class ;
  rdfs:label "AccumulatorReset" ;
  rdfs:comment "This command reset the counter value to zero."@en ;
  rdfs:isDefinedBy :Package_Standard ;
  rdfs:subClassOf cim:Control ;
  uml:id "EAID_1B2DD17A_F6BA_45e8_81F3_0DDDBF5D05EE" .

cim:AccumulatorValue a owl:Class ;
  rdfs:label "AccumulatorValue" ;
  rdfs:comment "AccumulatorValue represents an accumulated (counted) MeasurementValue."@en ;
  rdfs:isDefinedBy :Package_Standard ;
  rdfs:subClassOf cim:MeasurementValue ;
  uml:id "EAID_9409698A_0EC0_43bf_8FBF_4E4E58D1CE36" .

cim:ActivePowerLimit a owl:Class ;
  rdfs:label "ActivePowerLimit" ;
  rdfs:comment "Limit on active power flow."@en ;
  rdfs:isDefinedBy :Package_Standard ;
  rdfs:subClassOf cim:OperationalLimit ;
  uml:id "EAID_61B761A7_FE31_42cd_AFAA_0278276E2666" .

cim:ActivityRecord a owl:Class ;
  rdfs:label "ActivityRecord" ;
  rdfs:comment "Records activity for an entity at a point in time; activity may be for an event that has already occurred or for a planned activity."@en ;
  rdfs:isDefinedBy :Package_Standard ;
  rdfs:subClassOf cim:IdentifiedObject ;
  uml:id "EAID_EF61019D_23DF_4dff_A1FE_19EF35342293" .

cim:Analog a owl:Class ;
  rdfs:label "Analog" ;
  rdfs:comment "Analog represents an analog Measurement."@en ;
  rdfs:isDefinedBy :Package_Standard ;
  rdfs:subClassOf cim:Measurement ;
  uml:id "EAID_CB8B382D_E1E5_49b4_877C_02FC908506D1" .

cim:AnalogControl a owl:Class ;
  rdfs:label "AnalogControl" ;
  rdfs:comment "An analog control used for supervisory control."@en ;
  rdfs:isDefinedBy :Package_Standard ;
  rdfs:subClassOf cim:Control ;
  uml:id "EAID_E96CD0F4_2DB9_463c_BF30_CBF0A8702C8A" .

cim:AnalogLimit a owl:Class ;
  rdfs:label "AnalogLimit" ;
  rdfs:comment "Limit values for Analog measurements."@en ;
  rdfs:isDefinedBy :Package_Standard ;
  rdfs:subClassOf cim:Limit ;
  uml:id "EAID_67988799_9B9D_4878_A3A0_EAD65D9FFC20" .

cim:AnalogLimitSet a owl:Class ;
  rdfs:label "AnalogLimitSet" ;
  rdfs:comment "An AnalogLimitSet specifies a set of Limits that are associated with an Analog measurement."@en ;
  rdfs:isDefinedBy :Package_Standard ;
  rdfs:subClassOf cim:LimitSet ;
  uml:id "EAID_3C2B50FE_D897_412a_9E32_62E1BBB4261A" .

cim:AnalogValue a owl:Class ;
  rdfs:label "AnalogValue" ;
  rdfs:comment "AnalogValue represents an analog MeasurementValue."@en ;
  rdfs:isDefinedBy :Package_Standard ;
  rdfs:subClassOf cim:MeasurementValue ;
  uml:id "EAID_307246AC_652B_48db_818E_BC07E24B988A" .

cim:ApparentPowerLimit a owl:Class ;
  rdfs:label "ApparentPowerLimit" ;
  rdfs:comment "Apparent power limit."@en ;
  rdfs:isDefinedBy :Package_Standard ;
  rdfs:subClassOf cim:OperationalLimit ;
  uml:id "EAID_72C6D115_0441_410b_91AB_0256894957C5" .

cim:AssetInfo a owl:Class ;
  rdfs:label "AssetInfo" ;
  rdfs:comment """Set of attributes of an asset, representing typical data-sheet information of a physical device, that can be instantiated and shared in different data exchange contexts:
- as attributes of an asset instance (installed or in stock)
- as attributes of an asset model (product by a manufacturer)
- as attributes of a type asset (generic type of an asset as used in designs/extension planning)."""@en ;
  rdfs:isDefinedBy :Package_Standard ;
  uml:id "EAID_F828BFC4_FF3B_4f7b_9918_D2CFE7FFB08F" .

cim:AssetModelUsageKind a owl:Class ;
  rdfs:label "AssetModelUsageKind" ;
  rdfs:comment "Usage for an asset model."@en ;
  rdfs:isDefinedBy :Package_CIMEnumerations ;
  uml:hasStereotype uml:enumeration ;
  uml:id "EAID_95C22779_AD14_4e7b_875E_E85E8EACEC42" .

cim:AsynchronousMachineKind a owl:Class ;
  rdfs:label "AsynchronousMachineKind" ;
  rdfs:comment "Kind of Asynchronous Machine."@en ;
  rdfs:isDefinedBy :Package_CIMEnumerations ;
  uml:hasStereotype uml:enumeration ;
  uml:id "EAID_C2395579_2094_4bc6_B96D_56E185200EB1" .

cim:AuxiliaryEquipment a owl:Class ;
  rdfs:label "AuxiliaryEquipment" ;
  rdfs:comment """AuxiliaryEquipment describe equipment that is not performing any primary functions but support for the equipment performing the primary function.
AuxiliaryEquipment is attached to primary eqipment via an association with Terminal."""@en ;
  rdfs:isDefinedBy :Package_Standard ;
  rdfs:subClassOf cim:Equipment ;
  uml:id "EAID_E4350618_FA63_4233_A322_084A3D8D6344" .

cim:BaseVoltage a owl:Class ;
  rdfs:label "BaseVoltage" ;
  rdfs:comment "Defines a system base voltage which is referenced."@en ;
  rdfs:isDefinedBy :Package_Standard ;
  rdfs:subClassOf cim:IdentifiedObject ;
  uml:id "EAID_83005361_3004_42e7_9F4E_BDAFE90C3C8E" .

cim:BasicIntervalSchedule a owl:Class ;
  rdfs:label "BasicIntervalSchedule" ;
  rdfs:comment "Schedule of values at points in time."@en ;
  rdfs:isDefinedBy :Package_Standard ;
  rdfs:subClassOf cim:IdentifiedObject ;
  uml:id "EAID_11278F41_E0DD_41c3_872F_9E9A7D02578B" .

cim:Bay a owl:Class ;
  rdfs:label "Bay" ;
  rdfs:comment "A collection of power system resources (within a given substation) including conducting equipment, protection relays, measurements, and telemetry."@en ;
  rdfs:isDefinedBy :Package_Standard ;
  rdfs:subClassOf cim:EquipmentContainer ;
  uml:id "EAID_ECFC9FB4_3930_4ddc_A74E_02150A8D494A" .

cim:Breaker a owl:Class ;
  rdfs:label "Breaker" ;
  rdfs:comment "A mechanical switching device capable of making, carrying, and breaking currents under normal circuit conditions and also making, carrying for a specified time, and breaking currents under specified abnormal circuit conditions e.g.  those of short circuit."@en ;
  rdfs:isDefinedBy :Package_Standard ;
  rdfs:subClassOf cim:ProtectedSwitch ;
  uml:id "EAID_F7EBE6CC_37B5_441e_AA67_048F19B86397" .

cim:BusbarSection a owl:Class ;
  rdfs:label "BusbarSection" ;
  rdfs:comment """A conductor, or group of conductors, with negligible impedance, that serve to connect other conducting equipment within a single substation. 
Voltage measurements are typically obtained from VoltageTransformers that are connected to busbar sections. A bus bar section may have many physical terminals but for analysis is modelled with exactly one logical terminal."""@en ;
  rdfs:isDefinedBy :Package_Standard ;
  rdfs:subClassOf cim:Connector ;
  uml:id "EAID_B53489B9_9717_454d_B9B2_8F1EF76F8C7D" .

cim:CDPSMVersion a owl:Class ;
  rdfs:label "CDPSMVersion" ;
  rdfs:comment "CDPSM profiles set version details."@en ;
  rdfs:isDefinedBy :Package_Extensions ;
  uml:hasStereotype uml:cdpsm ;
  uml:id "EAID_0D2BEBD3_B3EF_46c6_B7C8_533F3340D673" .

cim:CableConstructionKind a owl:Class ;
  rdfs:label "CableConstructionKind" ;
  rdfs:comment "Kind of cable construction."@en ;
  rdfs:isDefinedBy :Package_CIMEnumerations ;
  uml:hasStereotype uml:enumeration ;
  uml:id "EAID_A57A40AC_EA8E_400f_BA03_164E85900253" .

cim:CableOuterJacketKind a owl:Class ;
  rdfs:label "CableOuterJacketKind" ;
  rdfs:comment "Kind of cable outer jacket."@en ;
  rdfs:isDefinedBy :Package_CIMEnumerations ;
  uml:hasStereotype uml:enumeration ;
  uml:id "EAID_A507A747_6AAE_4791_A8EB_C551C6F5C249" .

cim:CableShieldMaterialKind a owl:Class ;
  rdfs:label "CableShieldMaterialKind" ;
  rdfs:comment "Kind of cable shield material."@en ;
  rdfs:isDefinedBy :Package_CIMEnumerations ;
  uml:hasStereotype uml:enumeration ;
  uml:id "EAID_8D834724_2F83_44b1_9CF6_81476C3CC028" .

cim:Clamp a owl:Class ;
  rdfs:label "Clamp" ;
  rdfs:comment """A Clamp is a galvanic connection at a line segment where other equipment is connected. A Clamp does not cut the line segment. 
A Clamp is ConductingEquipment and has one Terminal with an associated ConnectivityNode. Any other ConductingEquipment can be connected to the Clamp ConnectivityNode."""@en ;
  rdfs:isDefinedBy :Package_Standard ;
  rdfs:subClassOf cim:ConductingEquipment ;
  uml:id "EAID_45A9BC0B_DD92_4ed3_843E_80FBA5BDEB3A" .

cim:Command a owl:Class ;
  rdfs:label "Command" ;
  rdfs:comment "A Command is a discrete control used for supervisory control."@en ;
  rdfs:isDefinedBy :Package_Standard ;
  rdfs:subClassOf cim:Control ;
  uml:id "EAID_E4BA396F_9A04_46c2_AFE1_F2A12F304392" .

cim:ConductingEquipment a owl:Class ;
  rdfs:label "ConductingEquipment" ;
  rdfs:comment "The parts of the power system that are designed to carry current or that are conductively connected therewith. ConductingEquipment is contained within an EquipmentContainer that may be a Substation, or a VoltageLevel or a Bay within a Substation."@en ;
  rdfs:isDefinedBy :Package_Standard ;
  rdfs:subClassOf cim:Equipment ;
  uml:id "EAID_17635E36_A64E_48ac_9943_92A821E031AE" .

cim:Conductor a owl:Class ;
  rdfs:label "Conductor" ;
  rdfs:comment "Combination of conducting material with consistent electrical characteristics, building a single electrical system, used to carry current between points in the power system."@en ;
  rdfs:isDefinedBy :Package_Standard ;
  rdfs:subClassOf cim:ConductingEquipment ;
  uml:id "EAID_5196CA3B_8174_4eae_B08B_8675B24597E9" .

cim:ConformLoad a owl:Class ;
  rdfs:label "ConformLoad" ;
  rdfs:comment "ConformLoad represent loads that follow a daily load change pattern where the pattern can be used to scale the load with a system load."@en ;
  rdfs:isDefinedBy :Package_Standard ;
  rdfs:subClassOf cim:EnergyConsumer ;
  uml:id "EAID_3454A81A_AC03_49af_9A16_F2391231D918" .

cim:ConformLoadGroup a owl:Class ;
  rdfs:label "ConformLoadGroup" ;
  rdfs:comment "A group of loads conforming to an allocation pattern."@en ;
  rdfs:isDefinedBy :Package_Standard ;
  rdfs:subClassOf cim:LoadGroup ;
  uml:id "EAID_1CFB0BAD_FB96_4d11_A51C_594839590CEA" .

cim:ConformLoadSchedule a owl:Class ;
  rdfs:label "ConformLoadSchedule" ;
  rdfs:comment "A curve of load  versus time (X-axis) showing the active power values (Y1-axis) and reactive power (Y2-axis) for each unit of the period covered. This curve represents a typical pattern of load over the time period for a given day type and season."@en ;
  rdfs:isDefinedBy :Package_Standard ;
  rdfs:subClassOf cim:SeasonDayTypeSchedule ;
  uml:id "EAID_4D31652D_9655_4119_954E_AA4A86BB4449" .

cim:ConnectivityNode a owl:Class ;
  rdfs:label "ConnectivityNode" ;
  rdfs:comment "Connectivity nodes are points where terminals of conducting equipment are connected together with zero impedance."@en ;
  rdfs:isDefinedBy :Package_Standard ;
  rdfs:subClassOf cim:IdentifiedObject ;
  uml:id "EAID_779BB38C_4159_4b3b_B514_96060E70D5B9" .

cim:ConnectivityNodeContainer a owl:Class ;
  rdfs:label "ConnectivityNodeContainer" ;
  rdfs:comment "A base class for all objects that may contain ConnectivityNodes or TopologicalNodes."@en ;
  rdfs:isDefinedBy :Package_Standard ;
  rdfs:subClassOf cim:PowerSystemResource ;
  uml:id "EAID_E20BF07C_ADD2_4cc4_AC3A_7539E1F57201" .

cim:Connector a owl:Class ;
  rdfs:label "Connector" ;
  rdfs:comment "A conductor, or group of conductors, with negligible impedance, that serve to connect other conducting equipment within a single substation and are modelled with a single logical terminal."@en ;
  rdfs:isDefinedBy :Package_Standard ;
  rdfs:subClassOf cim:ConductingEquipment ;
  uml:id "EAID_05B789ED_9A2E_4278_ADE6_19C4CC89AF2D" .

cim:Control a owl:Class ;
  rdfs:label "Control" ;
  rdfs:comment "Control is used for supervisory/device control. It represents control outputs that are used to change the state in a process, e.g. close or open breaker, a set point value or a raise lower command."@en ;
  rdfs:isDefinedBy :Package_Standard ;
  rdfs:subClassOf cim:IdentifiedObject ;
  uml:id "EAID_D139BAA9_F770_45e2_997B_7C00746F7F56" .

cim:CsConverter a owl:Class ;
  rdfs:label "CsConverter" ;
  rdfs:comment "DC side of the current source converter (CSC)."@en ;
  rdfs:isDefinedBy :Package_Standard ;
  rdfs:subClassOf cim:ACDCConverter ;
  uml:id "EAID_C162ACC1_92E5_4a7b_9A75_FD25CFCAF011" .

cim:CurrentLimit a owl:Class ;
  rdfs:label "CurrentLimit" ;
  rdfs:comment "Operational limit on current."@en ;
  rdfs:isDefinedBy :Package_Standard ;
  rdfs:subClassOf cim:OperationalLimit ;
  uml:id "EAID_D2501F2F_6430_4eef_8FB0_9D8856F2931D" .

cim:CurrentTransformer a owl:Class ;
  rdfs:label "CurrentTransformer" ;
  rdfs:comment "Instrument transformer used to measure electrical qualities of the circuit that is being protected and/or monitored. Typically used as current transducer for the purpose of metering or protection. A typical secondary current rating would be 5A."@en ;
  rdfs:isDefinedBy :Package_Standard ;
  rdfs:subClassOf cim:Sensor ;
  uml:id "EAID_BC70A1BA_9060_405f_91ED_97EC81A6D4FD" .

cim:CurveStyle a owl:Class ;
  rdfs:label "CurveStyle" ;
  rdfs:comment "Style or shape of curve."@en ;
  rdfs:isDefinedBy :Package_CIMEnumerations ;
  uml:hasStereotype uml:enumeration ;
  uml:id "EAID_581AD431_AA05_4773_9693_5BD5767AA1F2" .

cim:Cut a owl:Class ;
  rdfs:label "Cut" ;
  rdfs:comment """A cut separates a line segment into two parts. The cut appears as a switch inserted between these two parts and connects them together. As the cut is normally open there is no galvanic connection between the two line segment parts. But it is possible to close the cut to get galvanic connection.
The cut terminals are oriented towards the line segment terminals with the same sequence number. Hence the cut terminal with sequence number equal to 1 is oriented to the line segment's terminal with sequence number equal to 1.
The cut terminals also act as connection points for jumpers and other equipment, e.g. a mobile generator. To enable this, connectivity nodes are placed at the cut terminals. Once the connectivity nodes are in place any conducting equipment can be connected at them."""@en ;
  rdfs:isDefinedBy :Package_Standard ;
  rdfs:subClassOf cim:Switch ;
  uml:id "EAID_AAD572FD_83F1_4d96_B8D6_E9CDA8CA1C61" .

cim:DateTimeInterval a owl:Class ;
  rdfs:label "DateTimeInterval" ;
  rdfs:comment "Interval between two date and time points."@en ;
  rdfs:isDefinedBy :Package_CompoundTypes ;
  uml:hasStereotype uml:compound ;
  uml:id "EAID_6941208A_3F6F_434f_A7D1_DD3484409331" .

cim:DayType a owl:Class ;
  rdfs:label "DayType" ;
  rdfs:comment "Group of similar days.   For example it could be used to represent weekdays, weekend, or holidays."@en ;
  rdfs:isDefinedBy :Package_Standard ;
  rdfs:subClassOf cim:IdentifiedObject ;
  uml:id "EAID_4BC38E1C_44D4_4d7c_8BD6_751B004B61A1" .

cim:Disconnector a owl:Class ;
  rdfs:label "Disconnector" ;
  rdfs:comment "A manually operated or motor operated mechanical switching device used for changing the connections in a circuit, or for isolating a circuit or equipment from a source of power. It is required to open or close circuits when negligible current is broken or made."@en ;
  rdfs:isDefinedBy :Package_Standard ;
  rdfs:subClassOf cim:Switch ;
  uml:id "EAID_AFBE2CEA_014F_40d8_90DC_FBEF13875EAB" .

cim:Discrete a owl:Class ;
  rdfs:label "Discrete" ;
  rdfs:comment "Discrete represents a discrete Measurement, i.e. a Measurement reprsenting discrete values, e.g. a Breaker position."@en ;
  rdfs:isDefinedBy :Package_Standard ;
  rdfs:subClassOf cim:Measurement ;
  uml:id "EAID_634720E8_D60B_490f_ABCC_15A34A0ABA31" .

cim:DiscreteValue a owl:Class ;
  rdfs:label "DiscreteValue" ;
  rdfs:comment "DiscreteValue represents a discrete MeasurementValue."@en ;
  rdfs:isDefinedBy :Package_Standard ;
  rdfs:subClassOf cim:MeasurementValue ;
  uml:id "EAID_A8639848_D22F_4902_9B41_9380914C67DF" .

cim:EarthFaultCompensator a owl:Class ;
  rdfs:label "EarthFaultCompensator" ;
  rdfs:comment "A conducting equipment used to represent a connection to ground which is typically used to compensate earth faults..   An earth fault compensator device modeled with a single terminal implies a second terminal solidly connected to ground.  If two terminals are modeled, the ground is not assumed and normal connection rules apply."@en ;
  rdfs:isDefinedBy :Package_Standard ;
  rdfs:subClassOf cim:ConductingEquipment ;
  uml:id "EAID_EDE5DBAC_703C_4144_89A5_4FCE4FBD6189" .

cim:EnergyArea a owl:Class ;
  rdfs:label "EnergyArea" ;
  rdfs:comment "Describes an area having energy production or consumption.  Specializations are intended to support the load allocation function as typically required in energy management systems or planning studies to allocate hypothesized load levels to individual load points for power flow analysis.  Often the energy area can be linked to both measured and forecast load levels."@en ;
  rdfs:isDefinedBy :Package_Standard ;
  rdfs:subClassOf cim:IdentifiedObject ;
  uml:id "EAID_4F65CB0A_EC71_4e58_8DD0_6B95958BB790" .

cim:EnergyConsumer a owl:Class ;
  rdfs:label "EnergyConsumer" ;
  rdfs:comment "Generic user of energy - a  point of consumption on the power system model"@en ;
  rdfs:isDefinedBy :Package_Standard ;
  rdfs:subClassOf next:EnergyConsumerEx ;
  uml:id "EAID_03EACE94_623E_49a4_A7A6_C416B0275D7E" .

cim:EnergyConsumerPhase a owl:Class ;
  rdfs:label "EnergyConsumerPhase" ;
  rdfs:isDefinedBy :Package_Standard ;
  rdfs:subClassOf cim:PowerSystemResource ;
  uml:id "EAID_E4EFA093_ACD3_482c_A5BD_EA2A3174860B" .

cim:EnergySource a owl:Class ;
  rdfs:label "EnergySource" ;
  rdfs:comment "A generic equivalent for an energy supplier on a transmission or distribution voltage level."@en ;
  rdfs:isDefinedBy :Package_Standard ;
  rdfs:subClassOf cim:ConductingEquipment ;
  uml:id "EAID_77E024DD_0CBF_4cff_A433_03EE5320ECAD" .

cim:Equipment a owl:Class ;
  rdfs:label "Equipment" ;
  rdfs:comment "The parts of a power system that are physical devices, electronic or mechanical"@en ;
  rdfs:isDefinedBy :Package_Standard ;
  rdfs:subClassOf cim:PowerSystemResource ;
  uml:id "EAID_B82E95D3_273D_4b82_AAB5_0CD2BDA1856D" .

cim:EquipmentContainer a owl:Class ;
  rdfs:label "EquipmentContainer" ;
  rdfs:comment "A modeling construct to provide a root class for containing equipment."@en, "This EquipmentContainer class is handled separately from the standard EquipmentContainer  to associate AdditionalGroupedEquipments to the Feeder only, not to other EquipmentContainer subclasses."@en ;
  rdfs:isDefinedBy :Package_Feeder, :Package_Standard ;
  rdfs:subClassOf next2:EquipmentContainerEx ;
  uml:id "EAID_50484252_A196_4e6e_AA0B_9F4E89FD6A14", "EAID_91F29D27_FBC2_4ec4_8D12_4A8B6C62BC01" .

cim:EquivalentEquipment a owl:Class ;
  rdfs:label "EquivalentEquipment" ;
  rdfs:comment "The class represents equivalent objects that are the result of a network reduction. The class is the base for equivalent objects of different types."@en ;
  rdfs:isDefinedBy :Package_Standard ;
  rdfs:subClassOf cim:ConductingEquipment ;
  uml:id "EAID_8CE203CF_B84C_43d1_84DF_A0D96BD4DE2E" .

cim:EquivalentInjection a owl:Class ;
  rdfs:label "EquivalentInjection" ;
  rdfs:comment "This class represents equivalent injections (generation or load).  Voltage regulation is allowed only at the point of connection."@en ;
  rdfs:isDefinedBy :Package_Standard ;
  rdfs:subClassOf cim:EquivalentEquipment ;
  uml:id "EAID_69E8ABEA_827C_4b0d_9A11_84253A745C42" .

cim:ExternalNetworkInjection a owl:Class ;
  rdfs:label "ExternalNetworkInjection" ;
  rdfs:comment "This class represents external network and it is used for IEC 60909 calculations."@en ;
  rdfs:isDefinedBy :Package_Standard ;
  rdfs:subClassOf cim:RegulatingCondEq ;
  uml:id "EAID_26F88C3D_E6EF_44b0_91F6_C8FAEC7A6654" .

cim:FaultIndicator a owl:Class ;
  rdfs:label "FaultIndicator" ;
  rdfs:comment "A FaultIndicator is typically only an indicator (which may or may not be remotely monitored), and not a piece of equipment that actually initiates a protection event. It is used for FLISR (Fault Location, Isolation and Restoration) purposes, assisting with the dispatch of crews to \"most likely\" part of the network (i.e. assists with determining circuit section where the fault most likely happened)."@en ;
  rdfs:isDefinedBy :Package_Standard ;
  rdfs:subClassOf cim:AuxiliaryEquipment ;
  uml:id "EAID_9EFE337E_1809_4dca_B55B_8216CD12CA90" .

cim:Feeder a owl:Class ;
  rdfs:label "Feeder" ;
  rdfs:isDefinedBy :Package_Feeder ;
  rdfs:subClassOf cim:EquipmentContainer ;
  uml:id "EAID_43543219_A85A_4869_9F70_4EDD756317B8" .

cim:Fuse a owl:Class ;
  rdfs:label "Fuse" ;
  rdfs:comment "An overcurrent protective device with a circuit opening fusible part that is heated and severed by the passage of overcurrent through it. A fuse is considered a switching device because it breaks current."@en ;
  rdfs:isDefinedBy :Package_Standard ;
  rdfs:subClassOf cim:Switch ;
  uml:id "EAID_2DE3AEF7_A6A4_44f6_8D4D_51D0E9E13A1C" .

cim:GeneratingUnit a owl:Class ;
  rdfs:label "GeneratingUnit" ;
  rdfs:comment "A single or set of synchronous machines for converting mechanical power into alternating-current power. For example, individual machines within a set may be defined for scheduling purposes while a single control signal is derived for the set. In this case there would be a GeneratingUnit for each member of the set and an additional GeneratingUnit corresponding to the set."@en ;
  rdfs:isDefinedBy :Package_Standard ;
  rdfs:subClassOf cim:Equipment ;
  uml:id "EAID_58AE6C16_5245_4df4_B888_D9853ACE679E" .

cim:GeneratorControlSource a owl:Class ;
  rdfs:label "GeneratorControlSource" ;
  rdfs:comment "The source of controls for a generating unit."@en ;
  rdfs:isDefinedBy :Package_CIMEnumerations ;
  uml:hasStereotype uml:enumeration ;
  uml:id "EAID_30E66CA1_5BEA_4df6_B147_E3BA6C8CCAB7" .

cim:GeographicalRegion a owl:Class ;
  rdfs:label "GeographicalRegion" ;
  rdfs:comment "A geographical region of a power system network model."@en ;
  rdfs:isDefinedBy :Package_Standard ;
  rdfs:subClassOf cim:IdentifiedObject ;
  uml:id "EAID_AC570A17_C7AF_49f7_A3A4_768E628BBD2F" .

cim:Ground a owl:Class ;
  rdfs:label "Ground" ;
  rdfs:comment "A common point for connecting grounded conducting equipment such as shunt capacitors. The power system model can have more than one ground."@en ;
  rdfs:isDefinedBy :Package_Standard ;
  rdfs:subClassOf cim:ConductingEquipment ;
  uml:id "EAID_4E453EB6_D458_4dfa_8B03_FDE54F380DCE" .

cim:GroundDisconnector a owl:Class ;
  rdfs:label "GroundDisconnector" ;
  rdfs:comment "A manually operated or motor operated mechanical switching device used for isolating a circuit or equipment from Ground."@en ;
  rdfs:isDefinedBy :Package_Standard ;
  rdfs:subClassOf cim:Switch ;
  uml:id "EAID_D118C89C_D326_4c7e_897B_DB43FA72FB0A" .

cim:GroundingImpedance a owl:Class ;
  rdfs:label "GroundingImpedance" ;
  rdfs:comment "A fixed impedance device used for grounding."@en ;
  rdfs:isDefinedBy :Package_Standard ;
  rdfs:subClassOf cim:EarthFaultCompensator ;
  uml:id "EAID_F9B17A56_469B_4bcb_B3CC_BD8FAAEDA430" .

cim:HydroGeneratingUnit a owl:Class ;
  rdfs:label "HydroGeneratingUnit" ;
  rdfs:comment "A generating unit whose prime mover is a hydraulic turbine (e.g., Francis, Pelton, Kaplan)."@en ;
  rdfs:isDefinedBy :Package_Standard ;
  rdfs:subClassOf cim:GeneratingUnit ;
  uml:id "EAID_F1B7D2AB_25F1_4b8d_8815_386EB4DF5D80" .

cim:HydroPlantStorageKind a owl:Class ;
  rdfs:label "HydroPlantStorageKind" ;
  rdfs:comment "The type of hydro power plant."@en ;
  rdfs:isDefinedBy :Package_CIMEnumerations ;
  uml:hasStereotype uml:enumeration ;
  uml:id "EAID_A93B398E_56F0_466c_B0DE_0F907EBB3614" .

cim:HydroPowerPlant a owl:Class ;
  rdfs:label "HydroPowerPlant" ;
  rdfs:comment "A hydro power station which can generate or pump. When generating, the generator turbines receive water from an upper reservoir. When pumping, the pumps receive their water from a lower reservoir."@en ;
  rdfs:isDefinedBy :Package_Standard ;
  rdfs:subClassOf cim:PowerSystemResource ;
  uml:id "EAID_89E7D54D_EBCE_4c63_8E0E_BD2203F207C0" .

cim:IEC61968CIMVersion a owl:Class ;
  rdfs:label "IEC61968CIMVersion" ;
  rdfs:comment "IEC 61968 version number assigned to this UML model."@en ;
  rdfs:isDefinedBy :Package_CDPSM2015_Versions ;
  uml:id "EAID_E46C312C_2296_448b_BD8F_889A26BE4A04" .

cim:IEC61970CIMVersion a owl:Class ;
  rdfs:label "IEC61970CIMVersion" ;
  rdfs:comment "This is the IEC 61970 CIM version number assigned to this UML model."@en ;
  rdfs:isDefinedBy :Package_CDPSM2015_Versions ;
  uml:id "EAID_D7DB6F76_F0D2_4df0_ADBA_8450E821106F" .

cim:IdentifiedObject a owl:Class ;
  rdfs:label "IdentifiedObject" ;
  rdfs:comment "This is a root class to provide common identification for all classes needing identification and naming attributes"@en ;
  rdfs:isDefinedBy :Package_Standard ;
  uml:id "EAID_9F5D5B14_A608_45f0_80E9_31C0DB022BF0" .

cim:Jumper a owl:Class ;
  rdfs:label "Jumper" ;
  rdfs:comment "A short section of conductor with negligible impedance which can be manually removed and replaced if the circuit is de-energized. Note that zero-impedance branches can be modelled by an ACLineSegment with a zero impedance ConductorType"@en ;
  rdfs:isDefinedBy :Package_Standard ;
  rdfs:subClassOf cim:Switch ;
  uml:id "EAID_F2C40DC7_5B2B_4fa6_8D43_14C089C90F5E" .

cim:Junction a owl:Class ;
  rdfs:label "Junction" ;
  rdfs:comment "A point where one or more conducting equipments are connected with zero resistance."@en ;
  rdfs:isDefinedBy :Package_Standard ;
  rdfs:subClassOf cim:Connector ;
  uml:id "EAID_2A9212D7_FF17_4876_BC94_6FF580E7FB73" .

cim:LifecycleDate a owl:Class ;
  rdfs:label "LifecycleDate" ;
  rdfs:comment "Dates for lifecycle events of an asset."@en ;
  rdfs:isDefinedBy :Package_CompoundTypes ;
  uml:hasStereotype uml:compound ;
  uml:id "EAID_071DD356_C080_45a8_8665_642A87AE1C75" .

cim:Limit a owl:Class ;
  rdfs:label "Limit" ;
  rdfs:comment "Specifies one limit value for a Measurement. A Measurement typically has several limits that are kept together by the LimitSet class. The actual meaning and use of a Limit instance (i.e., if it is an alarm or warning limit or if it is a high or low limit) is not captured in the Limit class. However the name of a Limit instance may indicate both meaning and use."@en ;
  rdfs:isDefinedBy :Package_Standard ;
  rdfs:subClassOf cim:IdentifiedObject ;
  uml:id "EAID_DD280888_6F8C_4231_8062_AF4B24A22E44" .

cim:LimitSet a owl:Class ;
  rdfs:label "LimitSet" ;
  rdfs:comment "Specifies a set of Limits that are associated with a Measurement. A Measurement may have several LimitSets corresponding to seasonal or other changing conditions. The condition is captured in the name and description attributes. The same LimitSet may be used for several Measurements. In particular percentage limits are used this way."@en ;
  rdfs:isDefinedBy :Package_Standard ;
  rdfs:subClassOf cim:IdentifiedObject ;
  uml:id "EAID_7774730A_6102_4735_86EC_10BDC5A690ED" .

cim:Line a owl:Class ;
  rdfs:label "Line" ;
  rdfs:comment "Contains equipment beyond a substation belonging to a power transmission line."@en ;
  rdfs:isDefinedBy :Package_Standard ;
  rdfs:subClassOf cim:EquipmentContainer ;
  uml:id "EAID_B31BA760_8A4F_4b75_AAC5_C5645ABE861D" .

cim:LinearShuntCompensator a owl:Class ;
  rdfs:label "LinearShuntCompensator" ;
  rdfs:comment "A linear shunt compensator has banks or sections with equal admittance values."@en ;
  rdfs:isDefinedBy :Package_Standard ;
  rdfs:subClassOf cim:ShuntCompensator ;
  uml:id "EAID_6155D99D_4F41_43b6_B335_8BCAF9095DA3" .

cim:LoadArea a owl:Class ;
  rdfs:label "LoadArea" ;
  rdfs:comment "The class is the root or first level in a hierarchical structure for grouping of loads for the purpose of load flow load scaling."@en ;
  rdfs:isDefinedBy :Package_Standard ;
  rdfs:subClassOf cim:EnergyArea ;
  uml:id "EAID_EEFB5A08_CD8A_4c1e_A022_76E18D575DE8" .

cim:LoadBreakSwitch a owl:Class ;
  rdfs:label "LoadBreakSwitch" ;
  rdfs:comment "A mechanical switching device capable of making, carrying, and breaking currents under normal operating conditions."@en ;
  rdfs:isDefinedBy :Package_Standard ;
  rdfs:subClassOf cim:ProtectedSwitch ;
  uml:id "EAID_D5271022_A512_4184_8EFF_6A8A15803A14" .

cim:LoadGroup a owl:Class ;
  rdfs:label "LoadGroup" ;
  rdfs:comment "The class is the third level in a hierarchical structure for grouping of loads for the purpose of load flow load scaling."@en ;
  rdfs:isDefinedBy :Package_Standard ;
  rdfs:subClassOf cim:IdentifiedObject ;
  uml:id "EAID_C3E8B27D_216F_4f00_A2AB_CCADD9E6E6BB" .

cim:Measurement a owl:Class ;
  rdfs:label "Measurement" ;
  rdfs:comment """A Measurement represents any measured, calculated or non-measured non-calculated quantity. Any piece of equipment may contain Measurements, e.g. a substation may have temperature measurements and door open indications, a transformer may have oil temperature and tank pressure measurements, a bay may contain a number of power flow measurements and a Breaker may contain a switch status measurement. 
The PSR - Measurement association is intended to capture this use of Measurement and is included in the naming hierarchy based on EquipmentContainer. The naming hierarchy typically has Measurements as leafs, e.g. Substation-VoltageLevel-Bay-Switch-Measurement.
Some Measurements represent quantities related to a particular sensor location in the network, e.g. a voltage transformer (PT) at a busbar or a current transformer (CT) at the bar between a breaker and an isolator. The sensing position is not captured in the PSR - Measurement association. Instead it is captured by the Measurement - Terminal association that is used to define the sensing location in the network topology. The location is defined by the connection of the Terminal to ConductingEquipment. 
Two possible paths exist:
1) Measurement-Terminal- ConnectivityNode-Terminal-ConductingEquipment
2) Measurement-Terminal-ConductingEquipment
Alternative 2 is the only allowed use. 
When the sensor location is needed both Measurement-PSR and Measurement-Terminal are used. The Measurement-Terminal association is never used alone."""@en ;
  rdfs:isDefinedBy :Package_Standard ;
  rdfs:subClassOf cim:IdentifiedObject ;
  uml:id "EAID_54CD7809_1D03_4b67_B876_4737EDD7B1D3" .

cim:MeasurementValue a owl:Class ;
  rdfs:label "MeasurementValue" ;
  rdfs:comment "The current state for a measurement. A state value is an instance of a measurement from a specific source. Measurements can be associated with many state values, each representing a different source for the measurement."@en ;
  rdfs:isDefinedBy :Package_Standard ;
  rdfs:subClassOf cim:IdentifiedObject ;
  uml:id "EAID_B4B1ED05_E775_4b9a_908F_987AE9E42EB5" .

cim:MeasurementValueSource a owl:Class ;
  rdfs:label "MeasurementValueSource" ;
  rdfs:comment "MeasurementValueSource describes the alternative sources updating a MeasurementValue. User conventions for how to use the MeasurementValueSource attributes are described in the introduction to IEC 61970-301."@en ;
  rdfs:isDefinedBy :Package_Standard ;
  rdfs:subClassOf cim:IdentifiedObject ;
  uml:id "EAID_47FDB193_9E66_4c3c_9278_415AC503D4B6" .

cim:Name a owl:Class ;
  rdfs:label "Name" ;
  rdfs:comment "The Name class provides the means to define any number of human readable  names for an object. A name is <b>not</b> to be used for defining inter-object relationships. For inter-object relationships instead use the object identification 'mRID'."@en ;
  rdfs:isDefinedBy :Package_Standard ;
  uml:id "EAID_66D2D8BC_7196_4732_AA18_4C1E27C0C93E" .

cim:NameType a owl:Class ;
  rdfs:label "NameType" ;
  rdfs:comment """Type of name. Possible values for attribute 'name' are implementation dependent but standard profiles may specify types. An enterprise may have multiple IT systems each having its own local name for the same object, e.g. a planning system may have different names from an EMS. An object may also have different names within the same IT system, e.g. localName and aliasName as defined in CIM version 14. Their definitions from CIM14 are
The localName is a human readable name of the object. It is only used with objects organized in a naming hierarchy. localName: A free text name local to a node in a naming hierarchy similar to a file directory structure. A power system related naming hierarchy may be: Substation, VoltageLevel, Equipment etc. Children of the same parent in such a hierarchy have names that typically are unique among them.
aliasName: A free text alternate name typically used in tabular reports where the column width is limited."""@en ;
  rdfs:isDefinedBy :Package_Standard ;
  uml:id "EAID_4888BA18_B172_45d6_9F1C_6AD840AA2FDD" .

cim:NameTypeAuthority a owl:Class ;
  rdfs:label "NameTypeAuthority" ;
  rdfs:comment "Authority responsible for creation and management of names of a given type; typically an organization or an enterprise system."@en ;
  rdfs:isDefinedBy :Package_Standard ;
  uml:id "EAID_BEC1D381_B55D_4010_AA14_DAAD9C04C6C5" .

cim:NonConformLoad a owl:Class ;
  rdfs:label "NonConformLoad" ;
  rdfs:comment "NonConformLoad represent loads that do not follow a daily load change pattern and changes are not correlated with the daily load change pattern."@en ;
  rdfs:isDefinedBy :Package_Standard ;
  rdfs:subClassOf cim:EnergyConsumer ;
  uml:id "EAID_FACE7379_0C5C_47dd_82C4_8C2E5D781017" .

cim:NonConformLoadGroup a owl:Class ;
  rdfs:label "NonConformLoadGroup" ;
  rdfs:comment "Loads that do not follow a daily and seasonal load variation pattern."@en ;
  rdfs:isDefinedBy :Package_Standard ;
  rdfs:subClassOf cim:LoadGroup ;
  uml:id "EAID_4A3E3B47_D3B9_49a8_8FD7_A72ADA6A1334" .

cim:NonConformLoadSchedule a owl:Class ;
  rdfs:label "NonConformLoadSchedule" ;
  rdfs:comment "An active power (Y1-axis) and reactive power (Y2-axis) schedule (curves) versus time (X-axis) for non-conforming loads, e.g., large industrial load or power station service (where modeled)."@en ;
  rdfs:isDefinedBy :Package_Standard ;
  rdfs:subClassOf cim:SeasonDayTypeSchedule ;
  uml:id "EAID_0CC3B168_B298_4d82_BB20_BA99C0AC1F3E" .

cim:OperatingParticipant a owl:Class ;
  rdfs:label "OperatingParticipant" ;
  rdfs:comment "An operator of multiple power system resource objects. Note multple operating participants may operate the same power system resource object.   This can be used for modeling jointly owned units where each owner operates as a contractual share."@en ;
  rdfs:isDefinedBy :Package_Standard ;
  uml:hasStereotype uml:description ;
  uml:id "EAID_2411DB1C_9F6C_4af9_97DF_8210C4EF77A1" .

cim:OperatingShare a owl:Class ;
  rdfs:label "OperatingShare" ;
  rdfs:comment "Specifies the operations contract relationship between a power system resource and a contract participant."@en ;
  rdfs:isDefinedBy :Package_Standard ;
  rdfs:subClassOf cim:IdentifiedObject ;
  uml:id "EAID_7BD7B8D4_A938_417c_AEE6_90DC94ACD876" .

cim:OperationalLimit a owl:Class ;
  rdfs:label "OperationalLimit" ;
  rdfs:comment """A value associated with a specific kind of limit. 
The sub class value attribute shall be positive. 
The sub class value attribute is inversely proportional to OperationalLimitType.acceptableDuration (acceptableDuration for short). A pair of value_x and acceptableDuration_x are related to each other as follows:
if value_1 &gt; value_2 &gt; value_3 &gt;... then
acceptableDuration_1 &lt; acceptableDuration_2 &lt; acceptableDuration_3 &lt; ...
A value_x with direction="high" shall be greater than a value_y with direction="low"."""@en ;
  rdfs:isDefinedBy :Package_Standard ;
  rdfs:subClassOf cim:IdentifiedObject ;
  uml:id "EAID_2E66B8DA_0272_4870_8A4C_C810D272B614" .

cim:OperationalLimitDirectionKind a owl:Class ;
  rdfs:label "OperationalLimitDirectionKind" ;
  rdfs:comment "The direction attribute describes the side of  a limit that is a violation."@en ;
  rdfs:isDefinedBy :Package_CIMEnumerations ;
  uml:hasStereotype uml:enumeration ;
  uml:id "EAID_851C85E6_4C7C_4fa1_ADC6_85BD43EBEE2D" .

cim:OperationalLimitSet a owl:Class ;
  rdfs:label "OperationalLimitSet" ;
  rdfs:comment "A set of limits associated with equipment.  Sets of limits might apply to a specific temperature, or season for example. A set of limits may contain different severities of limit levels that would apply to the same equipment. The set may contain limits of different types such as apparent power and current limits or high and low voltage limits  that are logically applied together as a set."@en ;
  rdfs:isDefinedBy :Package_Standard ;
  rdfs:subClassOf cim:IdentifiedObject ;
  uml:id "EAID_9E591814_DCCC_48a6_8B83_1EC02EC97C26" .

cim:OperationalLimitType a owl:Class ;
  rdfs:label "OperationalLimitType" ;
  rdfs:comment "The operational meaning of a category of limits."@en ;
  rdfs:isDefinedBy :Package_Standard ;
  rdfs:subClassOf entsoe:ENTSOEOperationalLimitType ;
  uml:id "EAID_3080CC4A_8033_462d_896E_0665CA2585ED" .

cim:OrientationKind a owl:Class ;
  rdfs:label "OrientationKind" ;
  rdfs:comment "The orientation of the coordinate system with respect to top, left, and the coordinate number system."@en ;
  rdfs:isDefinedBy :Package_CIMEnumerations ;
  uml:hasStereotype uml:enumeration ;
  uml:id "EAID_D1EF0087_BDE5_4b00_8462_DF7B5DD2CA29" .

cim:PSREvent a owl:Class ;
  rdfs:label "PSREvent" ;
  rdfs:comment "Event recording the change in operational status of a power system resource; may be for an event that has already occurred or for a planned activity."@en ;
  rdfs:isDefinedBy :Package_Standard ;
  rdfs:subClassOf cim:ActivityRecord ;
  uml:id "EAID_AB946712_EC97_4c2f_B8A8_55906B4852B0" .

cim:PSREventKind a owl:Class ;
  rdfs:label "PSREventKind" ;
  rdfs:comment "Kind of power system resource event."@en ;
  rdfs:isDefinedBy :Package_CIMEnumerations ;
  uml:hasStereotype uml:enumeration ;
  uml:id "EAID_72380D15_60A8_4a30_8311_256442CAA6EA" .

cim:PSRType a owl:Class ;
  rdfs:label "PSRType" ;
  rdfs:comment "Classifying instances of the same class, e.g. overhead and underground ACLineSegments. This classification mechanism is intended to provide flexibility outside the scope of this standard, i.e. provide customisation that is non standard."@en ;
  rdfs:isDefinedBy :Package_Standard ;
  rdfs:subClassOf cim:IdentifiedObject ;
  uml:id "EAID_814AE236_DBA7_464e_B81B_F83BD11AAE38" .

cim:PerLengthImpedance a owl:Class ;
  rdfs:label "PerLengthImpedance" ;
  rdfs:comment "Common type for per-length impedance electrical catalogues."@en ;
  rdfs:isDefinedBy :Package_Standard ;
  rdfs:subClassOf cim:PerLengthLineParameter ;
  uml:id "EAID_C0FD068F_D820_4d6d_979B_6D248F7147E9" .

cim:PerLengthLineParameter a owl:Class ;
  rdfs:label "PerLengthLineParameter" ;
  rdfs:comment "Common type for per-length electrical catalogues describing line parameters."@en ;
  rdfs:isDefinedBy :Package_Standard ;
  rdfs:subClassOf cim:IdentifiedObject ;
  uml:id "EAID_FC3FCF92_2B9B_4682_A67E_92E95ECB844B" .

cim:PhaseCode a owl:Class ;
  rdfs:label "PhaseCode" ;
  rdfs:comment """Enumeration of phase identifiers. Allows designation of phases for both transmission and distribution equipment, circuits and loads.
Residential and small commercial loads are often served from single-phase, or split-phase, secondary circuits. Phases 1 and 2 refer to hot wires that are 180 degrees out of phase, while N refers to the neutral wire. Through single-phase transformer connections, these secondary circuits may be served from one or two of the primary phases A, B, and C. For three-phase loads, use the A, B, C phase codes instead of s12N."""@en ;
  rdfs:isDefinedBy :Package_CIMEnumerations ;
  uml:hasStereotype uml:enumeration ;
  uml:id "EAID_4725DEF0_D125_4768_99B3_4AC3649D5D11" .

cim:PostLineSensor a owl:Class ;
  rdfs:label "PostLineSensor" ;
  rdfs:comment "A sensor used mainly in overhead distribution networks as the source of both current and voltage measurements."@en ;
  rdfs:isDefinedBy :Package_Standard ;
  rdfs:subClassOf cim:Sensor ;
  uml:id "EAID_8D320412_377C_4633_907F_8E03F0F4C86E" .

cim:PotentialTransformer a owl:Class ;
  rdfs:label "PotentialTransformer" ;
  rdfs:comment "Instrument transformer (also known as Voltage Transformer) used to measure electrical qualities of the circuit that is being protected and/or monitored. Typically used as voltage transducer for the purpose of metering, protection, or sometimes auxiliary substation supply. A typical secondary voltage rating would be 120V."@en ;
  rdfs:isDefinedBy :Package_Standard ;
  rdfs:subClassOf cim:Sensor ;
  uml:id "EAID_0E35E5FE_7B55_4aa3_80E9_CEEE9E47B9A0" .

cim:PowerSystemResource a owl:Class ;
  rdfs:label "PowerSystemResource" ;
  rdfs:comment """A power system resource can be an item of equipment such as a Switch, an EquipmentContainer containing many individual items of equipment such as a 
Substation, or an organisational entity such as Company or SubControlArea.  This provides for the nesting of collections of PowerSystemResources within other PowerSystemResources. For example, a Switch could be a member of a Substation and a Substation could be a member of a division of a Company."""@en ;
  rdfs:isDefinedBy :Package_Standard ;
  rdfs:subClassOf cim:IdentifiedObject ;
  uml:id "EAID_145F8C8E_E0FE_434e_9E9A_BF57D2525227" .

cim:PowerTransformer a owl:Class ;
  rdfs:label "PowerTransformer" ;
  rdfs:comment """An electrical device consisting of  two or more coupled windings, with or without a magnetic core, for introducing mutual coupling between electric circuits. Transformers can be used to control voltage and phase shift (active power flow).
A power transformer may be composed of separate transformer tanks that need not be identical.
The same power transformer can be modelled in two ways, namely with and without tanks:
<ol>
 <li>The power transformer that uses power transformer ends directly (without tanks) is suitable for balanced three-phase models. This is typical for transmission and sub-transmission network modelling. Such a transformer will require one power transformer end for each physical winding. There must be a one-to-one association between PowerTransformerEnd and Core::Terminal.</li>
 <li>The power transformer that uses transformer tanks is suitable for an unbalanced transformer, a balanced transformer within a single tank, or a balanced transformer made up of three tanks. This is typical for distribution network modelling and the only choice when modelling an unbalanced transformer, or a transformer that has more than three windings. Power transformer modelled with tanks will require for each tank, one transformer tank end per physical winding in the tank. There may be one, two, or three phases in the transformer tank end.  Examples: 3 phases for 3-phase delta or wye connected windings, 2 for one phase-to-phase winding, and 1 for a phase-to-neutral or phase-to-ground winding.  With 1 or 2 phases, more than one transformer tank end may be associated to the same 3-phase Core::Terminal instance, while with 3 phases there should be a one-to-one association.</li>
</ol>
This power transformer model is flexible in order to support different kinds of data exchange requirements. There are 5 possible ways to combine available classes and their attributes:
<ol>
 <li>Instance parameters - Use the r, x, r0, x0, b, b0, g, and g0 attributes on PowerTransformerEnd and ignore related TransformerStarImpedance, TransformerMeshImpedance, or TransformerCoreAdmittance. This option assumes a star connection of the series impedances. It is suitable for typical transmission, balanced three-phase transformer models, for transformers with 2 or three windings.</li>
 <li>Star instance parameters by association - Instead of the r, x, r0, x0, b, b0, g, and g0 attributes, use associations to TransformerStarImpedance and TransformerCoreAdmitance. This option is suitable in same scenarios as option 1, but when catalogue data is available for transformers.</li>
 <li>Mesh instance parameters by association: Instead of the r, x, r0, x0, b, b0, g, and g0 attributes, use associations to TransformerMeshImpedance and TransformerCoreAdmittance. This option supports transformers with more than three windings.</li>
 <li>Catalog mesh parameters by association - Instead of attributes r, x, r0, x0, b, b0, g, and g0 and associations to TransformerStarImpedance, TransformerMeshImpedance, or TransformerCoreAdmittance, use the association to TransformerEndInfo. The TransformerEnd.endNumber should match the corresponding TransformerEndInfo.endNumber, following the IEC standard convention of numbering from the highest voltage ends to the lowest, starting at 1. This matching supports higher-level use of a catalog, through just one association between TransformerTank and TransformerTankInfo, with simpler exchanges and incremental updates. The associated TransformerEndInfo will have associations to TransformerMeshImpedance and TransformerCoreAdmittance. This option supports unbalanced transformer, with more than three windings and is suitable whenever the transformer test data has been converted to an electrical model.</li>
 <li>Catalog test data by association - This is the same as option 4, except TransformerEndInfo will have associations to AssetModels::TransformerTest decendents, instead of to TransformerMeshImpedance and TransformerCoreAdmittance.  This option is suitable when the test data is available, and the receiving application is able to interpret the test data.</li>
</ol>
Every profile should specify which one or more of these options are supported."""@en ;
  rdfs:isDefinedBy :Package_Standard ;
  rdfs:subClassOf cim:ConductingEquipment ;
  uml:id "EAID_0F117DB1_8A12_4956_BD82_6AB67CA63182" .

cim:PowerTransformerEnd a owl:Class ;
  rdfs:label "PowerTransformerEnd" ;
  rdfs:comment """A PowerTransformerEnd is associated with each Terminal of a PowerTransformer.
The impdedance values r, r0, x, and x0 of a PowerTransformerEnd represents a star equivalentas follows
1) for a two Terminal PowerTransformer the high voltage PowerTransformerEnd has non zero values on r, r0, x, and x0 while the low voltage PowerTransformerEnd has zero values for r, r0, x, and x0.
2) for a three Terminal PowerTransformer the three PowerTransformerEnds represents a star equivalent with each leg in the star represented by r, r0, x, and x0 values.
3) for a PowerTransformer with more than three Terminals the PowerTransformerEnd impedance values cannot be used. Instead use the TransformerMeshImpedance or split the transformer into multiple PowerTransformers."""@en ;
  rdfs:isDefinedBy :Package_Standard ;
  rdfs:subClassOf cim:TransformerEnd ;
  uml:id "EAID_51B4EF6E_CB7A_4c94_BC51_E227C501CAC2" .

cim:ProtectedSwitch a owl:Class ;
  rdfs:label "ProtectedSwitch" ;
  rdfs:comment "A ProtectedSwitch is a switching device that can be operated by ProtectionEquipment."@en ;
  rdfs:isDefinedBy :Package_Standard ;
  rdfs:subClassOf next:ProtectedSwitchEx ;
  uml:id "EAID_CB662EBD_C588_4d6b_94FA_887A73069C88" .

cim:ProtectionEquipment a owl:Class ;
  rdfs:label "ProtectionEquipment" ;
  rdfs:comment "An electrical device designed to respond to input conditions in a prescribed manner and after specified conditions are met to cause contact operation or similar abrupt change in associated electric control circuits, or simply to display the detected condition. Protection equipment are associated with conducting equipment and usually operate circuit breakers."@en ;
  rdfs:isDefinedBy :Package_Standard ;
  rdfs:subClassOf cim:Equipment ;
  uml:id "EAID_F11B8A0B_B9AF_480b_82FA_D0EC59DBFC73" .

cim:RE_UnitMultiplier a owl:Class ;
  rdfs:label "RE_UnitMultiplier" ;
  rdfs:comment "The unit multipliers defined for the CIM"@en ;
  rdfs:isDefinedBy :Package_CIMEnumerations ;
  uml:hasStereotype uml:enumeration ;
  uml:id "EAID_CCD2B42A_2923_46e8_8908_ABA4A853B758" .

cim:RE_UnitSymbol a owl:Class ;
  rdfs:label "RE_UnitSymbol" ;
  rdfs:comment "The units defiend for usage in the CIM"@en ;
  rdfs:isDefinedBy :Package_CIMEnumerations ;
  uml:hasStereotype uml:enumeration ;
  uml:id "EAID_82CF8971_5F46_440c_88F3_A1B5783F9EA7" .

cim:RaiseLowerCommand a owl:Class ;
  rdfs:label "RaiseLowerCommand" ;
  rdfs:comment "An analog control that increase or decrease a set point value with pulses."@en ;
  rdfs:isDefinedBy :Package_Standard ;
  rdfs:subClassOf cim:AnalogControl ;
  uml:id "EAID_798C80BB_25A6_4600_BB36_75B44B096048" .

cim:RatioTapChanger a owl:Class ;
  rdfs:label "RatioTapChanger" ;
  rdfs:comment "A tap changer that changes the voltage ratio impacting the voltage magnitude but not the phase angle across the transformer."@en ;
  rdfs:isDefinedBy :Package_Standard ;
  rdfs:subClassOf cim:TapChanger ;
  uml:id "EAID_BDF38D3F_B98A_4c6e_818F_46ED4F780172" .

cim:Recloser a owl:Class ;
  rdfs:label "Recloser" ;
  rdfs:comment "Pole-mounted fault interrupter with built-in phase and ground relays, current transformer (CT), and supplemental controls."@en ;
  rdfs:isDefinedBy :Package_Standard ;
  rdfs:subClassOf cim:ProtectedSwitch ;
  uml:id "EAID_F2EEE982_B4A7_4b59_8940_06E50F9C0D52" .

cim:RegularIntervalSchedule a owl:Class ;
  rdfs:label "RegularIntervalSchedule" ;
  rdfs:comment "The schedule has time points where the time between them is constant."@en ;
  rdfs:isDefinedBy :Package_Standard ;
  rdfs:subClassOf cim:BasicIntervalSchedule ;
  uml:id "EAID_CC553F0B_AA2C_476f_82A8_B998E464E446" .

cim:RegularTimePoint a owl:Class ;
  rdfs:label "RegularTimePoint" ;
  rdfs:comment "Time point for a schedule where the time between the consecutive points is constant."@en ;
  rdfs:isDefinedBy :Package_Standard ;
  uml:id "EAID_1723DD0A_5C8A_4639_8F9D_E8D13893D1CB" .

cim:RegulatingCondEq a owl:Class ;
  rdfs:label "RegulatingCondEq" ;
  rdfs:comment "A type of conducting equipment that can regulate a quanity (i.e. voltage or flow) at a specific point in the network."@en ;
  rdfs:isDefinedBy :Package_Standard ;
  rdfs:subClassOf cim:ConductingEquipment ;
  uml:id "EAID_3145239E_E13A_4e9d_86F6_E096AE0F76FA" .

cim:RegulatingControl a owl:Class ;
  rdfs:label "RegulatingControl" ;
  rdfs:comment """Specifies a set of equipment that works together to control a power system quantity such as voltage or flow. 
Remote bus voltage control is possible by specifying the controlled terminal located at some place remote from the controlling equipment.
In case multiple equipment, possibly of different types, control same terminal there must be only one RegulatingControl at that terminal. The most specific subtype of RegulatingControl shall be used in case such equipment participate in the control, e.g. TapChangerControl for tap changers.
For flow control  load sign convention is used, i.e. positive sign means flow out from a TopologicalNode (bus) into the conducting equipment."""@en ;
  rdfs:isDefinedBy :Package_Standard ;
  rdfs:subClassOf cim:PowerSystemResource ;
  uml:id "EAID_63BED673_836C_45b9_BA52_85F7047DA525" .

cim:RegulatingControlModeKind a owl:Class ;
  rdfs:label "RegulatingControlModeKind" ;
  rdfs:comment "The kind of regulation model.   For example regulating voltage, reactive power, active power, etc."@en ;
  rdfs:isDefinedBy :Package_CIMEnumerations ;
  uml:hasStereotype uml:enumeration ;
  uml:id "EAID_69E37D4A_38E7_4ba8_8F1B_2E0DC8735AAD" .

cim:RegulationSchedule a owl:Class ;
  rdfs:label "RegulationSchedule" ;
  rdfs:comment "A pre-established pattern over time for a controlled variable, e.g., busbar voltage."@en ;
  rdfs:isDefinedBy :Package_Standard ;
  rdfs:subClassOf cim:SeasonDayTypeSchedule ;
  uml:id "EAID_6078FC6D_B4BA_42c2_9048_7BD7AE4A7B0D" .

cim:RemoteControl a owl:Class ;
  rdfs:label "RemoteControl" ;
  rdfs:comment "Remote controls are ouputs that are sent by the remote unit to actuators in the process."@en ;
  rdfs:isDefinedBy :Package_Standard ;
  rdfs:subClassOf cim:RemotePoint ;
  uml:id "EAID_28BB6520_E06F_4b19_85E2_11EEF8598145" .

cim:RemotePoint a owl:Class ;
  rdfs:label "RemotePoint" ;
  rdfs:comment "For a RTU remote points correspond to telemetered values or control outputs. Other units (e.g. control centers) usually also contain calculated values."@en ;
  rdfs:isDefinedBy :Package_Standard ;
  rdfs:subClassOf cim:IdentifiedObject ;
  uml:id "EAID_74A411F4_A224_4106_A5E9_C8C886722300" .

cim:ReportingGroup a owl:Class ;
  rdfs:label "ReportingGroup" ;
  rdfs:comment "A reporting group is used for various ad-hoc groupings used for reporting."@en ;
  rdfs:isDefinedBy :Package_Standard ;
  rdfs:subClassOf cim:IdentifiedObject ;
  uml:id "EAID_0C0185F2_03C4_48d4_9276_CE47101731C9" .

cim:RotatingMachine a owl:Class ;
  rdfs:label "RotatingMachine" ;
  rdfs:comment "A rotating machine which may be used as a generator or motor."@en ;
  rdfs:isDefinedBy :Package_Standard ;
  rdfs:subClassOf cim:RegulatingCondEq ;
  uml:id "EAID_BFCF9287_59D8_4ee6_82CC_8BCC9D1FC5E1" .

cim:Season a owl:Class ;
  rdfs:label "Season" ;
  rdfs:comment "A specified time period of the year."@en ;
  rdfs:isDefinedBy :Package_Standard ;
  rdfs:subClassOf cim:IdentifiedObject ;
  uml:id "EAID_75F3FB30_972B_47fd_B63E_86F953B95964" .

cim:SeasonDayTypeSchedule a owl:Class ;
  rdfs:label "SeasonDayTypeSchedule" ;
  rdfs:comment "A time schedule covering a 24 hour period, with curve data for a specific type of season and day."@en ;
  rdfs:isDefinedBy :Package_Standard ;
  rdfs:subClassOf cim:RegularIntervalSchedule ;
  uml:id "EAID_0CC63187_722B_4113_A276_87A8FA4F62AC" .

cim:Sectionaliser a owl:Class ;
  rdfs:label "Sectionaliser" ;
  rdfs:comment "Automatic switch that will lock open to isolate a faulted section. It may, or may not, have load breaking capability. Its primary purpose is to provide fault sectionalising at locations where the fault current is either too high, or too low, for proper coordination of fuses."@en ;
  rdfs:isDefinedBy :Package_Standard ;
  rdfs:subClassOf cim:Switch ;
  uml:id "EAID_5392F289_FE58_497b_880B_2406D6F3B3E7" .

cim:Sensor a owl:Class ;
  rdfs:label "Sensor" ;
  rdfs:comment "This class describe devices that transform a measured quantity into signals that can be presented at displays, used in control or be recorded."@en ;
  rdfs:isDefinedBy :Package_Standard ;
  rdfs:subClassOf cim:AuxiliaryEquipment ;
  uml:id "EAID_BCFBA847_D945_4981_B95B_7B570DD1052D" .

cim:SetPoint a owl:Class ;
  rdfs:label "SetPoint" ;
  rdfs:comment "An analog control that issue a set point value."@en ;
  rdfs:isDefinedBy :Package_Standard ;
  rdfs:subClassOf cim:AnalogControl ;
  uml:id "EAID_6749251D_C548_482d_9D8F_DF5DC4C86E63" .

cim:ShuntCompensator a owl:Class ;
  rdfs:label "ShuntCompensator" ;
  rdfs:comment "A shunt capacitor or reactor or switchable bank of shunt capacitors or reactors. A section of a shunt compensator is an individual capacitor or reactor.  A negative value for reactivePerSection indicates that the compensator is a reactor. ShuntCompensator is a single terminal device.  Ground is implied."@en ;
  rdfs:isDefinedBy :Package_Standard ;
  rdfs:subClassOf cim:RegulatingCondEq ;
  uml:id "EAID_A5127983_B738_4060_94B3_456448DDB311" .

cim:SinglePhaseKind a owl:Class ;
  rdfs:label "SinglePhaseKind" ;
  rdfs:comment "Enumeration of single phase identifiers. Allows designation of single phases for both transmission and distribution equipment, circuits and loads."@en ;
  rdfs:isDefinedBy :Package_CIMEnumerations ;
  uml:hasStereotype uml:enumeration ;
  uml:id "EAID_F2284250_7D26_434c_BF35_98EA18648856" .

cim:SolarGeneratingUnit a owl:Class ;
  rdfs:label "SolarGeneratingUnit" ;
  rdfs:comment "A solar thermal generating unit."@en ;
  rdfs:isDefinedBy :Package_Standard ;
  rdfs:subClassOf cim:GeneratingUnit ;
  uml:id "EAID_64BC73F4_3663_45d0_9DBD_5A6B21567E7C" .

cim:Source a owl:Class ;
  rdfs:label "Source" ;
  rdfs:comment "Source gives information related to the origin of a value."@en ;
  rdfs:isDefinedBy :Package_CIMEnumerations ;
  uml:hasStereotype uml:enumeration ;
  uml:id "EAID_7CF6775C_176F_4790_9985_E2A403F01F15" .

cim:StationSupply a owl:Class ;
  rdfs:label "StationSupply" ;
  rdfs:comment "Station supply with load derived from the station output."@en ;
  rdfs:isDefinedBy :Package_Standard ;
  rdfs:subClassOf cim:EnergyConsumer ;
  uml:id "EAID_6FF3006A_0AAB_4839_8439_CD66423C4631" .

cim:Status a owl:Class ;
  rdfs:label "Status" ;
  rdfs:comment "Current status information relevant to an entity."@en ;
  rdfs:isDefinedBy :Package_CompoundTypes ;
  uml:hasStereotype uml:compound ;
  uml:id "EAID_C289C1B8_B2A7_44dc_9539_6FF6A864D9A7" .

cim:StreetAddress a owl:Class ;
  rdfs:label "StreetAddress" ;
  rdfs:comment "General purpose street address information."@en ;
  rdfs:isDefinedBy :Package_CompoundTypes ;
  uml:hasStereotype uml:compound ;
  uml:id "EAID_4E00C826_D63A_4b62_A6AA_D3C86C1D8D9A" .

cim:StreetDetail a owl:Class ;
  rdfs:label "StreetDetail" ;
  rdfs:comment "Street details, in the context of address."@en ;
  rdfs:isDefinedBy :Package_CompoundTypes ;
  uml:hasStereotype uml:compound ;
  uml:id "EAID_2896C068_81B3_4338_8314_BF55C9D20652" .

cim:StringMeasurement a owl:Class ;
  rdfs:label "StringMeasurement" ;
  rdfs:comment "StringMeasurement represents a measurement with values of type string."@en ;
  rdfs:isDefinedBy :Package_Standard ;
  rdfs:subClassOf cim:Measurement ;
  uml:id "EAID_430976AA_6463_4983_9D4B_06D34933CE41" .

cim:StringMeasurementValue a owl:Class ;
  rdfs:label "StringMeasurementValue" ;
  rdfs:comment "StringMeasurementValue represents a measurement value of type string."@en ;
  rdfs:isDefinedBy :Package_Standard ;
  rdfs:subClassOf cim:MeasurementValue ;
  uml:id "EAID_D02C6296_7E50_46d9_8158_87CDD4CD2DF8" .

cim:SubGeographicalRegion a owl:Class ;
  rdfs:label "SubGeographicalRegion" ;
  rdfs:comment "A subset of a geographical region of a power system network model."@en ;
  rdfs:isDefinedBy :Package_Standard ;
  rdfs:subClassOf cim:IdentifiedObject ;
  uml:id "EAID_EDA46C86_AA97_4c65_8B48_7D1A84037975" .

cim:SubLoadArea a owl:Class ;
  rdfs:label "SubLoadArea" ;
  rdfs:comment "The class is the second level in a hierarchical structure for grouping of loads for the purpose of load flow load scaling."@en ;
  rdfs:isDefinedBy :Package_Standard ;
  rdfs:subClassOf cim:EnergyArea ;
  uml:id "EAID_1EDB5897_A122_41aa_B4A9_3792F6159CA1" .

cim:Substation a owl:Class ;
  rdfs:label "Substation" ;
  rdfs:comment "A collection of equipment for purposes other than generation or utilization, through which electric energy in bulk is passed for the purposes of switching or modifying its characteristics."@en ;
  rdfs:isDefinedBy :Package_Standard ;
  rdfs:subClassOf cim:EquipmentContainer ;
  uml:id "EAID_4123E8A3_7DF3_4ed1_9709_2CDE1D89A67D" .

cim:SurgeArrester a owl:Class ;
  rdfs:label "SurgeArrester" ;
  rdfs:comment "Shunt device, installed on the network, usually in the proximity of electrical equipment in order to protect the said equipment against transient voltage transients caused by lightning or switching activity."@en ;
  rdfs:isDefinedBy :Package_Standard ;
  rdfs:subClassOf cim:AuxiliaryEquipment ;
  uml:id "EAID_BD9ACE42_6E9E_4ab3_BDEF_F1514F8F7A26" .

cim:Switch a owl:Class ;
  rdfs:label "Switch" ;
  rdfs:comment "A generic device designed to close, or open, or both, one or more electric circuits."@en ;
  rdfs:isDefinedBy :Package_Standard ;
  rdfs:subClassOf cim:ConductingEquipment ;
  uml:id "EAID_84DE6041_76B0_4c20_A330_A3323B08D12A" .

cim:SwitchSchedule a owl:Class ;
  rdfs:label "SwitchSchedule" ;
  rdfs:comment "A schedule of switch positions.  If RegularTimePoint.value1 is 0, the switch is open.  If 1, the switch is closed."@en ;
  rdfs:isDefinedBy :Package_Standard ;
  rdfs:subClassOf cim:SeasonDayTypeSchedule ;
  uml:id "EAID_2262FFF5_55A5_4115_8390_7437FD384910" .

cim:SynchronousMachine a owl:Class ;
  rdfs:label "SynchronousMachine" ;
  rdfs:comment "An electromechanical device that operates with shaft rotating synchronously with the network. It is a single machine operating either as a generator or synchronous condenser or pump."@en ;
  rdfs:isDefinedBy :Package_Standard ;
  rdfs:subClassOf cim:RotatingMachine ;
  uml:id "EAID_DD07A159_5291_4a78_86C9_257995AB052E" .

cim:SynchronousMachineKind a owl:Class ;
  rdfs:label "SynchronousMachineKind" ;
  rdfs:comment "Synchronous machine type."@en ;
  rdfs:isDefinedBy :Package_CIMEnumerations ;
  uml:hasStereotype uml:enumeration ;
  uml:id "EAID_0271C369_418B_4753_97E7_8F46A0235E90" .

cim:SynchronousMachineOperatingMode a owl:Class ;
  rdfs:label "SynchronousMachineOperatingMode" ;
  rdfs:comment "Synchronous machine operating mode."@en ;
  rdfs:isDefinedBy :Package_CIMEnumerations ;
  uml:hasStereotype uml:enumeration ;
  uml:id "EAID_9E79D1F1_41A0_49fe_85FD_4B4E849646A4" .

cim:TapChanger a owl:Class ;
  rdfs:label "TapChanger" ;
  rdfs:comment "Mechanism for changing transformer winding tap positions."@en ;
  rdfs:isDefinedBy :Package_Standard ;
  rdfs:subClassOf cim:PowerSystemResource ;
  uml:id "EAID_2CCC82F5_79A2_4262_A99D_20FCABFBBB1C" .

cim:TapChangerControl a owl:Class ;
  rdfs:label "TapChangerControl" ;
  rdfs:comment "Describes behavior specific to tap changers, e.g. how the voltage at the end of a line varies with the load level and compensation of the voltage drop by tap adjustment."@en ;
  rdfs:isDefinedBy :Package_Standard ;
  rdfs:subClassOf cim:RegulatingControl ;
  uml:id "EAID_1EFDA9C8_7D75_4f58_9B95_BD7319281343" .

cim:TapSchedule a owl:Class ;
  rdfs:label "TapSchedule" ;
  rdfs:comment "A pre-established pattern over time for a tap step."@en ;
  rdfs:isDefinedBy :Package_Standard ;
  rdfs:subClassOf cim:SeasonDayTypeSchedule ;
  uml:id "EAID_E4740339_4327_4d49_99C0_FAFC95DC21E1" .

cim:Terminal a owl:Class ;
  rdfs:label "Terminal" ;
  rdfs:comment "An electrical connection point to a piece of conducting equipment. Terminals are connected at physical connection points called \"connectivity nodes\"."@en ;
  rdfs:isDefinedBy :Package_Standard ;
  rdfs:subClassOf cim:ACDCTerminal ;
  uml:id "EAID_819D88BA_920C_49c5_AD51_557097EE2E7D" .

cim:ThermalGeneratingUnit a owl:Class ;
  rdfs:label "ThermalGeneratingUnit" ;
  rdfs:comment "A generating unit whose prime mover could be a steam turbine, combustion turbine, or diesel engine."@en ;
  rdfs:isDefinedBy :Package_Standard ;
  rdfs:subClassOf cim:GeneratingUnit ;
  uml:id "EAID_ADB95AC7_7EA0_47c5_A9A0_CC4071ABF9EA" .

cim:TownDetail a owl:Class ;
  rdfs:label "TownDetail" ;
  rdfs:comment "Town details, in the context of address."@en ;
  rdfs:isDefinedBy :Package_CompoundTypes ;
  uml:hasStereotype uml:compound ;
  uml:id "EAID_F6B511C6_7BF1_4322_9D5A_CECDA55A1F3F" .

cim:TransformerControlMode a owl:Class ;
  rdfs:label "TransformerControlMode" ;
  rdfs:comment "Control modes for a transformer."@en ;
  rdfs:isDefinedBy :Package_CIMEnumerations ;
  uml:hasStereotype uml:enumeration ;
  uml:id "EAID_30994180_C510_4a68_9CF1_36A25A1F79B5" .

cim:TransformerEnd a owl:Class ;
  rdfs:label "TransformerEnd" ;
  rdfs:comment "TransformerEnd is a conducting connection point of a power transformer. It corresponds to a physical transformer winding terminal.  In earlier CIM versions, the TransformerWinding class served a similar purpose. This successor TransformerEnd class is more flexible and has important differences with TransformerWinding."@en ;
  rdfs:isDefinedBy :Package_Standard ;
  rdfs:subClassOf cim:IdentifiedObject ;
  uml:id "EAID_C101350A_B9BD_473e_A774_489948CE2EFA" .

cim:UnitMultiplier a owl:Class ;
  rdfs:label "UnitMultiplier" ;
  rdfs:comment "The unit multipliers defined for the CIM"@en ;
  rdfs:isDefinedBy :Package_CIMEnumerations ;
  uml:hasStereotype uml:enumeration ;
  uml:id "EAID_64CEA0C6_6C26_41bd_B02E_00CF2F02A294" .

cim:UnitSymbol a owl:Class ;
  rdfs:label "UnitSymbol" ;
  rdfs:comment "The units defined for usage in the CIM."@en ;
  rdfs:isDefinedBy :Package_CIMEnumerations ;
  uml:hasStereotype uml:enumeration ;
  uml:id "EAID_0A91C126_5421_4ec9_868D_FAA0E1B091A9" .

cim:ValueAliasSet a owl:Class ;
  rdfs:label "ValueAliasSet" ;
  rdfs:comment "Describes the translation of a set of values into a name and is intendend to facilitate cusom translations. Each ValueAliasSet has a name, description etc. A specific Measurement may represent a discrete state like Open, Closed, Intermediate etc. This requires a translation from the MeasurementValue.value number to a string, e.g. 0-&gt;\"Invalid\", 1-&gt;\"Open\", 2-&gt;\"Closed\", 3-&gt;\"Intermediate\". Each ValueToAlias member in ValueAliasSet.Value describe a mapping for one particular value to a name."@en ;
  rdfs:isDefinedBy :Package_Standard ;
  rdfs:subClassOf cim:IdentifiedObject ;
  uml:id "EAID_0CE25BD9_C7E8_411b_A401_C6176B3C4E75" .

cim:ValueToAlias a owl:Class ;
  rdfs:label "ValueToAlias" ;
  rdfs:comment "Describes the translation of one particular value into a name, e.g. 1 as \"Open\"."@en ;
  rdfs:isDefinedBy :Package_Standard ;
  rdfs:subClassOf cim:IdentifiedObject ;
  uml:id "EAID_01270E58_ECDC_4a9b_A0F0_25E01D51BE4E" .

cim:VoltageLevel a owl:Class ;
  rdfs:label "VoltageLevel" ;
  rdfs:comment "A collection of equipment at one common system voltage forming a switchgear. The equipment typically consist of breakers, busbars, instrumentation, control, regulation and protection devices as well as assemblies of all these."@en ;
  rdfs:isDefinedBy :Package_Standard ;
  rdfs:subClassOf cim:EquipmentContainer ;
  uml:id "EAID_9540CB06_BC51_4f02_8113_57F4B1AE6B7C" .

cim:VoltageLimit a owl:Class ;
  rdfs:label "VoltageLimit" ;
  rdfs:comment "Operational limit applied to voltage."@en ;
  rdfs:isDefinedBy :Package_Standard ;
  rdfs:subClassOf cim:OperationalLimit ;
  uml:id "EAID_E7655AB8_4FE1_4767_8F5C_200BA8753B90" .

cim:VsConverter a owl:Class ;
  rdfs:label "VsConverter" ;
  rdfs:comment "DC side of the voltage source converter (VSC)."@en ;
  rdfs:isDefinedBy :Package_Standard ;
  rdfs:subClassOf cim:ACDCConverter ;
  uml:id "EAID_0AB0E871_744F_4064_80B4_C9B07B0C1D1D" .

cim:WindGenUnitKind a owl:Class ;
  rdfs:label "WindGenUnitKind" ;
  rdfs:comment "Kind of wind generating unit."@en ;
  rdfs:isDefinedBy :Package_CIMEnumerations ;
  uml:hasStereotype uml:enumeration ;
  uml:id "EAID_E7574EE8_C9C2_4466_B309_787007D5DA32" .

cim:WindGeneratingUnit a owl:Class ;
  rdfs:label "WindGeneratingUnit" ;
  rdfs:comment "A wind driven generating unit.  May be used to represent a single turbine or an aggregation."@en ;
  rdfs:isDefinedBy :Package_Standard ;
  rdfs:subClassOf cim:GeneratingUnit ;
  uml:id "EAID_3D7CA6F1_2797_4c3a_987B_5F1CEF77B423" .

cim:WindingConnection a owl:Class ;
  rdfs:label "WindingConnection" ;
  rdfs:comment "Winding connection type."@en ;
  rdfs:isDefinedBy :Package_CIMEnumerations ;
  uml:hasStereotype uml:enumeration ;
  uml:id "EAID_2079870A_25A3_4d77_98C3_B142C2FD391D" .

cim:WireInsulationKind a owl:Class ;
  rdfs:label "WireInsulationKind" ;
  rdfs:comment "Kind of wire insulation."@en ;
  rdfs:isDefinedBy :Package_CIMEnumerations ;
  uml:hasStereotype uml:enumeration ;
  uml:id "EAID_9C1C15AB_1FB5_4bd8_90AA_79939AC0A9F6" .

cim:WireMaterialKind a owl:Class ;
  rdfs:label "WireMaterialKind" ;
  rdfs:comment "Kind of wire material."@en ;
  rdfs:isDefinedBy :Package_CIMEnumerations ;
  uml:hasStereotype uml:enumeration ;
  uml:id "EAID_1F6368A6_BE59_418c_8DA4_DA1ACCA7A850" .

cim:WireUsageKind a owl:Class ;
  rdfs:label "WireUsageKind" ;
  rdfs:comment "Kind of wire usage."@en ;
  rdfs:isDefinedBy :Package_CIMEnumerations ;
  uml:hasStereotype uml:enumeration ;
  uml:id "EAID_3307BFA5_45D7_4cf5_91BD_0AA72AB03138" .

entsoe:ENTSOEOperationalLimitType a owl:Class ;
  rdfs:label "ENTSOEOperationalLimitType" ;
  rdfs:comment "The extension is described in the ENTSO-E document Policy 3 section 3 and appendix to Policy 3."@en ;
  rdfs:isDefinedBy :Package_EntsoeExtensions ;
  rdfs:subClassOf cim:IdentifiedObject ;
  uml:hasStereotype uml:entsoe ;
  uml:id "EAID_38850159_864B_4cd0_804C_DABFA7C5F7D5" .

entsoe:LimitTypeKind a owl:Class ;
  rdfs:label "LimitTypeKind" ;
  rdfs:comment "The enumeration defines the kinds of the limit types."@en ;
  rdfs:isDefinedBy :Package_EntsoeExtensions ;
  uml:hasStereotype uml:entsoe, uml:enumeration ;
  uml:id "EAID_F74847DE_6251_4d32_A07F_F0B465A31CB1" .

md:Description a owl:Class ;
  rdfs:label "Description" ;
  rdfs:comment "Identity contain comon descriptive information."@en ;
  rdfs:isDefinedBy :Package_ModelDescription ;
  uml:hasStereotype uml:deprecated ;
  uml:id "EAID_EA6429C5_DBE5_4667_A4E7_9B691DCB27C7" .

md:DescriptionID a owl:Class ;
  rdfs:label "DescriptionID" ;
  rdfs:isDefinedBy :Package_ModelDescription ;
  rdfs:subClassOf md:Description ;
  uml:hasStereotype uml:deprecated ;
  uml:id "EAID_11C3E838_F554_495b_9C57_BF88D3E00C11" .

md:DifferenceModel a owl:Class ;
  rdfs:label "DifferenceModel" ;
  rdfs:isDefinedBy :Package_ModelDescription ;
  rdfs:subClassOf md:Model ;
  uml:id "EAID_96A36E86_5379_448d_9604_56095A1905CE" .

md:FullModel a owl:Class ;
  rdfs:label "FullModel" ;
  rdfs:isDefinedBy :Package_ModelDescription ;
  rdfs:subClassOf md:Model ;
  uml:id "EAID_66403EF1_5399_499b_9023_9A568B9EDE41" .

md:FullModelDocumentElement a owl:Class ;
  rdfs:label "FullModelDocumentElement" ;
  rdfs:isDefinedBy :Package_ModelDescription ;
  uml:hasStereotype uml:deprecated ;
  uml:id "EAID_7D924A77_DD88_4aca_9D53_3285248B856D" .

md:Model a owl:Class ;
  rdfs:label "Model" ;
  rdfs:isDefinedBy :Package_ModelDescription ;
  uml:id "EAID_B6CC60A3_3A7C_4d1e_B87B_34B75E586359" .

md:ModelDescriptionCIMVersion a owl:Class ;
  rdfs:label "ModelDescriptionCIMVersion" ;
  rdfs:isDefinedBy :Package_ModelDescription ;
  uml:id "EAID_E5EE368A_4650_44ad_BE63_43EE2D9DFF2B" .

md:Statements a owl:Class ;
  rdfs:label "Statements" ;
  rdfs:isDefinedBy :Package_ModelDescription ;
  rdfs:subClassOf md:FullModelDocumentElement ;
  uml:id "EAID_1DF18623_9167_4901_9EA6_33DE8A0733D5" .

next2:EquipmentContainerEx a owl:Class ;
  rdfs:label "EquipmentContainer" ;
  rdfs:isDefinedBy :Package_CIMExtensions ;
  rdfs:subClassOf cim:ConnectivityNodeContainer ;
  uml:hasStereotype uml:extension ;
  uml:id "EAID_4DAFB8C1_215D_4b08_AEBD_35D4D91E7095" .

next3:WeatherStation a owl:Class ;
  rdfs:label "WeatherStation" ;
  rdfs:comment "This represents a source of ambient temperature."@en ;
  rdfs:isDefinedBy :Package_InfIEC61970 ;
  rdfs:subClassOf cim:PowerSystemResource ;
  uml:id "EAID_46BF6E9E_517E_4419_B75B_34999A20751B" .

next:EnergyConsumerEx a owl:Class ;
  rdfs:label "EnergyConsumer" ;
  rdfs:isDefinedBy :Package_EDFExtensionsFunctional ;
  rdfs:subClassOf cim:ConductingEquipment ;
  uml:hasStereotype uml:extension ;
  uml:id "EAID_6750DA82_1B95_49a3_B667_5CE80F0FED14" .

next:ProtectedSwitchEx a owl:Class ;
  rdfs:label "ProtectedSwitch" ;
  rdfs:isDefinedBy :Package_EDFExtensionsFunctional ;
  rdfs:subClassOf cim:Switch ;
  uml:hasStereotype uml:extension ;
  uml:id "EAID_30B22C4E_DB64_435f_92B6_D9CFC977A27E" .

uml:Package a owl:Class .

uml:Stereotype a owl:Class .

:ModelingAuthority.ModelingAuthoritySets a owl:ObjectProperty, owl:InverseFunctionalProperty ;
  rdfs:label "ModelingAuthoritySets" ;
  rdfs:comment "A Modeling Authority set supplies and maintains the data for the objects in a Modeling Authority Set."@en ;
  owl:inverseOf :ModelingAuthoritySet.ModelingAuthority ;
  rdfs:domain :ModelingAuthority ;
  rdfs:isDefinedBy :Package_ModelAuthority ;
  rdfs:range :ModelingAuthoritySet ;
  uml:id "EAID_DD1413D0_73ED_4d90_8ADB_E87B483F7D14-A" .

:ModelingAuthoritySet.ModelingAuthority a owl:ObjectProperty, owl:FunctionalProperty ;
  rdfs:label "ModelingAuthority" ;
  rdfs:comment "A Modeling Authority set supplies and maintains the data for the objects in a Modeling Authority Set."@en ;
  owl:inverseOf :ModelingAuthority.ModelingAuthoritySets ;
  rdfs:domain :ModelingAuthoritySet ;
  rdfs:isDefinedBy :Package_ModelAuthority ;
  rdfs:range :ModelingAuthority ;
  uml:id "EAID_DD1413D0_73ED_4d90_8ADB_E87B483F7D14-B" .

:PowerSystemProjectSchedule.status a owl:ObjectProperty, owl:FunctionalProperty ;
  rdfs:label "status" ;
  rdfs:domain :PowerSystemProjectSchedule ;
  rdfs:isDefinedBy :Package_PowerSystemProject ;
  rdfs:range :ProjectStepStatusKind ;
  uml:hasStereotype uml:attribute ;
  uml:id "EAID_A2782127_6316_4c7a_8FD3_0BAFF34696EA" .

:PowerSystemProjectSchedule.stepType a owl:ObjectProperty, owl:FunctionalProperty ;
  rdfs:label "stepType" ;
  rdfs:domain :PowerSystemProjectSchedule ;
  rdfs:isDefinedBy :Package_PowerSystemProject ;
  rdfs:range :StepKind ;
  uml:hasStereotype uml:attribute ;
  uml:id "EAID_E5F56033_237D_4136_B67F_992E49D34D4C" .

:ProjectStep.status a owl:ObjectProperty, owl:FunctionalProperty ;
  rdfs:label "status" ;
  rdfs:domain :ProjectStep ;
  rdfs:isDefinedBy :Package_PowerSystemProject ;
  rdfs:range :ProjectStepStatusKind ;
  uml:hasStereotype uml:attribute ;
  uml:id "EAID_066625C1_EB9A_4637_A571_09C23BB3A0ED" .

:ProjectStep.stepType a owl:ObjectProperty, owl:FunctionalProperty ;
  rdfs:label "stepType" ;
  rdfs:domain :ProjectStep ;
  rdfs:isDefinedBy :Package_PowerSystemProject ;
  rdfs:range :StepKind ;
  uml:hasStereotype uml:attribute ;
  uml:id "EAID_949103D0_A373_4f5d_BC2A_8CE9427856FA" .

cim:ACDCTerminal.Measurement a owl:ObjectProperty, owl:InverseFunctionalProperty ;
  rdfs:label "Measurement" ;
  rdfs:comment "Measurements associated with this terminal defining  where the measurement is placed in the network topology.  It may be used, for instance, to capture the sensor position, such as a voltage transformer (PT) at a busbar or a current transformer (CT) at the bar between a breaker and an isolator."@en ;
  owl:inverseOf cim:Measurement.Terminal ;
  rdfs:domain cim:ACDCTerminal ;
  rdfs:isDefinedBy :Package_Standard ;
  rdfs:range cim:Measurement ;
  uml:id "EAID_952C2E70_618A_4c2b_9D47_C2B175B263DB-B" .

cim:ACDCTerminal.OperationalLimitSet a owl:ObjectProperty, owl:InverseFunctionalProperty ;
  rdfs:label "OperationalLimitSet" ;
  owl:inverseOf cim:OperationalLimitSet.Terminal ;
  rdfs:domain cim:ACDCTerminal ;
  rdfs:isDefinedBy :Package_Standard ;
  rdfs:range cim:OperationalLimitSet ;
  uml:id "EAID_B879ACB4_5EB0_4709_8236_3964485589CC-B" .

cim:ACLineSegment.Clamp a owl:ObjectProperty, owl:InverseFunctionalProperty ;
  rdfs:label "Clamp" ;
  rdfs:comment "The clamps connected to the line segment."@en ;
  owl:inverseOf cim:Clamp.ACLineSegment ;
  rdfs:domain cim:ACLineSegment ;
  rdfs:isDefinedBy :Package_Standard ;
  rdfs:range cim:Clamp ;
  uml:id "EAID_CD424117_16E9_4ec6_A08A_B03B3DE0B125-B" .

cim:ACLineSegment.Cut a owl:ObjectProperty, owl:InverseFunctionalProperty ;
  rdfs:label "Cut" ;
  rdfs:comment "Cuts applied to the line segment."@en ;
  owl:inverseOf cim:Cut.ACLineSegment ;
  rdfs:domain cim:ACLineSegment ;
  rdfs:isDefinedBy :Package_Standard ;
  rdfs:range cim:Cut ;
  uml:id "EAID_D952CA2E_6735_446b_A713_D60C651C7ECA-B" .

cim:ACLineSegment.PerLengthImpedance a owl:ObjectProperty, owl:FunctionalProperty ;
  rdfs:label "PerLengthImpedance" ;
  rdfs:comment "Per-length impedance of this line segment."@en ;
  owl:inverseOf cim:PerLengthImpedance.ACLineSegment ;
  rdfs:domain cim:ACLineSegment ;
  rdfs:isDefinedBy :Package_Standard ;
  rdfs:range cim:PerLengthImpedance ;
  uml:id "EAID_BA020DF3_CA9A_4d46_B70E_F7FC12EFBD94-A" .

cim:Accumulator.AccumulatorValue a owl:ObjectProperty, owl:InverseFunctionalProperty ;
  rdfs:label "AccumulatorValue" ;
  rdfs:comment "The values connected to this measurement."@en ;
  owl:inverseOf cim:AccumulatorValue.Accumulator ;
  rdfs:domain cim:Accumulator ;
  rdfs:isDefinedBy :Package_Standard ;
  rdfs:range cim:AccumulatorValue ;
  uml:id "EAID_47F75C09_9528_490a_AD83_A0CC63D07545-B" .

cim:Accumulator.LimitSets a owl:ObjectProperty ;
  rdfs:label "LimitSets" ;
  rdfs:comment "A measurement may have zero or more limit ranges defined for it."@en ;
  owl:inverseOf cim:AccumulatorLimitSet.Measurements ;
  rdfs:domain cim:Accumulator ;
  rdfs:isDefinedBy :Package_Standard ;
  rdfs:range cim:AccumulatorLimitSet ;
  uml:id "EAID_CF7F424F_B8EA_440b_B8E3_7A4C4CDF5524-B" .

cim:AccumulatorLimit.LimitSet a owl:ObjectProperty, owl:FunctionalProperty ;
  rdfs:label "LimitSet" ;
  rdfs:comment "The set of limits."@en ;
  owl:inverseOf cim:AccumulatorLimitSet.Limits ;
  rdfs:domain cim:AccumulatorLimit ;
  rdfs:isDefinedBy :Package_Standard ;
  rdfs:range cim:AccumulatorLimitSet ;
  uml:hasStereotype uml:ofAggregate ;
  uml:id "EAID_C9F2D6E7_87E6_477c_8325_5A2C63E5F33A-A" .

cim:AccumulatorLimitSet.Limits a owl:ObjectProperty, owl:InverseFunctionalProperty ;
  rdfs:label "Limits" ;
  rdfs:comment "The limit values used for supervision of Measurements."@en ;
  owl:inverseOf cim:AccumulatorLimit.LimitSet ;
  rdfs:domain cim:AccumulatorLimitSet ;
  rdfs:isDefinedBy :Package_Standard ;
  rdfs:range cim:AccumulatorLimit ;
  uml:hasStereotype uml:aggregateOf ;
  uml:id "EAID_C9F2D6E7_87E6_477c_8325_5A2C63E5F33A-B" .

cim:AccumulatorLimitSet.Measurements a owl:ObjectProperty ;
  rdfs:label "Measurements" ;
  rdfs:comment "The Measurements using the LimitSet."@en ;
  owl:inverseOf cim:Accumulator.LimitSets ;
  rdfs:domain cim:AccumulatorLimitSet ;
  rdfs:isDefinedBy :Package_Standard ;
  rdfs:range cim:Accumulator ;
  uml:id "EAID_CF7F424F_B8EA_440b_B8E3_7A4C4CDF5524-A" .

cim:AccumulatorReset.AccumulatorValue a owl:ObjectProperty, owl:FunctionalProperty, owl:InverseFunctionalProperty ;
  rdfs:label "AccumulatorValue" ;
  rdfs:comment "The accumulator value that is reset by the command."@en ;
  owl:inverseOf cim:AccumulatorValue.AccumulatorReset ;
  rdfs:domain cim:AccumulatorReset ;
  rdfs:isDefinedBy :Package_Standard ;
  rdfs:range cim:AccumulatorValue ;
  uml:id "EAID_1DD8A1E5_3391_4c2e_BC4E_D3CCAF014A8F-A" .

cim:AccumulatorValue.Accumulator a owl:ObjectProperty, owl:FunctionalProperty ;
  rdfs:label "Accumulator" ;
  rdfs:comment "Measurement to which this value is connected."@en ;
  owl:inverseOf cim:Accumulator.AccumulatorValue ;
  rdfs:domain cim:AccumulatorValue ;
  rdfs:isDefinedBy :Package_Standard ;
  rdfs:range cim:Accumulator ;
  uml:id "EAID_47F75C09_9528_490a_AD83_A0CC63D07545-A" .

cim:AccumulatorValue.AccumulatorReset a owl:ObjectProperty, owl:FunctionalProperty, owl:InverseFunctionalProperty ;
  rdfs:label "AccumulatorReset" ;
  rdfs:comment "The command that reset the accumulator value."@en ;
  owl:inverseOf cim:AccumulatorReset.AccumulatorValue ;
  rdfs:domain cim:AccumulatorValue ;
  rdfs:isDefinedBy :Package_Standard ;
  rdfs:range cim:AccumulatorReset ;
  uml:id "EAID_1DD8A1E5_3391_4c2e_BC4E_D3CCAF014A8F-B" .

cim:ActivePowerLimit.value a owl:ObjectProperty, owl:DatatypeProperty, owl:FunctionalProperty ;
  rdfs:label "value" ;
  rdfs:comment "Value of active power limit."@en ;
  rdfs:domain cim:ActivePowerLimit ;
  rdfs:isDefinedBy :Package_Standard ;
  rdfs:range cim:ActivePower ;
  uml:hasStereotype uml:attribute ;
  uml:id "EAID_4A3D363F_82D3_46ad_B0D0_3D233C5B15F6" .

cim:ActivityRecord.status a owl:ObjectProperty, owl:FunctionalProperty ;
  rdfs:label "status" ;
  rdfs:comment "Information on consequence of event resulting in this activity record."@en ;
  rdfs:domain cim:ActivityRecord ;
  rdfs:isDefinedBy :Package_Standard ;
  rdfs:range cim:Status ;
  uml:hasStereotype uml:attribute ;
  uml:id "EAID_9FDE0E95_306A_4092_8C74_FC42DE73E012" .

cim:Analog.AnalogValue a owl:ObjectProperty, owl:InverseFunctionalProperty ;
  rdfs:label "AnalogValue" ;
  rdfs:comment "The values connected to this measurement."@en ;
  owl:inverseOf cim:AnalogValue.Analog ;
  rdfs:domain cim:Analog ;
  rdfs:isDefinedBy :Package_Standard ;
  rdfs:range cim:AnalogValue ;
  uml:id "EAID_C323C320_A651_4286_88F9_DA3316A0461F-B" .

cim:Analog.LimitSets a owl:ObjectProperty ;
  rdfs:label "LimitSets" ;
  rdfs:comment "A measurement may have zero or more limit ranges defined for it."@en ;
  owl:inverseOf cim:AnalogLimitSet.Measurements ;
  rdfs:domain cim:Analog ;
  rdfs:isDefinedBy :Package_Standard ;
  rdfs:range cim:AnalogLimitSet ;
  uml:id "EAID_FC5DEA10_D4AC_4618_87DA_563AD51932C5-A" .

cim:AnalogControl.AnalogValue a owl:ObjectProperty, owl:FunctionalProperty, owl:InverseFunctionalProperty ;
  rdfs:label "AnalogValue" ;
  rdfs:comment "The MeasurementValue that is controlled."@en ;
  owl:inverseOf cim:AnalogValue.AnalogControl ;
  rdfs:domain cim:AnalogControl ;
  rdfs:isDefinedBy :Package_Standard ;
  rdfs:range cim:AnalogValue ;
  uml:id "EAID_1E59E228_D5A3_4216_84C3_9E1802903584-A" .

cim:AnalogLimit.LimitSet a owl:ObjectProperty, owl:FunctionalProperty ;
  rdfs:label "LimitSet" ;
  rdfs:comment "The set of limits."@en ;
  owl:inverseOf cim:AnalogLimitSet.Limit ;
  rdfs:domain cim:AnalogLimit ;
  rdfs:isDefinedBy :Package_Standard ;
  rdfs:range cim:AnalogLimitSet ;
  uml:hasStereotype uml:ofAggregate ;
  uml:id "EAID_E918C7D8_F416_4bdf_9B6B_839B6FF58F11-A" .

cim:AnalogLimitSet.Limit a owl:ObjectProperty, owl:InverseFunctionalProperty ;
  rdfs:label "Limit" ;
  rdfs:comment "The limit values used for supervision of Measurements."@en ;
  owl:inverseOf cim:AnalogLimit.LimitSet ;
  rdfs:domain cim:AnalogLimitSet ;
  rdfs:isDefinedBy :Package_Standard ;
  rdfs:range cim:AnalogLimit ;
  uml:hasStereotype uml:aggregateOf ;
  uml:id "EAID_E918C7D8_F416_4bdf_9B6B_839B6FF58F11-B" .

cim:AnalogLimitSet.Measurements a owl:ObjectProperty ;
  rdfs:label "Measurements" ;
  rdfs:comment "The Measurements using the LimitSet."@en ;
  owl:inverseOf cim:Analog.LimitSets ;
  rdfs:domain cim:AnalogLimitSet ;
  rdfs:isDefinedBy :Package_Standard ;
  rdfs:range cim:Analog ;
  uml:id "EAID_FC5DEA10_D4AC_4618_87DA_563AD51932C5-B" .

cim:AnalogValue.Analog a owl:ObjectProperty, owl:FunctionalProperty ;
  rdfs:label "Analog" ;
  rdfs:comment "Measurement to which this value is connected."@en ;
  owl:inverseOf cim:Analog.AnalogValue ;
  rdfs:domain cim:AnalogValue ;
  rdfs:isDefinedBy :Package_Standard ;
  rdfs:range cim:Analog ;
  uml:id "EAID_C323C320_A651_4286_88F9_DA3316A0461F-A" .

cim:AnalogValue.AnalogControl a owl:ObjectProperty, owl:FunctionalProperty, owl:InverseFunctionalProperty ;
  rdfs:label "AnalogControl" ;
  rdfs:comment "The Control variable associated with the MeasurementValue."@en ;
  owl:inverseOf cim:AnalogControl.AnalogValue ;
  rdfs:domain cim:AnalogValue ;
  rdfs:isDefinedBy :Package_Standard ;
  rdfs:range cim:AnalogControl ;
  uml:id "EAID_1E59E228_D5A3_4216_84C3_9E1802903584-B" .

cim:ApparentPowerLimit.value a owl:ObjectProperty, owl:DatatypeProperty, owl:FunctionalProperty ;
  rdfs:label "value" ;
  rdfs:comment "The apparent power limit."@en ;
  rdfs:domain cim:ApparentPowerLimit ;
  rdfs:isDefinedBy :Package_Standard ;
  rdfs:range cim:ApparentPower ;
  uml:hasStereotype uml:attribute ;
  uml:id "EAID_082AF792_5FB3_425a_BB82_89DBA7919AE7" .

cim:AssetInfo.PowerSystemResource a owl:ObjectProperty, owl:InverseFunctionalProperty ;
  rdfs:label "PowerSystemResource" ;
  rdfs:comment "All power system resources with this datasheet information."@en ;
  owl:inverseOf cim:PowerSystemResource.AssetDatasheet ;
  rdfs:domain cim:AssetInfo ;
  rdfs:isDefinedBy :Package_Standard ;
  rdfs:range cim:PowerSystemResource ;
  uml:id "EAID_146AFA1E_C3CB_4681_9EBE_B586F18C7410-B" .

cim:AuxiliaryEquipment.Terminal a owl:ObjectProperty, owl:FunctionalProperty ;
  rdfs:label "Terminal" ;
  rdfs:comment "The Terminal at the equipment where the AuxiliaryEquipment is attached."@en ;
  owl:inverseOf cim:Terminal.AuxiliaryEquipment ;
  rdfs:domain cim:AuxiliaryEquipment ;
  rdfs:isDefinedBy :Package_Standard ;
  rdfs:range cim:Terminal ;
  uml:id "EAID_3CC8CF1D_CF6F_4b11_89E9_C843D6C7581B-A" .

cim:BaseVoltage.ConductingEquipment a owl:ObjectProperty, owl:InverseFunctionalProperty ;
  rdfs:label "ConductingEquipment" ;
  rdfs:comment "All conducting equipment with this base voltage.  Use only when there is no voltage level container used and only one base voltage applies.  For example, not used for transformers."@en ;
  owl:inverseOf cim:ConductingEquipment.BaseVoltage ;
  rdfs:domain cim:BaseVoltage ;
  rdfs:isDefinedBy :Package_Standard ;
  rdfs:range cim:ConductingEquipment ;
  uml:id "EAID_7D53DD1D_52C9_49b3_ABE9_3776188CFA91-B" .

cim:BaseVoltage.VoltageLevel a owl:ObjectProperty, owl:InverseFunctionalProperty ;
  rdfs:label "VoltageLevel" ;
  rdfs:comment "The voltage levels having this base voltage."@en ;
  owl:inverseOf cim:VoltageLevel.BaseVoltage ;
  rdfs:domain cim:BaseVoltage ;
  rdfs:isDefinedBy :Package_Standard ;
  rdfs:range cim:VoltageLevel ;
  uml:id "EAID_B6CD04E3_BF6F_4e11_9354_61425EDE1CAD-B" .

cim:BaseVoltage.nominalVoltage a owl:ObjectProperty, owl:DatatypeProperty, owl:FunctionalProperty ;
  rdfs:label "nominalVoltage" ;
  rdfs:comment "The PowerSystemResource's base voltage."@en ;
  rdfs:domain cim:BaseVoltage ;
  rdfs:isDefinedBy :Package_Standard ;
  rdfs:range cim:Voltage ;
  uml:hasStereotype uml:attribute ;
  uml:id "EAID_38234C29_3762_4080_B7E8_4317A4C85DCF" .

cim:BasicIntervalSchedule.value1Unit a owl:ObjectProperty, owl:FunctionalProperty ;
  rdfs:label "value1Unit" ;
  rdfs:comment "Value1 units of measure."@en ;
  rdfs:domain cim:BasicIntervalSchedule ;
  rdfs:isDefinedBy :Package_Standard ;
  rdfs:range cim:UnitSymbol ;
  uml:hasStereotype uml:attribute ;
  uml:id "EAID_2A0D45E1_F3AA_4545_8483_116E81A78117" .

cim:BasicIntervalSchedule.value2Unit a owl:ObjectProperty, owl:FunctionalProperty ;
  rdfs:label "value2Unit" ;
  rdfs:comment "Value2 units of measure."@en ;
  rdfs:domain cim:BasicIntervalSchedule ;
  rdfs:isDefinedBy :Package_Standard ;
  rdfs:range cim:UnitSymbol ;
  uml:hasStereotype uml:attribute ;
  uml:id "EAID_50745734_E579_48f7_B082_CC844A8C388A" .

cim:Bay.Substation a owl:ObjectProperty, owl:FunctionalProperty ;
  rdfs:label "Substation" ;
  rdfs:comment "The association is used in the naming hierarchy."@en ;
  rdfs:domain cim:Bay ;
  rdfs:isDefinedBy :Package_Standard ;
  rdfs:range cim:Substation ;
  uml:hasStereotype uml:ofAggregate ;
  uml:id "EAID_8F76E16C_8CFC_4acd_B634_151EBB335770-A" .

cim:Bay.VoltageLevel a owl:ObjectProperty, owl:FunctionalProperty ;
  rdfs:label "VoltageLevel" ;
  rdfs:comment "The association is used in the naming hierarchy."@en ;
  rdfs:domain cim:Bay ;
  rdfs:isDefinedBy :Package_Standard ;
  rdfs:range cim:VoltageLevel ;
  uml:hasStereotype uml:ofAggregate ;
  uml:id "EAID_64BB6D04_DB15_4631_B9A0_805DC5278480-A" .

cim:Clamp.ACLineSegment a owl:ObjectProperty, owl:FunctionalProperty ;
  rdfs:label "ACLineSegment" ;
  rdfs:comment "The line segment to which the clamp is connected."@en ;
  owl:inverseOf cim:ACLineSegment.Clamp ;
  rdfs:domain cim:Clamp ;
  rdfs:isDefinedBy :Package_Standard ;
  rdfs:range cim:ACLineSegment ;
  uml:id "EAID_CD424117_16E9_4ec6_A08A_B03B3DE0B125-A" .

cim:Clamp.lengthFromTerminal1 a owl:ObjectProperty, owl:DatatypeProperty, owl:FunctionalProperty ;
  rdfs:label "lengthFromTerminal1" ;
  rdfs:comment "The length to the place where the clamp is located starting from side one of the line segment, i.e. the line segment terminal with sequence number equal to 1."@en ;
  rdfs:domain cim:Clamp ;
  rdfs:isDefinedBy :Package_Standard ;
  rdfs:range cim:Length ;
  uml:hasStereotype uml:attribute ;
  uml:id "EAID_F6B87894_AE48_409a_8D76_ABE4F7FC8D5D" .

cim:Command.DiscreteValue a owl:ObjectProperty, owl:FunctionalProperty, owl:InverseFunctionalProperty ;
  rdfs:label "DiscreteValue" ;
  rdfs:comment "The MeasurementValue that is controlled."@en ;
  owl:inverseOf cim:DiscreteValue.Command ;
  rdfs:domain cim:Command ;
  rdfs:isDefinedBy :Package_Standard ;
  rdfs:range cim:DiscreteValue ;
  uml:id "EAID_43AED751_ECB2_4afe_A6AC_63ABFE11AA4A-A" .

cim:Command.ValueAliasSet a owl:ObjectProperty, owl:FunctionalProperty ;
  rdfs:label "ValueAliasSet" ;
  rdfs:comment "The ValueAliasSet used for translation of a Control value to a name."@en ;
  owl:inverseOf cim:ValueAliasSet.Command ;
  rdfs:domain cim:Command ;
  rdfs:isDefinedBy :Package_Standard ;
  rdfs:range cim:ValueAliasSet ;
  uml:id "EAID_944A3138_E14B_487b_9B2D_A249CF9BC5FD-A" .

cim:ConductingEquipment.BaseVoltage a owl:ObjectProperty, owl:FunctionalProperty ;
  rdfs:label "BaseVoltage" ;
  rdfs:comment "Base voltage of this conducting equipment.  Use only when there is no voltage level container used and only one base voltage applies.  For example, not used for transformers."@en ;
  owl:inverseOf cim:BaseVoltage.ConductingEquipment ;
  rdfs:domain cim:ConductingEquipment ;
  rdfs:isDefinedBy :Package_Standard ;
  rdfs:range cim:BaseVoltage ;
  uml:id "EAID_7D53DD1D_52C9_49b3_ABE9_3776188CFA91-A" .

cim:ConductingEquipment.ProtectionEquipments a owl:ObjectProperty ;
  rdfs:label "ProtectionEquipments" ;
  rdfs:comment "Protection equipment  used to protect specific conducting equipment."@en ;
  owl:inverseOf cim:ProtectionEquipment.ConductingEquipments ;
  rdfs:domain cim:ConductingEquipment ;
  rdfs:isDefinedBy :Package_Standard ;
  rdfs:range cim:ProtectionEquipment ;
  uml:hasStereotype uml:aggregateOf ;
  uml:id "EAID_8CF444BF_B136_4069_91E7_DB736553CE53-B" .

cim:ConductingEquipment.Terminal a owl:ObjectProperty, owl:InverseFunctionalProperty ;
  rdfs:label "Terminal" ;
  rdfs:comment "Conducting equipment have terminals that may be connected to other conducting equipment terminals via connectivity nodes or topological nodes."@en ;
  owl:inverseOf cim:Terminal.ConductingEquipment ;
  rdfs:domain cim:ConductingEquipment ;
  rdfs:isDefinedBy :Package_Standard ;
  rdfs:range cim:Terminal ;
  uml:id "EAID_64D6B527_CC81_4f6a_BAB9_22FC5E218F34-B" .

cim:Conductor.length a owl:ObjectProperty, owl:DatatypeProperty, owl:FunctionalProperty ;
  rdfs:label "length" ;
  rdfs:comment "Segment length for calculating line section capabilities"@en ;
  rdfs:domain cim:Conductor ;
  rdfs:isDefinedBy :Package_Standard ;
  rdfs:range cim:Length ;
  uml:hasStereotype uml:attribute ;
  uml:id "EAID_26460FE3_C4CD_46b0_A64E_8B9462D3735A" .

cim:ConformLoad.LoadGroup a owl:ObjectProperty, owl:FunctionalProperty ;
  rdfs:label "LoadGroup" ;
  rdfs:comment "Group of this ConformLoad."@en ;
  owl:inverseOf cim:ConformLoadGroup.EnergyConsumer ;
  rdfs:domain cim:ConformLoad ;
  rdfs:isDefinedBy :Package_Standard ;
  rdfs:range cim:ConformLoadGroup ;
  uml:id "EAID_A2F17BAB_1215_46d6_B71F_435A607510E4-A" .

cim:ConformLoadGroup.ConformLoadSchedule a owl:ObjectProperty, owl:InverseFunctionalProperty ;
  rdfs:label "ConformLoadSchedule" ;
  rdfs:comment "The ConformLoadSchedules in the ConformLoadGroup."@en ;
  owl:inverseOf cim:ConformLoadSchedule.ConformLoadGroup ;
  rdfs:domain cim:ConformLoadGroup ;
  rdfs:isDefinedBy :Package_Standard ;
  rdfs:range cim:ConformLoadSchedule ;
  uml:hasStereotype uml:aggregateOf ;
  uml:id "EAID_6BDDF3FD_5CB3_4e02_9784_FC8C2A967B78-B" .

cim:ConformLoadGroup.EnergyConsumer a owl:ObjectProperty, owl:InverseFunctionalProperty ;
  rdfs:label "EnergyConsumer" ;
  rdfs:comment "Conform loads assigned to this ConformLoadGroup."@en ;
  owl:inverseOf cim:ConformLoad.LoadGroup ;
  rdfs:domain cim:ConformLoadGroup ;
  rdfs:isDefinedBy :Package_Standard ;
  rdfs:range cim:ConformLoad ;
  uml:id "EAID_A2F17BAB_1215_46d6_B71F_435A607510E4-B" .

cim:ConformLoadSchedule.ConformLoadGroup a owl:ObjectProperty, owl:FunctionalProperty ;
  rdfs:label "ConformLoadGroup" ;
  rdfs:comment "The ConformLoadGroup where the ConformLoadSchedule belongs."@en ;
  owl:inverseOf cim:ConformLoadGroup.ConformLoadSchedule ;
  rdfs:domain cim:ConformLoadSchedule ;
  rdfs:isDefinedBy :Package_Standard ;
  rdfs:range cim:ConformLoadGroup ;
  uml:hasStereotype uml:ofAggregate ;
  uml:id "EAID_6BDDF3FD_5CB3_4e02_9784_FC8C2A967B78-A" .

cim:ConnectivityNode.ConnectivityNodeContainer a owl:ObjectProperty, owl:FunctionalProperty ;
  rdfs:label "ConnectivityNodeContainer" ;
  rdfs:comment "Container of this connectivity node."@en ;
  owl:inverseOf cim:ConnectivityNodeContainer.ConnectivityNode ;
  rdfs:domain cim:ConnectivityNode ;
  rdfs:isDefinedBy :Package_Standard ;
  rdfs:range cim:ConnectivityNodeContainer ;
  uml:id "EAID_31C8B673_3922_44d0_81ED_6D73FD506D8A-A" .

cim:ConnectivityNode.Terminal a owl:ObjectProperty, owl:InverseFunctionalProperty ;
  rdfs:label "Terminal" ;
  rdfs:comment "Terminals interconnected with zero impedance at a this connectivity node."@en ;
  owl:inverseOf cim:Terminal.ConnectivityNode ;
  rdfs:domain cim:ConnectivityNode ;
  rdfs:isDefinedBy :Package_Standard ;
  rdfs:range cim:Terminal ;
  uml:id "EAID_FA200B53_A524_49d4_AA56_BE2DFC130DAC-B" .

cim:ConnectivityNodeContainer.ConnectivityNode a owl:ObjectProperty, owl:InverseFunctionalProperty ;
  rdfs:label "ConnectivityNode" ;
  rdfs:comment "Connectivity nodes which belong to this connectivity node container."@en ;
  owl:inverseOf cim:ConnectivityNode.ConnectivityNodeContainer ;
  rdfs:domain cim:ConnectivityNodeContainer ;
  rdfs:isDefinedBy :Package_Standard ;
  rdfs:range cim:ConnectivityNode ;
  uml:id "EAID_31C8B673_3922_44d0_81ED_6D73FD506D8A-B" .

cim:Control.PowerSystemResource a owl:ObjectProperty, owl:FunctionalProperty ;
  rdfs:label "PowerSystemResource" ;
  rdfs:comment "Regulating device governed by this control output."@en ;
  owl:inverseOf cim:PowerSystemResource.Control ;
  rdfs:domain cim:Control ;
  rdfs:isDefinedBy :Package_Standard ;
  rdfs:range cim:PowerSystemResource ;
  uml:id "EAID_DA4BF365_6235_482d_B3A8_9AF7E39CCAE4-A" .

cim:Control.RemoteControl a owl:ObjectProperty, owl:FunctionalProperty, owl:InverseFunctionalProperty ;
  rdfs:label "RemoteControl" ;
  rdfs:comment "The remote point controlling the physical actuator."@en ;
  owl:inverseOf cim:RemoteControl.Control ;
  rdfs:domain cim:Control ;
  rdfs:isDefinedBy :Package_Standard ;
  rdfs:range cim:RemoteControl ;
  uml:id "EAID_B9A6DD8E_EA10_4c56_9AC9_5F4188962209-B" .

cim:Control.unitMultiplier a owl:ObjectProperty, owl:FunctionalProperty ;
  rdfs:label "unitMultiplier" ;
  rdfs:comment "The unit multiplier of the controlled quantity."@en ;
  rdfs:domain cim:Control ;
  rdfs:isDefinedBy :Package_Standard ;
  rdfs:range cim:UnitMultiplier ;
  uml:hasStereotype uml:attribute ;
  uml:id "EAID_BE35ADCA_CA21_4253_BC4D_94653A2D7C01" .

cim:Control.unitSymbol a owl:ObjectProperty, owl:FunctionalProperty ;
  rdfs:label "unitSymbol" ;
  rdfs:comment "The unit of measure of the controlled quantity."@en ;
  rdfs:domain cim:Control ;
  rdfs:isDefinedBy :Package_Standard ;
  rdfs:range cim:UnitSymbol ;
  uml:hasStereotype uml:attribute ;
  uml:id "EAID_09B4E9A0_0161_40a4_9804_33C24984A2F7" .

cim:CurrentLimit.value a owl:ObjectProperty, owl:DatatypeProperty, owl:FunctionalProperty ;
  rdfs:label "value" ;
  rdfs:comment "Limit on current flow."@en ;
  rdfs:domain cim:CurrentLimit ;
  rdfs:isDefinedBy :Package_Standard ;
  rdfs:range cim:CurrentFlow ;
  uml:hasStereotype uml:attribute ;
  uml:id "EAID_5719C495_2A3C_40ba_B7A5_BF63D6491FBF" .

cim:Cut.ACLineSegment a owl:ObjectProperty, owl:FunctionalProperty ;
  rdfs:label "ACLineSegment" ;
  rdfs:comment "The line segment to which the cut is applied."@en ;
  owl:inverseOf cim:ACLineSegment.Cut ;
  rdfs:domain cim:Cut ;
  rdfs:isDefinedBy :Package_Standard ;
  rdfs:range cim:ACLineSegment ;
  uml:id "EAID_D952CA2E_6735_446b_A713_D60C651C7ECA-A" .

cim:Cut.lengthFromTerminal1 a owl:ObjectProperty, owl:DatatypeProperty, owl:FunctionalProperty ;
  rdfs:label "lengthFromTerminal1" ;
  rdfs:comment "The length to the place where the cut is located starting from side one of the cut line segment, i.e. the line segment Terminal with sequenceNumber equal to 1."@en ;
  rdfs:domain cim:Cut ;
  rdfs:isDefinedBy :Package_Standard ;
  rdfs:range cim:Length ;
  uml:hasStereotype uml:attribute ;
  uml:id "EAID_E3272969_E2AF_470e_96CC_13D8F5218A8C" .

cim:DayType.SeasonDayTypeSchedule a owl:ObjectProperty, owl:InverseFunctionalProperty ;
  rdfs:label "SeasonDayTypeSchedule" ;
  rdfs:comment "Schedules that use this DayType."@en ;
  owl:inverseOf cim:SeasonDayTypeSchedule.DayType ;
  rdfs:domain cim:DayType ;
  rdfs:isDefinedBy :Package_Standard ;
  rdfs:range cim:SeasonDayTypeSchedule ;
  uml:id "EAID_BB741793_089B_4901_9993_2194B4BE2F75-B" .

cim:Discrete.DiscreteValue a owl:ObjectProperty, owl:InverseFunctionalProperty ;
  rdfs:label "DiscreteValue" ;
  rdfs:comment "The values connected to this measurement."@en ;
  owl:inverseOf cim:DiscreteValue.Discrete ;
  rdfs:domain cim:Discrete ;
  rdfs:isDefinedBy :Package_Standard ;
  rdfs:range cim:DiscreteValue ;
  uml:id "EAID_50254CED_412A_46e7_844E_A91C77FA3D75-B" .

cim:Discrete.ValueAliasSet a owl:ObjectProperty, owl:FunctionalProperty ;
  rdfs:label "ValueAliasSet" ;
  rdfs:comment "The ValueAliasSet used for translation of a MeasurementValue.value to a name."@en ;
  owl:inverseOf cim:ValueAliasSet.Discrete ;
  rdfs:domain cim:Discrete ;
  rdfs:isDefinedBy :Package_Standard ;
  rdfs:range cim:ValueAliasSet ;
  uml:id "EAID_B12363BD_CFEE_4d4c_BA42_F955B39C19FA-A" .

cim:DiscreteValue.Command a owl:ObjectProperty, owl:FunctionalProperty, owl:InverseFunctionalProperty ;
  rdfs:label "Command" ;
  rdfs:comment "The Control variable associated with the MeasurementValue."@en ;
  owl:inverseOf cim:Command.DiscreteValue ;
  rdfs:domain cim:DiscreteValue ;
  rdfs:isDefinedBy :Package_Standard ;
  rdfs:range cim:Command ;
  uml:id "EAID_43AED751_ECB2_4afe_A6AC_63ABFE11AA4A-B" .

cim:DiscreteValue.Discrete a owl:ObjectProperty, owl:FunctionalProperty ;
  rdfs:label "Discrete" ;
  rdfs:comment "Measurement to which this value is connected."@en ;
  owl:inverseOf cim:Discrete.DiscreteValue ;
  rdfs:domain cim:DiscreteValue ;
  rdfs:isDefinedBy :Package_Standard ;
  rdfs:range cim:Discrete ;
  uml:id "EAID_50254CED_412A_46e7_844E_A91C77FA3D75-A" .

cim:EnergyConsumer.EnergyConsumerPhase a owl:ObjectProperty, owl:InverseFunctionalProperty ;
  rdfs:label "EnergyConsumerPhase" ;
  rdfs:comment "The individual phase models for this energy consumer."@en ;
  owl:inverseOf cim:EnergyConsumerPhase.EnergyConsumer ;
  rdfs:domain cim:EnergyConsumer ;
  rdfs:isDefinedBy :Package_Standard ;
  rdfs:range cim:EnergyConsumerPhase ;
  uml:id "EAID_E16E2CF0_B5A8_47e6_AD39_53FD88863F5D-B" .

cim:EnergyConsumerPhase.EnergyConsumer a owl:ObjectProperty, owl:FunctionalProperty ;
  rdfs:label "EnergyConsumer" ;
  rdfs:comment "The energy consumer to which this phase belongs."@en ;
  owl:inverseOf cim:EnergyConsumer.EnergyConsumerPhase ;
  rdfs:domain cim:EnergyConsumerPhase ;
  rdfs:isDefinedBy :Package_Standard ;
  rdfs:range cim:EnergyConsumer ;
  uml:id "EAID_E16E2CF0_B5A8_47e6_AD39_53FD88863F5D-A" .

cim:EnergyConsumerPhase.phase a owl:ObjectProperty, owl:FunctionalProperty ;
  rdfs:label "phase" ;
  rdfs:comment "Phase of this energy consumer component.   If the energy consumer is wye connected, the connection is from the indicated phase to the central ground or neutral point.  If the energy consumer is delta connected, the phase indicates an energy consumer connected from the indicated phase to the next logical non-neutral phase."@en ;
  rdfs:domain cim:EnergyConsumerPhase ;
  rdfs:isDefinedBy :Package_Standard ;
  rdfs:range cim:SinglePhaseKind ;
  uml:hasStereotype uml:attribute ;
  uml:id "EAID_78A031FD_9F48_49c1_B483_D31C5116F28F" .

cim:Equipment.AdditionalEquipmentContainer a owl:ObjectProperty ;
  rdfs:label "AdditionalEquipmentContainer" ;
  rdfs:comment "Additional equipment container beyond the primary equipment container.  The equipment is contained in another equipment container, but also grouped with this equipment container."@en ;
  owl:inverseOf cim:EquipmentContainer.AdditionalGroupedEquipment ;
  rdfs:domain cim:Equipment ;
  rdfs:isDefinedBy :Package_Standard ;
  rdfs:range cim:EquipmentContainer ;
  uml:id "EAID_28BF52BE_C487_4696_860C_3A18E6A59803-B" .

cim:Equipment.EquipmentContainer a owl:ObjectProperty, owl:FunctionalProperty ;
  rdfs:label "EquipmentContainer" ;
  rdfs:comment "Container of this equipment."@en ;
  owl:inverseOf cim:EquipmentContainer.Equipments ;
  rdfs:domain cim:Equipment ;
  rdfs:isDefinedBy :Package_Standard ;
  rdfs:range cim:EquipmentContainer ;
  uml:hasStereotype uml:ofAggregate ;
  uml:id "EAID_C707B922_34B1_473b_B88D_ACA331914E77-A" .

cim:Equipment.OperationalLimitSet a owl:ObjectProperty, owl:InverseFunctionalProperty ;
  rdfs:label "OperationalLimitSet" ;
  rdfs:comment "The operational limit sets associated with this equipment."@en ;
  owl:inverseOf cim:OperationalLimitSet.Equipment ;
  rdfs:domain cim:Equipment ;
  rdfs:isDefinedBy :Package_Standard ;
  rdfs:range cim:OperationalLimitSet ;
  uml:id "EAID_67BC7C1E_A2ED_40ee_AEEA_E917394D2535-B" .

cim:EquipmentContainer.AdditionalGroupedEquipment a owl:ObjectProperty ;
  rdfs:label "AdditionalGroupedEquipment" ;
  rdfs:comment "The additonal contained equipment.  The equipment belong to the equipment container. The equipment is contained in another equipment container, but also grouped with this equipment container.  Examples include when a switch contained in a substation is also desired to be grouped with a line contianer or when a switch is included in a secondary substation and also grouped in a feeder."@en ;
  owl:inverseOf cim:Equipment.AdditionalEquipmentContainer ;
  rdfs:domain cim:EquipmentContainer ;
  rdfs:isDefinedBy :Package_Standard ;
  rdfs:range cim:Equipment ;
  uml:id "EAID_28BF52BE_C487_4696_860C_3A18E6A59803-A" .

cim:EquipmentContainer.Equipments a owl:ObjectProperty, owl:InverseFunctionalProperty ;
  rdfs:label "Equipments" ;
  rdfs:comment "Contained equipment."@en ;
  owl:inverseOf cim:Equipment.EquipmentContainer ;
  rdfs:domain cim:EquipmentContainer ;
  rdfs:isDefinedBy :Package_Standard ;
  rdfs:range cim:Equipment ;
  uml:hasStereotype uml:aggregateOf ;
  uml:id "EAID_C707B922_34B1_473b_B88D_ACA331914E77-B" .

cim:Feeder.NamingSecondarySubstation a owl:ObjectProperty, owl:InverseFunctionalProperty ;
  rdfs:label "NamingSecondarySubstation" ;
  rdfs:comment "The secondary substations that are normally energized from the feeder.  Used for naming purposes.   Should be consistent with the other associations for energizing terminal specification and the feeder energization specification."@en ;
  owl:inverseOf cim:Substation.NamingFeeder ;
  rdfs:domain cim:Feeder ;
  rdfs:isDefinedBy :Package_Standard ;
  rdfs:range cim:Substation ;
  uml:hasStereotype uml:aggregateOf ;
  uml:id "EAID_37B50302_F3BA_41f0_A4CE_108D484CD459-A" .

cim:Feeder.NormalEnergizedSubstation a owl:ObjectProperty ;
  rdfs:label "NormalEnergizedSubstation" ;
  rdfs:comment "The substations that are normally energized by the feeder."@en ;
  owl:inverseOf cim:Substation.NormalEnergizingFeeder ;
  rdfs:domain cim:Feeder ;
  rdfs:isDefinedBy :Package_Standard ;
  rdfs:range cim:Substation ;
  uml:id "EAID_160F8306_5A51_4969_9EC8_1D547FB94B4B-A" .

cim:Feeder.NormalEnergizingSubstation a owl:ObjectProperty, owl:FunctionalProperty ;
  rdfs:label "NormalEnergizingSubstation" ;
  rdfs:comment "The substation that nominally energizes the feeder.  Also used for naming purposes."@en ;
  owl:inverseOf cim:Substation.NormalEnergizedFeeder ;
  rdfs:domain cim:Feeder ;
  rdfs:isDefinedBy :Package_Standard ;
  rdfs:range cim:Substation ;
  uml:hasStereotype uml:ofAggregate ;
  uml:id "EAID_A102BC69_2DBA_498e_AC02_FB647D4A3685-A" .

cim:Feeder.NormalHeadTerminal a owl:ObjectProperty, owl:InverseFunctionalProperty ;
  rdfs:label "NormalHeadTerminal" ;
  rdfs:comment "The normal head terminal or terminals of the feeder."@en ;
  owl:inverseOf cim:Terminal.NormalHeadFeeder ;
  rdfs:domain cim:Feeder ;
  rdfs:isDefinedBy :Package_Standard ;
  rdfs:range cim:Terminal ;
  uml:id "EAID_183D2B47_D1FB_4912_91F1_7BE76ED69922-A" .

cim:GeneratingUnit.RotatingMachine a owl:ObjectProperty, owl:InverseFunctionalProperty ;
  rdfs:label "RotatingMachine" ;
  rdfs:comment "A synchronous machine may operate as a generator and as such becomes a member of a generating unit."@en ;
  owl:inverseOf cim:RotatingMachine.GeneratingUnit ;
  rdfs:domain cim:GeneratingUnit ;
  rdfs:isDefinedBy :Package_Standard ;
  rdfs:range cim:RotatingMachine ;
  uml:id "EAID_A98398C8_727E_4545_9CB7_E1018A0239FB-B" .

cim:HydroGeneratingUnit.HydroPowerPlant a owl:ObjectProperty, owl:FunctionalProperty ;
  rdfs:label "HydroPowerPlant" ;
  rdfs:comment "The hydro generating unit belongs to a hydro power plant."@en ;
  owl:inverseOf cim:HydroPowerPlant.HydroGeneratingUnit ;
  rdfs:domain cim:HydroGeneratingUnit ;
  rdfs:isDefinedBy :Package_Standard ;
  rdfs:range cim:HydroPowerPlant ;
  uml:hasStereotype uml:ofAggregate ;
  uml:id "EAID_58B7CA34_2BDE_4f7a_B931_DF6F1BDB8EE6-A" .

cim:HydroPowerPlant.HydroGeneratingUnit a owl:ObjectProperty, owl:InverseFunctionalProperty ;
  rdfs:label "HydroGeneratingUnit" ;
  rdfs:comment "The hydro generating unit belongs to a hydro power plant."@en ;
  owl:inverseOf cim:HydroGeneratingUnit.HydroPowerPlant ;
  rdfs:domain cim:HydroPowerPlant ;
  rdfs:isDefinedBy :Package_Standard ;
  rdfs:range cim:HydroGeneratingUnit ;
  uml:hasStereotype uml:aggregateOf ;
  uml:id "EAID_58B7CA34_2BDE_4f7a_B931_DF6F1BDB8EE6-B" .

cim:IdentifiedObject.Names a owl:ObjectProperty, owl:InverseFunctionalProperty ;
  rdfs:label "Names" ;
  rdfs:comment "All names of this identified object."@en ;
  owl:inverseOf cim:Name.IdentifiedObject ;
  rdfs:domain cim:IdentifiedObject ;
  rdfs:isDefinedBy :Package_Standard ;
  rdfs:range cim:Name ;
  uml:id "EAID_126F6E28_7A22_49ba_9C3A_9D194B3B900C-A" .

cim:Line.Region a owl:ObjectProperty, owl:FunctionalProperty ;
  rdfs:label "Region" ;
  rdfs:comment "A Line can be contained by a SubGeographical Region."@en ;
  rdfs:domain cim:Line ;
  rdfs:isDefinedBy :Package_Standard ;
  rdfs:range cim:SubGeographicalRegion ;
  uml:hasStereotype uml:ofAggregate ;
  uml:id "EAID_E6517741_2B38_4e6f_A3DA_FA702BE54582-A" .

cim:LoadArea.SubLoadArea a owl:ObjectProperty, owl:InverseFunctionalProperty ;
  rdfs:label "SubLoadArea" ;
  rdfs:comment "The SubLoadAreas in the LoadArea."@en ;
  owl:inverseOf cim:SubLoadArea.LoadArea ;
  rdfs:domain cim:LoadArea ;
  rdfs:isDefinedBy :Package_Standard ;
  rdfs:range cim:SubLoadArea ;
  uml:hasStereotype uml:aggregateOf ;
  uml:id "EAID_B8D3C66D_C590_4302_B444_B8A6633E4AD3-B" .

cim:LoadGroup.SubLoadArea a owl:ObjectProperty, owl:FunctionalProperty ;
  rdfs:label "SubLoadArea" ;
  rdfs:comment "The SubLoadArea where the Loadgroup belongs."@en ;
  owl:inverseOf cim:SubLoadArea.LoadGroup ;
  rdfs:domain cim:LoadGroup ;
  rdfs:isDefinedBy :Package_Standard ;
  rdfs:range cim:SubLoadArea ;
  uml:hasStereotype uml:ofAggregate ;
  uml:id "EAID_0965FD33_7B62_4433_901D_E2C66F2D3034-A" .

cim:Measurement.PowerSystemResource a owl:ObjectProperty, owl:FunctionalProperty ;
  rdfs:label "PowerSystemResource" ;
  rdfs:comment "The power system resource that contains the measurement."@en ;
  owl:inverseOf cim:PowerSystemResource.Measurement ;
  rdfs:domain cim:Measurement ;
  rdfs:isDefinedBy :Package_Standard ;
  rdfs:range cim:PowerSystemResource ;
  uml:hasStereotype uml:ofAggregate ;
  uml:id "EAID_B36CCEA4_2D8B_4ac5_A93A_13224B5BF378-A" .

cim:Measurement.Terminal a owl:ObjectProperty, owl:FunctionalProperty ;
  rdfs:label "Terminal" ;
  rdfs:comment "One or more measurements may be associated with a terminal in the network."@en ;
  owl:inverseOf cim:ACDCTerminal.Measurement ;
  rdfs:domain cim:Measurement ;
  rdfs:isDefinedBy :Package_Standard ;
  rdfs:range cim:ACDCTerminal ;
  uml:id "EAID_952C2E70_618A_4c2b_9D47_C2B175B263DB-A" .

cim:Measurement.phases a owl:ObjectProperty, owl:FunctionalProperty ;
  rdfs:label "phases" ;
  rdfs:comment "Indicates to which phases the measurement applies and avoids the need to use 'measurementType' to also encode phase information (which would explode the types). Since Controls have associations with Measurements, they will have the capability to handle each phase. The phase information in Measurement, along with 'measurementType' and 'phaseConnection' uniquely defines a Measurement for a device, based on normal network phase. Their meaning will not change when the computed energizing phasing is changed due to jumpers or other reasons."@en ;
  rdfs:domain cim:Measurement ;
  rdfs:isDefinedBy :Package_Standard ;
  rdfs:range cim:PhaseCode ;
  uml:hasStereotype uml:attribute ;
  uml:id "EAID_178B74AA_906B_480f_8F55_0D821AA12F64" .

cim:Measurement.unitMultiplier a owl:ObjectProperty, owl:FunctionalProperty ;
  rdfs:label "unitMultiplier" ;
  rdfs:comment "The unit multiplier of the measured quantity."@en ;
  rdfs:domain cim:Measurement ;
  rdfs:isDefinedBy :Package_Standard ;
  rdfs:range cim:UnitMultiplier ;
  uml:hasStereotype uml:attribute ;
  uml:id "EAID_563FF72F_6096_4aa8_AD4F_61BB4CDD90BB" .

cim:Measurement.unitSymbol a owl:ObjectProperty, owl:FunctionalProperty ;
  rdfs:label "unitSymbol" ;
  rdfs:comment "The unit of measure of the measured quantity."@en ;
  rdfs:domain cim:Measurement ;
  rdfs:isDefinedBy :Package_Standard ;
  rdfs:range cim:UnitSymbol ;
  uml:hasStereotype uml:attribute ;
  uml:id "EAID_2404516B_C4F5_475b_ADB6_8F7DC3BA0C00" .

cim:MeasurementValue.MeasurementValueSource a owl:ObjectProperty, owl:FunctionalProperty ;
  rdfs:label "MeasurementValueSource" ;
  rdfs:comment "A reference to the type of source that updates the MeasurementValue, e.g. SCADA, CCLink, manual, etc. User conventions for the names of sources are contained in the introduction to IEC 61970-301."@en ;
  owl:inverseOf cim:MeasurementValueSource.MeasurementValue ;
  rdfs:domain cim:MeasurementValue ;
  rdfs:isDefinedBy :Package_Standard ;
  rdfs:range cim:MeasurementValueSource ;
  uml:id "EAID_A1A6BBC4_66C5_4dba_A0DC_B595A4605752-A" .

cim:MeasurementValueSource.MeasurementValue a owl:ObjectProperty, owl:InverseFunctionalProperty ;
  rdfs:label "MeasurementValue" ;
  rdfs:comment "The MeasurementValues updated by the source."@en ;
  owl:inverseOf cim:MeasurementValue.MeasurementValueSource ;
  rdfs:domain cim:MeasurementValueSource ;
  rdfs:isDefinedBy :Package_Standard ;
  rdfs:range cim:MeasurementValue ;
  uml:id "EAID_A1A6BBC4_66C5_4dba_A0DC_B595A4605752-B" .

cim:Name.IdentifiedObject a owl:ObjectProperty, owl:FunctionalProperty ;
  rdfs:label "IdentifiedObject" ;
  rdfs:comment "Identified object that this name designates."@en ;
  owl:inverseOf cim:IdentifiedObject.Names ;
  rdfs:domain cim:Name ;
  rdfs:isDefinedBy :Package_Standard ;
  rdfs:range cim:IdentifiedObject ;
  uml:id "EAID_126F6E28_7A22_49ba_9C3A_9D194B3B900C-B" .

cim:Name.NameType a owl:ObjectProperty, owl:FunctionalProperty ;
  rdfs:label "NameType" ;
  rdfs:comment "Type of this name."@en ;
  owl:inverseOf cim:NameType.Names ;
  rdfs:domain cim:Name ;
  rdfs:isDefinedBy :Package_Standard ;
  rdfs:range cim:NameType ;
  uml:id "EAID_AB78CB67_D384_4438_914D_9C4A5DC8ACC6-A" .

cim:NameType.NameTypeAuthority a owl:ObjectProperty, owl:FunctionalProperty ;
  rdfs:label "NameTypeAuthority" ;
  rdfs:comment "Authority responsible for managing names of this type."@en ;
  owl:inverseOf cim:NameTypeAuthority.NameTypes ;
  rdfs:domain cim:NameType ;
  rdfs:isDefinedBy :Package_Standard ;
  rdfs:range cim:NameTypeAuthority ;
  uml:id "EAID_CD4BC887_A931_450b_AA2E_C5BFB637AFAE-A" .

cim:NameType.Names a owl:ObjectProperty, owl:InverseFunctionalProperty ;
  rdfs:label "Names" ;
  rdfs:comment "All names of this type."@en ;
  owl:inverseOf cim:Name.NameType ;
  rdfs:domain cim:NameType ;
  rdfs:isDefinedBy :Package_Standard ;
  rdfs:range cim:Name ;
  uml:id "EAID_AB78CB67_D384_4438_914D_9C4A5DC8ACC6-B" .

cim:NameTypeAuthority.NameTypes a owl:ObjectProperty, owl:InverseFunctionalProperty ;
  rdfs:label "NameTypes" ;
  rdfs:comment "All name types managed by this authority."@en ;
  owl:inverseOf cim:NameType.NameTypeAuthority ;
  rdfs:domain cim:NameTypeAuthority ;
  rdfs:isDefinedBy :Package_Standard ;
  rdfs:range cim:NameType ;
  uml:id "EAID_CD4BC887_A931_450b_AA2E_C5BFB637AFAE-B" .

cim:NonConformLoad.LoadGroup a owl:ObjectProperty, owl:FunctionalProperty ;
  rdfs:label "LoadGroup" ;
  rdfs:comment "Group of this ConformLoad."@en ;
  owl:inverseOf cim:NonConformLoadGroup.EnergyConsumer ;
  rdfs:domain cim:NonConformLoad ;
  rdfs:isDefinedBy :Package_Standard ;
  rdfs:range cim:NonConformLoadGroup ;
  uml:id "EAID_FD87E6CD_8C78_4af5_82D5_E3E61AA9436E-A" .

cim:NonConformLoadGroup.EnergyConsumer a owl:ObjectProperty, owl:InverseFunctionalProperty ;
  rdfs:label "EnergyConsumer" ;
  rdfs:comment "Conform loads assigned to this ConformLoadGroup."@en ;
  owl:inverseOf cim:NonConformLoad.LoadGroup ;
  rdfs:domain cim:NonConformLoadGroup ;
  rdfs:isDefinedBy :Package_Standard ;
  rdfs:range cim:NonConformLoad ;
  uml:id "EAID_FD87E6CD_8C78_4af5_82D5_E3E61AA9436E-B" .

cim:NonConformLoadGroup.NonConformLoadSchedule a owl:ObjectProperty, owl:InverseFunctionalProperty ;
  rdfs:label "NonConformLoadSchedule" ;
  rdfs:comment "The NonConformLoadSchedules in the NonConformLoadGroup."@en ;
  owl:inverseOf cim:NonConformLoadSchedule.NonConformLoadGroup ;
  rdfs:domain cim:NonConformLoadGroup ;
  rdfs:isDefinedBy :Package_Standard ;
  rdfs:range cim:NonConformLoadSchedule ;
  uml:hasStereotype uml:aggregateOf ;
  uml:id "EAID_12713C88_D5D2_4431_AB94_618D440450F3-B" .

cim:NonConformLoadSchedule.NonConformLoadGroup a owl:ObjectProperty, owl:FunctionalProperty ;
  rdfs:label "NonConformLoadGroup" ;
  rdfs:comment "The NonConformLoadGroup where the NonConformLoadSchedule belongs."@en ;
  owl:inverseOf cim:NonConformLoadGroup.NonConformLoadSchedule ;
  rdfs:domain cim:NonConformLoadSchedule ;
  rdfs:isDefinedBy :Package_Standard ;
  rdfs:range cim:NonConformLoadGroup ;
  uml:hasStereotype uml:ofAggregate ;
  uml:id "EAID_12713C88_D5D2_4431_AB94_618D440450F3-A" .

cim:OperatingParticipant.OperatingShare a owl:ObjectProperty, owl:InverseFunctionalProperty ;
  rdfs:label "OperatingShare" ;
  rdfs:comment "The operating shares of this operating participant.  An operating participant can be resused for any number of power system resources."@en ;
  owl:inverseOf cim:OperatingShare.OperatingParticipant ;
  rdfs:domain cim:OperatingParticipant ;
  rdfs:isDefinedBy :Package_Standard ;
  rdfs:range cim:OperatingShare ;
  uml:id "EAID_C5F52C68_A596_4f92_9F82_45A71D4C2AFE-B" .

cim:OperatingShare.OperatingParticipant a owl:ObjectProperty, owl:FunctionalProperty ;
  rdfs:label "OperatingParticipant" ;
  rdfs:comment "The operating participant having this share with the associated power system resource."@en ;
  owl:inverseOf cim:OperatingParticipant.OperatingShare ;
  rdfs:domain cim:OperatingShare ;
  rdfs:isDefinedBy :Package_Standard ;
  rdfs:range cim:OperatingParticipant ;
  uml:id "EAID_C5F52C68_A596_4f92_9F82_45A71D4C2AFE-A" .

cim:OperatingShare.PowerSystemResource a owl:ObjectProperty, owl:FunctionalProperty ;
  rdfs:label "PowerSystemResource" ;
  rdfs:comment "The power system resource to which the share applies."@en ;
  owl:inverseOf cim:PowerSystemResource.OperatingShare ;
  rdfs:domain cim:OperatingShare ;
  rdfs:isDefinedBy :Package_Standard ;
  rdfs:range cim:PowerSystemResource ;
  uml:id "EAID_31E43789_BA04_425c_A5AF_A5C88F4DA1F6-A" .

cim:OperatingShare.percentage a owl:ObjectProperty, owl:DatatypeProperty, owl:FunctionalProperty ;
  rdfs:label "percentage" ;
  rdfs:comment "Percentage operational ownership between the pair (power system resource and operatging participant) associated with this share. The total percentage ownership for a power system resource should add to 100%."@en ;
  rdfs:domain cim:OperatingShare ;
  rdfs:isDefinedBy :Package_Standard ;
  rdfs:range cim:PerCent ;
  uml:hasStereotype uml:attribute ;
  uml:id "EAID_F617B4D1_4267_48a9_920D_66D0EB521E7C" .

cim:OperationalLimit.OperationalLimitSet a owl:ObjectProperty, owl:FunctionalProperty ;
  rdfs:label "OperationalLimitSet" ;
  rdfs:comment "The limit set to which the limit values belong."@en ;
  owl:inverseOf cim:OperationalLimitSet.OperationalLimitValue ;
  rdfs:domain cim:OperationalLimit ;
  rdfs:isDefinedBy :Package_Standard ;
  rdfs:range cim:OperationalLimitSet ;
  uml:hasStereotype uml:ofAggregate ;
  uml:id "EAID_518EFAF0_C8D9_43c6_8146_E9ADC3C4831F-A" .

cim:OperationalLimit.OperationalLimitType a owl:ObjectProperty, owl:FunctionalProperty ;
  rdfs:label "OperationalLimitType" ;
  rdfs:comment "The limit type associated with this limit."@en ;
  owl:inverseOf cim:OperationalLimitType.OperationalLimit ;
  rdfs:domain cim:OperationalLimit ;
  rdfs:isDefinedBy :Package_Standard ;
  rdfs:range cim:OperationalLimitType ;
  uml:id "EAID_E8BF274E_6978_4831_B323_CF453AFEC807-A" .

cim:OperationalLimitSet.Equipment a owl:ObjectProperty, owl:FunctionalProperty ;
  rdfs:label "Equipment" ;
  rdfs:comment "The equipment to which the limit set applies."@en ;
  owl:inverseOf cim:Equipment.OperationalLimitSet ;
  rdfs:domain cim:OperationalLimitSet ;
  rdfs:isDefinedBy :Package_Standard ;
  rdfs:range cim:Equipment ;
  uml:id "EAID_67BC7C1E_A2ED_40ee_AEEA_E917394D2535-A" .

cim:OperationalLimitSet.OperationalLimitValue a owl:ObjectProperty, owl:InverseFunctionalProperty ;
  rdfs:label "OperationalLimitValue" ;
  rdfs:comment "Values of equipment limits."@en ;
  owl:inverseOf cim:OperationalLimit.OperationalLimitSet ;
  rdfs:domain cim:OperationalLimitSet ;
  rdfs:isDefinedBy :Package_Standard ;
  rdfs:range cim:OperationalLimit ;
  uml:hasStereotype uml:aggregateOf ;
  uml:id "EAID_518EFAF0_C8D9_43c6_8146_E9ADC3C4831F-B" .

cim:OperationalLimitSet.Terminal a owl:ObjectProperty, owl:FunctionalProperty ;
  rdfs:label "Terminal" ;
  owl:inverseOf cim:ACDCTerminal.OperationalLimitSet ;
  rdfs:domain cim:OperationalLimitSet ;
  rdfs:isDefinedBy :Package_Standard ;
  rdfs:range cim:ACDCTerminal ;
  uml:id "EAID_B879ACB4_5EB0_4709_8236_3964485589CC-A" .

cim:OperationalLimitType.OperationalLimit a owl:ObjectProperty, owl:InverseFunctionalProperty ;
  rdfs:label "OperationalLimit" ;
  rdfs:comment "The operational limits associated with this type of limit."@en ;
  owl:inverseOf cim:OperationalLimit.OperationalLimitType ;
  rdfs:domain cim:OperationalLimitType ;
  rdfs:isDefinedBy :Package_Standard ;
  rdfs:range cim:OperationalLimit ;
  uml:id "EAID_E8BF274E_6978_4831_B323_CF453AFEC807-B" .

cim:OperationalLimitType.acceptableDuration a owl:ObjectProperty, owl:DatatypeProperty, owl:FunctionalProperty ;
  rdfs:label "acceptableDuration" ;
  rdfs:comment "The nominal acceptable duration of the limit.  Limits are commonly expressed in terms of the a time limit for which the limit is normally acceptable.   The actual acceptable duration of a specific limit may depend on other local factors such as temperature or wind speed."@en ;
  rdfs:domain cim:OperationalLimitType ;
  rdfs:isDefinedBy :Package_Standard ;
  rdfs:range cim:Seconds ;
  uml:hasStereotype uml:attribute ;
  uml:id "EAID_04DE1617_94FD_45c4_8EA2_55DC20DD2BD9" .

cim:OperationalLimitType.direction a owl:ObjectProperty, owl:FunctionalProperty ;
  rdfs:label "direction" ;
  rdfs:comment "The direction of the limit."@en ;
  rdfs:domain cim:OperationalLimitType ;
  rdfs:isDefinedBy :Package_Standard ;
  rdfs:range cim:OperationalLimitDirectionKind ;
  uml:hasStereotype uml:attribute ;
  uml:id "EAID_EFE7F681_720E_49aa_91C8_02CFC5BFEE99" .

cim:PSREvent.PowerSystemResource a owl:ObjectProperty, owl:FunctionalProperty ;
  rdfs:label "PowerSystemResource" ;
  rdfs:comment "Power system resource that generated this event."@en ;
  owl:inverseOf cim:PowerSystemResource.PSREvents ;
  rdfs:domain cim:PSREvent ;
  rdfs:isDefinedBy :Package_Standard ;
  rdfs:range cim:PowerSystemResource ;
  uml:id "EAID_B09299BA_63A1_4591_8646_E23594EAC9B2-A" .

cim:PSREvent.kind a owl:ObjectProperty, owl:FunctionalProperty ;
  rdfs:label "kind" ;
  rdfs:comment "Kind of event."@en ;
  rdfs:domain cim:PSREvent ;
  rdfs:isDefinedBy :Package_Standard ;
  rdfs:range cim:PSREventKind ;
  uml:hasStereotype uml:attribute ;
  uml:id "EAID_38E6AEF6_E4EB_441c_9B03_429B7568B645" .

cim:PSRType.PowerSystemResource a owl:ObjectProperty, owl:InverseFunctionalProperty ;
  rdfs:label "PowerSystemResource" ;
  rdfs:comment "Power system resources classified with this power system resource type."@en ;
  owl:inverseOf cim:PowerSystemResource.PSRType ;
  rdfs:domain cim:PSRType ;
  rdfs:isDefinedBy :Package_Standard ;
  rdfs:range cim:PowerSystemResource ;
  uml:id "EAID_BE4215DD_20F7_4077_840E_499D5CA6262A-B" .

cim:PerLengthImpedance.ACLineSegment a owl:ObjectProperty, owl:InverseFunctionalProperty ;
  rdfs:label "ACLineSegment" ;
  rdfs:comment "All line segments described by this per-length impedance."@en ;
  owl:inverseOf cim:ACLineSegment.PerLengthImpedance ;
  rdfs:domain cim:PerLengthImpedance ;
  rdfs:isDefinedBy :Package_Standard ;
  rdfs:range cim:ACLineSegment ;
  uml:id "EAID_BA020DF3_CA9A_4d46_B70E_F7FC12EFBD94-B" .

cim:PowerSystemResource.AssetDatasheet a owl:ObjectProperty, owl:FunctionalProperty ;
  rdfs:label "AssetDatasheet" ;
  rdfs:comment "Datasheet information for this power system resource."@en ;
  owl:inverseOf cim:AssetInfo.PowerSystemResource ;
  rdfs:domain cim:PowerSystemResource ;
  rdfs:isDefinedBy :Package_Standard ;
  rdfs:range cim:AssetInfo ;
  uml:id "EAID_146AFA1E_C3CB_4681_9EBE_B586F18C7410-A" .

cim:PowerSystemResource.Control a owl:ObjectProperty, owl:InverseFunctionalProperty ;
  rdfs:label "Control" ;
  rdfs:comment "The controller outputs used to actually govern a regulating device, e.g. the magnetization of a synchronous machine or capacitor bank breaker actuator."@en ;
  owl:inverseOf cim:Control.PowerSystemResource ;
  rdfs:domain cim:PowerSystemResource ;
  rdfs:isDefinedBy :Package_Standard ;
  rdfs:range cim:Control ;
  uml:id "EAID_DA4BF365_6235_482d_B3A8_9AF7E39CCAE4-B" .

cim:PowerSystemResource.Measurement a owl:ObjectProperty, owl:InverseFunctionalProperty ;
  rdfs:label "Measurement" ;
  rdfs:comment "The measurements associated with this power system resource."@en ;
  owl:inverseOf cim:Measurement.PowerSystemResource ;
  rdfs:domain cim:PowerSystemResource ;
  rdfs:isDefinedBy :Package_Standard ;
  rdfs:range cim:Measurement ;
  uml:hasStereotype uml:aggregateOf ;
  uml:id "EAID_B36CCEA4_2D8B_4ac5_A93A_13224B5BF378-B" .

cim:PowerSystemResource.OperatingShare a owl:ObjectProperty, owl:InverseFunctionalProperty ;
  rdfs:label "OperatingShare" ;
  rdfs:comment "The operating shares of this power system resource."@en ;
  owl:inverseOf cim:OperatingShare.PowerSystemResource ;
  rdfs:domain cim:PowerSystemResource ;
  rdfs:isDefinedBy :Package_Standard ;
  rdfs:range cim:OperatingShare ;
  uml:id "EAID_31E43789_BA04_425c_A5AF_A5C88F4DA1F6-B" .

cim:PowerSystemResource.PSREvents a owl:ObjectProperty, owl:InverseFunctionalProperty ;
  rdfs:label "PSREvents" ;
  rdfs:comment "All events associated with this power system resource."@en ;
  owl:inverseOf cim:PSREvent.PowerSystemResource ;
  rdfs:domain cim:PowerSystemResource ;
  rdfs:isDefinedBy :Package_Standard ;
  rdfs:range cim:PSREvent ;
  uml:id "EAID_B09299BA_63A1_4591_8646_E23594EAC9B2-B" .

cim:PowerSystemResource.PSRType a owl:ObjectProperty, owl:FunctionalProperty ;
  rdfs:label "PSRType" ;
  rdfs:comment "Custom classification for this power system resource."@en ;
  owl:inverseOf cim:PSRType.PowerSystemResource ;
  rdfs:domain cim:PowerSystemResource ;
  rdfs:isDefinedBy :Package_Standard ;
  rdfs:range cim:PSRType ;
  uml:id "EAID_BE4215DD_20F7_4077_840E_499D5CA6262A-A" .

cim:PowerTransformerEnd.PowerTransformer a owl:ObjectProperty, owl:FunctionalProperty ;
  rdfs:label "PowerTransformer" ;
  rdfs:comment "The power transformer of this power transformer end."@en ;
  rdfs:domain cim:PowerTransformerEnd ;
  rdfs:isDefinedBy :Package_Standard ;
  rdfs:range cim:PowerTransformer ;
  uml:id "EAID_EF743CC0_6565_4da8_A194_F1E92A8AD0D5-A" .

cim:ProtectedSwitch.OperatedByProtectionEquipment a owl:ObjectProperty ;
  rdfs:label "OperatedByProtectionEquipment" ;
  rdfs:comment "Protection equipments that operate this ProtectedSwitch."@en ;
  owl:inverseOf cim:ProtectionEquipment.ProtectedSwitches ;
  rdfs:domain cim:ProtectedSwitch ;
  rdfs:isDefinedBy :Package_Standard ;
  rdfs:range cim:ProtectionEquipment ;
  uml:hasStereotype uml:aggregateOf ;
  uml:id "EAID_341A2500_4736_425b_BA27_7A71ADCB3FD2-B" .

cim:ProtectionEquipment.ConductingEquipments a owl:ObjectProperty ;
  rdfs:label "ConductingEquipments" ;
  rdfs:comment "Protection equipment may be used to protect specific conducting equipment."@en ;
  owl:inverseOf cim:ConductingEquipment.ProtectionEquipments ;
  rdfs:domain cim:ProtectionEquipment ;
  rdfs:isDefinedBy :Package_Standard ;
  rdfs:range cim:ConductingEquipment ;
  uml:hasStereotype uml:ofAggregate ;
  uml:id "EAID_8CF444BF_B136_4069_91E7_DB736553CE53-A" .

cim:ProtectionEquipment.ProtectedSwitches a owl:ObjectProperty ;
  rdfs:label "ProtectedSwitches" ;
  rdfs:comment "Protected switches operated by this ProtectionEquipment."@en ;
  owl:inverseOf cim:ProtectedSwitch.OperatedByProtectionEquipment ;
  rdfs:domain cim:ProtectionEquipment ;
  rdfs:isDefinedBy :Package_Standard ;
  rdfs:range cim:ProtectedSwitch ;
  uml:hasStereotype uml:ofAggregate ;
  uml:id "EAID_341A2500_4736_425b_BA27_7A71ADCB3FD2-A" .

cim:RaiseLowerCommand.ValueAliasSet a owl:ObjectProperty, owl:FunctionalProperty ;
  rdfs:label "ValueAliasSet" ;
  rdfs:comment "The ValueAliasSet used for translation of a Control value to a name."@en ;
  owl:inverseOf cim:ValueAliasSet.RaiseLowerCommand ;
  rdfs:domain cim:RaiseLowerCommand ;
  rdfs:isDefinedBy :Package_Standard ;
  rdfs:range cim:ValueAliasSet ;
  uml:id "EAID_21217731_1EB8_4cc7_8C51_4CCA898641E8-A" .

cim:RatioTapChanger.TransformerEnd a owl:ObjectProperty, owl:FunctionalProperty, owl:InverseFunctionalProperty ;
  rdfs:label "TransformerEnd" ;
  rdfs:comment "Transformer end to which this ratio tap changer belongs."@en ;
  owl:inverseOf cim:TransformerEnd.RatioTapChanger ;
  rdfs:domain cim:RatioTapChanger ;
  rdfs:isDefinedBy :Package_Standard ;
  rdfs:range cim:TransformerEnd ;
  uml:id "EAID_E02A7ADA_DD34_4655_AA49_DF2930CA89CE-A" .

cim:RegularIntervalSchedule.TimePoint a owl:ObjectProperty, owl:InverseFunctionalProperty ;
  rdfs:label "TimePoint" ;
  rdfs:comment "The regular interval time point data values that define this schedule."@en ;
  owl:inverseOf cim:RegularTimePoint.IntervalSchedule ;
  rdfs:domain cim:RegularIntervalSchedule ;
  rdfs:isDefinedBy :Package_Standard ;
  rdfs:range cim:RegularTimePoint ;
  uml:hasStereotype uml:aggregateOf ;
  uml:id "EAID_534B5D65_2095_480e_AE8C_9D6F37B3E312-B" .

cim:RegularIntervalSchedule.timeStep a owl:ObjectProperty, owl:DatatypeProperty, owl:FunctionalProperty ;
  rdfs:label "timeStep" ;
  rdfs:comment "The time between each pair of subsequent regular time points in sequence order."@en ;
  rdfs:domain cim:RegularIntervalSchedule ;
  rdfs:isDefinedBy :Package_Standard ;
  rdfs:range cim:Seconds ;
  uml:hasStereotype uml:attribute ;
  uml:id "EAID_E5A4CE0B_D521_4ac3_91F8_3D08107F9B00" .

cim:RegularTimePoint.IntervalSchedule a owl:ObjectProperty, owl:FunctionalProperty ;
  rdfs:label "IntervalSchedule" ;
  rdfs:comment "Regular interval schedule containing this time point."@en ;
  owl:inverseOf cim:RegularIntervalSchedule.TimePoint ;
  rdfs:domain cim:RegularTimePoint ;
  rdfs:isDefinedBy :Package_Standard ;
  rdfs:range cim:RegularIntervalSchedule ;
  uml:hasStereotype uml:ofAggregate ;
  uml:id "EAID_534B5D65_2095_480e_AE8C_9D6F37B3E312-A" .

cim:RegulatingCondEq.RegulatingControl a owl:ObjectProperty, owl:FunctionalProperty ;
  rdfs:label "RegulatingControl" ;
  rdfs:comment "The regulating control scheme in which this equipment participates."@en ;
  owl:inverseOf cim:RegulatingControl.RegulatingCondEq ;
  rdfs:domain cim:RegulatingCondEq ;
  rdfs:isDefinedBy :Package_Standard ;
  rdfs:range cim:RegulatingControl ;
  uml:id "EAID_5B00CD08_1168_475a_9043_4992F2C5B7A6-A" .

cim:RegulatingControl.RegulatingCondEq a owl:ObjectProperty, owl:InverseFunctionalProperty ;
  rdfs:label "RegulatingCondEq" ;
  rdfs:comment "The equipment that participates in this regulating control scheme."@en ;
  owl:inverseOf cim:RegulatingCondEq.RegulatingControl ;
  rdfs:domain cim:RegulatingControl ;
  rdfs:isDefinedBy :Package_Standard ;
  rdfs:range cim:RegulatingCondEq ;
  uml:id "EAID_5B00CD08_1168_475a_9043_4992F2C5B7A6-B" .

cim:RegulatingControl.RegulationSchedule a owl:ObjectProperty, owl:InverseFunctionalProperty ;
  rdfs:label "RegulationSchedule" ;
  rdfs:comment "Schedule for this Regulating regulating control."@en ;
  owl:inverseOf cim:RegulationSchedule.RegulatingControl ;
  rdfs:domain cim:RegulatingControl ;
  rdfs:isDefinedBy :Package_Standard ;
  rdfs:range cim:RegulationSchedule ;
  uml:id "EAID_E0118353_84F2_48ce_844B_6C5E323866CB-B" .

cim:RegulatingControl.Terminal a owl:ObjectProperty, owl:FunctionalProperty ;
  rdfs:label "Terminal" ;
  rdfs:comment "The terminal associated with this regulating control.  The terminal is associated instead of a node, since the terminal could connect into either a topological node (bus in bus-branch model) or a connectivity node (detailed switch model).  Sometimes it is useful to model regulation at a terminal of a bus bar object since the bus bar can be present in both a bus-branch model or a model with switch detail."@en ;
  owl:inverseOf cim:Terminal.RegulatingControl ;
  rdfs:domain cim:RegulatingControl ;
  rdfs:isDefinedBy :Package_Standard ;
  rdfs:range cim:Terminal ;
  uml:id "EAID_72046CD4_3544_4a09_BEE8_6B98D03229A2-A" .

cim:RegulatingControl.mode a owl:ObjectProperty, owl:FunctionalProperty ;
  rdfs:label "mode" ;
  rdfs:comment "The regulating control mode presently available.  This specification allows for determining the kind of regulation without need for obtaining the units from a schedule."@en ;
  rdfs:domain cim:RegulatingControl ;
  rdfs:isDefinedBy :Package_Standard ;
  rdfs:range cim:RegulatingControlModeKind ;
  uml:hasStereotype uml:attribute ;
  uml:id "EAID_141AFFD0_55DF_4243_BA56_514E404A3F34" .

cim:RegulationSchedule.RegulatingControl a owl:ObjectProperty, owl:FunctionalProperty ;
  rdfs:label "RegulatingControl" ;
  rdfs:comment "Regulating controls that have this Schedule."@en ;
  owl:inverseOf cim:RegulatingControl.RegulationSchedule ;
  rdfs:domain cim:RegulationSchedule ;
  rdfs:isDefinedBy :Package_Standard ;
  rdfs:range cim:RegulatingControl ;
  uml:id "EAID_E0118353_84F2_48ce_844B_6C5E323866CB-A" .

cim:RemoteControl.Control a owl:ObjectProperty, owl:FunctionalProperty, owl:InverseFunctionalProperty ;
  rdfs:label "Control" ;
  rdfs:comment "The Control for the RemoteControl point."@en ;
  owl:inverseOf cim:Control.RemoteControl ;
  rdfs:domain cim:RemoteControl ;
  rdfs:isDefinedBy :Package_Standard ;
  rdfs:range cim:Control ;
  uml:id "EAID_B9A6DD8E_EA10_4c56_9AC9_5F4188962209-A" .

cim:RotatingMachine.GeneratingUnit a owl:ObjectProperty, owl:FunctionalProperty ;
  rdfs:label "GeneratingUnit" ;
  rdfs:comment "A synchronous machine may operate as a generator and as such becomes a member of a generating unit."@en ;
  owl:inverseOf cim:GeneratingUnit.RotatingMachine ;
  rdfs:domain cim:RotatingMachine ;
  rdfs:isDefinedBy :Package_Standard ;
  rdfs:range cim:GeneratingUnit ;
  uml:id "EAID_A98398C8_727E_4545_9CB7_E1018A0239FB-A" .

cim:Season.SeasonDayTypeSchedule a owl:ObjectProperty, owl:InverseFunctionalProperty ;
  rdfs:label "SeasonDayTypeSchedule" ;
  rdfs:comment "Schedules that use this Season."@en ;
  owl:inverseOf cim:SeasonDayTypeSchedule.Season ;
  rdfs:domain cim:Season ;
  rdfs:isDefinedBy :Package_Standard ;
  rdfs:range cim:SeasonDayTypeSchedule ;
  uml:id "EAID_4A5CB2B1_FA1B_4d3c_9CCA_0CBF1C92BFB2-B" .

cim:Season.endDate a owl:ObjectProperty, owl:DatatypeProperty, owl:FunctionalProperty ;
  rdfs:label "endDate" ;
  rdfs:comment "Date season ends."@en ;
  rdfs:domain cim:Season ;
  rdfs:isDefinedBy :Package_Standard ;
  rdfs:range cim:MonthDay ;
  uml:hasStereotype uml:attribute ;
  uml:id "EAID_E2C663AF_C230_4811_AE65_55854D976859" .

cim:Season.startDate a owl:ObjectProperty, owl:DatatypeProperty, owl:FunctionalProperty ;
  rdfs:label "startDate" ;
  rdfs:comment "Date season starts."@en ;
  rdfs:domain cim:Season ;
  rdfs:isDefinedBy :Package_Standard ;
  rdfs:range cim:MonthDay ;
  uml:hasStereotype uml:attribute ;
  uml:id "EAID_1D9138C3_B0FF_461f_ABCD_13020646936D" .

cim:SeasonDayTypeSchedule.DayType a owl:ObjectProperty, owl:FunctionalProperty ;
  rdfs:label "DayType" ;
  rdfs:comment "DayType for the Schedule."@en ;
  owl:inverseOf cim:DayType.SeasonDayTypeSchedule ;
  rdfs:domain cim:SeasonDayTypeSchedule ;
  rdfs:isDefinedBy :Package_Standard ;
  rdfs:range cim:DayType ;
  uml:id "EAID_BB741793_089B_4901_9993_2194B4BE2F75-A" .

cim:SeasonDayTypeSchedule.Season a owl:ObjectProperty, owl:FunctionalProperty ;
  rdfs:label "Season" ;
  rdfs:comment "Season for the Schedule."@en ;
  owl:inverseOf cim:Season.SeasonDayTypeSchedule ;
  rdfs:domain cim:SeasonDayTypeSchedule ;
  rdfs:isDefinedBy :Package_Standard ;
  rdfs:range cim:Season ;
  uml:id "EAID_4A5CB2B1_FA1B_4d3c_9CCA_0CBF1C92BFB2-A" .

cim:StreetAddress.streetDetail a owl:ObjectProperty, owl:FunctionalProperty ;
  rdfs:label "streetDetail" ;
  rdfs:comment "Street detail."@en ;
  rdfs:domain cim:StreetAddress ;
  rdfs:isDefinedBy :Package_CompoundTypes ;
  rdfs:range cim:StreetDetail ;
  uml:hasStereotype uml:attribute ;
  uml:id "EAID_FE7C53E0_21C7_42cd_82C0_B199179621BD" .

cim:StreetAddress.townDetail a owl:ObjectProperty, owl:FunctionalProperty ;
  rdfs:label "townDetail" ;
  rdfs:comment "Town detail."@en ;
  rdfs:domain cim:StreetAddress ;
  rdfs:isDefinedBy :Package_CompoundTypes ;
  rdfs:range cim:TownDetail ;
  uml:hasStereotype uml:attribute ;
  uml:id "EAID_3EA71AA6_ED5C_4f67_BCA2_3A6FB26C45AA" .

cim:StringMeasurement.StringMeasurementValue a owl:ObjectProperty, owl:InverseFunctionalProperty ;
  rdfs:label "StringMeasurementValue" ;
  rdfs:comment "The values connected to this measurement."@en ;
  owl:inverseOf cim:StringMeasurementValue.StringMeasurement ;
  rdfs:domain cim:StringMeasurement ;
  rdfs:isDefinedBy :Package_Standard ;
  rdfs:range cim:StringMeasurementValue ;
  uml:id "EAID_6A002C7C_F0E5_4617_9B38_A5A05BC1FFCE-B" .

cim:StringMeasurementValue.StringMeasurement a owl:ObjectProperty, owl:FunctionalProperty ;
  rdfs:label "StringMeasurement" ;
  rdfs:comment "Measurement to which this value is connected."@en ;
  owl:inverseOf cim:StringMeasurement.StringMeasurementValue ;
  rdfs:domain cim:StringMeasurementValue ;
  rdfs:isDefinedBy :Package_Standard ;
  rdfs:range cim:StringMeasurement ;
  uml:id "EAID_6A002C7C_F0E5_4617_9B38_A5A05BC1FFCE-A" .

cim:SubGeographicalRegion.Region a owl:ObjectProperty, owl:FunctionalProperty ;
  rdfs:label "Region" ;
  rdfs:comment "The association is used in the naming hierarchy."@en ;
  rdfs:domain cim:SubGeographicalRegion ;
  rdfs:isDefinedBy :Package_Standard ;
  rdfs:range cim:GeographicalRegion ;
  uml:hasStereotype uml:ofAggregate ;
  uml:id "EAID_468AC0FC_B0BD_4db9_B8A5_0ABB20ACFACE-A" .

cim:SubLoadArea.LoadArea a owl:ObjectProperty, owl:FunctionalProperty ;
  rdfs:label "LoadArea" ;
  rdfs:comment "The LoadArea where the SubLoadArea belongs."@en ;
  owl:inverseOf cim:LoadArea.SubLoadArea ;
  rdfs:domain cim:SubLoadArea ;
  rdfs:isDefinedBy :Package_Standard ;
  rdfs:range cim:LoadArea ;
  uml:hasStereotype uml:ofAggregate ;
  uml:id "EAID_B8D3C66D_C590_4302_B444_B8A6633E4AD3-A" .

cim:SubLoadArea.LoadGroup a owl:ObjectProperty, owl:InverseFunctionalProperty ;
  rdfs:label "LoadGroup" ;
  rdfs:comment "The Loadgroups in the SubLoadArea."@en ;
  owl:inverseOf cim:LoadGroup.SubLoadArea ;
  rdfs:domain cim:SubLoadArea ;
  rdfs:isDefinedBy :Package_Standard ;
  rdfs:range cim:LoadGroup ;
  uml:hasStereotype uml:aggregateOf ;
  uml:id "EAID_0965FD33_7B62_4433_901D_E2C66F2D3034-B" .

cim:Substation.NamingFeeder a owl:ObjectProperty, owl:FunctionalProperty ;
  rdfs:label "NamingFeeder" ;
  rdfs:comment "The primary feeder that normally energizes the secondary substation. Used for naming purposes.  Either this association or the substation to subgeographical region should be used for hiearchical containment specification."@en ;
  owl:inverseOf cim:Feeder.NamingSecondarySubstation ;
  rdfs:domain cim:Substation ;
  rdfs:isDefinedBy :Package_Standard ;
  rdfs:range cim:Feeder ;
  uml:hasStereotype uml:ofAggregate ;
  uml:id "EAID_37B50302_F3BA_41f0_A4CE_108D484CD459-B" .

cim:Substation.NormalEnergizedFeeder a owl:ObjectProperty, owl:InverseFunctionalProperty ;
  rdfs:label "NormalEnergizedFeeder" ;
  rdfs:comment "The normal energized feeders of the substation. Also used for naming purposes."@en ;
  owl:inverseOf cim:Feeder.NormalEnergizingSubstation ;
  rdfs:domain cim:Substation ;
  rdfs:isDefinedBy :Package_Standard ;
  rdfs:range cim:Feeder ;
  uml:hasStereotype uml:aggregateOf ;
  uml:id "EAID_A102BC69_2DBA_498e_AC02_FB647D4A3685-B" .

cim:Substation.NormalEnergizingFeeder a owl:ObjectProperty ;
  rdfs:label "NormalEnergizingFeeder" ;
  rdfs:comment "The feeders that potentially energize  the downstream substation.  Should be consistent with the associations that describe the naming hiearchy."@en ;
  owl:inverseOf cim:Feeder.NormalEnergizedSubstation ;
  rdfs:domain cim:Substation ;
  rdfs:isDefinedBy :Package_Standard ;
  rdfs:range cim:Feeder ;
  uml:id "EAID_160F8306_5A51_4969_9EC8_1D547FB94B4B-B" .

cim:Substation.Region a owl:ObjectProperty, owl:FunctionalProperty ;
  rdfs:label "Region" ;
  rdfs:comment "The association is used in the naming hierarchy."@en ;
  rdfs:domain cim:Substation ;
  rdfs:isDefinedBy :Package_Standard ;
  rdfs:range cim:SubGeographicalRegion ;
  uml:hasStereotype uml:ofAggregate ;
  uml:id "EAID_26441E52_5302_476f_A82E_8EDD2DF85F26-A" .

cim:Switch.SwitchSchedule a owl:ObjectProperty, owl:InverseFunctionalProperty ;
  rdfs:label "SwitchSchedule" ;
  rdfs:comment "A Switch can be associated with SwitchSchedules."@en ;
  owl:inverseOf cim:SwitchSchedule.Switch ;
  rdfs:domain cim:Switch ;
  rdfs:isDefinedBy :Package_Standard ;
  rdfs:range cim:SwitchSchedule ;
  uml:id "EAID_AF97159E_7B5F_4769_9FCC_57D5C8583077-B" .

cim:SwitchSchedule.Switch a owl:ObjectProperty, owl:FunctionalProperty ;
  rdfs:label "Switch" ;
  rdfs:comment "A SwitchSchedule is associated with a Switch."@en ;
  owl:inverseOf cim:Switch.SwitchSchedule ;
  rdfs:domain cim:SwitchSchedule ;
  rdfs:isDefinedBy :Package_Standard ;
  rdfs:range cim:Switch ;
  uml:id "EAID_AF97159E_7B5F_4769_9FCC_57D5C8583077-A" .

cim:TapChanger.TapChangerControl a owl:ObjectProperty, owl:FunctionalProperty ;
  rdfs:label "TapChangerControl" ;
  rdfs:comment "The regulating control scheme in which this tap changer participates."@en ;
  owl:inverseOf cim:TapChangerControl.TapChanger ;
  rdfs:domain cim:TapChanger ;
  rdfs:isDefinedBy :Package_Standard ;
  rdfs:range cim:TapChangerControl ;
  uml:id "EAID_13466F8F_9089_4836_ACE6_26E562BB6028-A" .

cim:TapChanger.TapSchedule a owl:ObjectProperty, owl:InverseFunctionalProperty ;
  rdfs:label "TapSchedule" ;
  rdfs:comment "A TapChanger can have TapSchedules."@en ;
  owl:inverseOf cim:TapSchedule.TapChanger ;
  rdfs:domain cim:TapChanger ;
  rdfs:isDefinedBy :Package_Standard ;
  rdfs:range cim:TapSchedule ;
  uml:id "EAID_4CC1A90B_7D34_49f7_ACB3_830EAF09C396-B" .

cim:TapChangerControl.TapChanger a owl:ObjectProperty, owl:InverseFunctionalProperty ;
  rdfs:label "TapChanger" ;
  rdfs:comment "The tap changers that participates in this regulating tap control scheme."@en ;
  owl:inverseOf cim:TapChanger.TapChangerControl ;
  rdfs:domain cim:TapChangerControl ;
  rdfs:isDefinedBy :Package_Standard ;
  rdfs:range cim:TapChanger ;
  uml:id "EAID_13466F8F_9089_4836_ACE6_26E562BB6028-B" .

cim:TapSchedule.TapChanger a owl:ObjectProperty, owl:FunctionalProperty ;
  rdfs:label "TapChanger" ;
  rdfs:comment "A TapSchedule is associated with a TapChanger."@en ;
  owl:inverseOf cim:TapChanger.TapSchedule ;
  rdfs:domain cim:TapSchedule ;
  rdfs:isDefinedBy :Package_Standard ;
  rdfs:range cim:TapChanger ;
  uml:id "EAID_4CC1A90B_7D34_49f7_ACB3_830EAF09C396-A" .

cim:Terminal.AuxiliaryEquipment a owl:ObjectProperty, owl:InverseFunctionalProperty ;
  rdfs:label "AuxiliaryEquipment" ;
  rdfs:comment "The auxiliary equipment connected to the terminal."@en ;
  owl:inverseOf cim:AuxiliaryEquipment.Terminal ;
  rdfs:domain cim:Terminal ;
  rdfs:isDefinedBy :Package_Standard ;
  rdfs:range cim:AuxiliaryEquipment ;
  uml:id "EAID_3CC8CF1D_CF6F_4b11_89E9_C843D6C7581B-B" .

cim:Terminal.ConductingEquipment a owl:ObjectProperty, owl:FunctionalProperty ;
  rdfs:label "ConductingEquipment" ;
  rdfs:comment "The conducting equipment of the terminal.  Conducting equipment have  terminals that may be connected to other conducting equipment terminals via connectivity nodes or topological nodes."@en ;
  owl:inverseOf cim:ConductingEquipment.Terminal ;
  rdfs:domain cim:Terminal ;
  rdfs:isDefinedBy :Package_Standard ;
  rdfs:range cim:ConductingEquipment ;
  uml:id "EAID_64D6B527_CC81_4f6a_BAB9_22FC5E218F34-A" .

cim:Terminal.ConnectivityNode a owl:ObjectProperty, owl:FunctionalProperty ;
  rdfs:label "ConnectivityNode" ;
  rdfs:comment "The connectivity node to which this terminal connects with zero impedance."@en ;
  owl:inverseOf cim:ConnectivityNode.Terminal ;
  rdfs:domain cim:Terminal ;
  rdfs:isDefinedBy :Package_Standard ;
  rdfs:range cim:ConnectivityNode ;
  uml:id "EAID_FA200B53_A524_49d4_AA56_BE2DFC130DAC-A" .

cim:Terminal.NormalHeadFeeder a owl:ObjectProperty, owl:FunctionalProperty ;
  rdfs:label "NormalHeadFeeder" ;
  rdfs:comment "The feeder that this terminal normally feeds.  Only specifed for the terminals at head of feeders."@en ;
  owl:inverseOf cim:Feeder.NormalHeadTerminal ;
  rdfs:domain cim:Terminal ;
  rdfs:isDefinedBy :Package_Standard ;
  rdfs:range cim:Feeder ;
  uml:id "EAID_183D2B47_D1FB_4912_91F1_7BE76ED69922-B" .

cim:Terminal.RegulatingControl a owl:ObjectProperty, owl:InverseFunctionalProperty ;
  rdfs:label "RegulatingControl" ;
  rdfs:comment "The controls regulating this terminal."@en ;
  owl:inverseOf cim:RegulatingControl.Terminal ;
  rdfs:domain cim:Terminal ;
  rdfs:isDefinedBy :Package_Standard ;
  rdfs:range cim:RegulatingControl ;
  uml:id "EAID_72046CD4_3544_4a09_BEE8_6B98D03229A2-B" .

cim:Terminal.TransformerEnd a owl:ObjectProperty, owl:InverseFunctionalProperty ;
  rdfs:label "TransformerEnd" ;
  rdfs:comment "All transformer ends connected at this terminal."@en ;
  owl:inverseOf cim:TransformerEnd.Terminal ;
  rdfs:domain cim:Terminal ;
  rdfs:isDefinedBy :Package_Standard ;
  rdfs:range cim:TransformerEnd ;
  uml:id "EAID_5107683E_AA98_49db_85EB_62A3B02BC77A-B" .

cim:Terminal.phases a owl:ObjectProperty, owl:FunctionalProperty ;
  rdfs:label "phases" ;
  rdfs:comment "Represents the normal network phasing condition."@en ;
  rdfs:domain cim:Terminal ;
  rdfs:isDefinedBy :Package_Standard ;
  rdfs:range cim:PhaseCode ;
  uml:hasStereotype uml:attribute ;
  uml:id "EAID_F8EADB7F_1BF5_48c5_9EF4_E5B0BBFB65B8" .

cim:TransformerEnd.BaseVoltage a owl:ObjectProperty, owl:FunctionalProperty ;
  rdfs:label "BaseVoltage" ;
  rdfs:comment "Base voltage of the transformer end.  This is essential for PU calculation."@en ;
  rdfs:domain cim:TransformerEnd ;
  rdfs:isDefinedBy :Package_Standard ;
  rdfs:range cim:BaseVoltage ;
  uml:id "EAID_9929932B_ED6E_40a7_B20D_B6F139922CA3-A" .

cim:TransformerEnd.RatioTapChanger a owl:ObjectProperty, owl:FunctionalProperty, owl:InverseFunctionalProperty ;
  rdfs:label "RatioTapChanger" ;
  rdfs:comment "Ratio tap changer associated with this transformer end."@en ;
  owl:inverseOf cim:RatioTapChanger.TransformerEnd ;
  rdfs:domain cim:TransformerEnd ;
  rdfs:isDefinedBy :Package_Standard ;
  rdfs:range cim:RatioTapChanger ;
  uml:id "EAID_E02A7ADA_DD34_4655_AA49_DF2930CA89CE-B" .

cim:TransformerEnd.Terminal a owl:ObjectProperty, owl:FunctionalProperty ;
  rdfs:label "Terminal" ;
  rdfs:comment "Terminal of the power transformer to which this transformer end belongs."@en ;
  owl:inverseOf cim:Terminal.TransformerEnd ;
  rdfs:domain cim:TransformerEnd ;
  rdfs:isDefinedBy :Package_Standard ;
  rdfs:range cim:Terminal ;
  uml:id "EAID_5107683E_AA98_49db_85EB_62A3B02BC77A-A" .

cim:ValueAliasSet.Command a owl:ObjectProperty, owl:InverseFunctionalProperty ;
  rdfs:label "Command" ;
  rdfs:comment "The Commands using the set for translation."@en ;
  owl:inverseOf cim:Command.ValueAliasSet ;
  rdfs:domain cim:ValueAliasSet ;
  rdfs:isDefinedBy :Package_Standard ;
  rdfs:range cim:Command ;
  uml:id "EAID_944A3138_E14B_487b_9B2D_A249CF9BC5FD-B" .

cim:ValueAliasSet.Discrete a owl:ObjectProperty, owl:InverseFunctionalProperty ;
  rdfs:label "Discrete" ;
  rdfs:comment "The Measurements using the set for translation."@en ;
  owl:inverseOf cim:Discrete.ValueAliasSet ;
  rdfs:domain cim:ValueAliasSet ;
  rdfs:isDefinedBy :Package_Standard ;
  rdfs:range cim:Discrete ;
  uml:id "EAID_B12363BD_CFEE_4d4c_BA42_F955B39C19FA-B" .

cim:ValueAliasSet.RaiseLowerCommand a owl:ObjectProperty, owl:InverseFunctionalProperty ;
  rdfs:label "RaiseLowerCommand" ;
  rdfs:comment "The Commands using the set for translation."@en ;
  owl:inverseOf cim:RaiseLowerCommand.ValueAliasSet ;
  rdfs:domain cim:ValueAliasSet ;
  rdfs:isDefinedBy :Package_Standard ;
  rdfs:range cim:RaiseLowerCommand ;
  uml:id "EAID_21217731_1EB8_4cc7_8C51_4CCA898641E8-B" .

cim:ValueAliasSet.Values a owl:ObjectProperty, owl:InverseFunctionalProperty ;
  rdfs:label "Values" ;
  rdfs:comment "The ValueToAlias mappings included in the set."@en ;
  owl:inverseOf cim:ValueToAlias.ValueAliasSet ;
  rdfs:domain cim:ValueAliasSet ;
  rdfs:isDefinedBy :Package_Standard ;
  rdfs:range cim:ValueToAlias ;
  uml:hasStereotype uml:aggregateOf ;
  uml:id "EAID_1F6C4422_46E6_4353_BEF8_E5FBA1605601-A" .

cim:ValueToAlias.ValueAliasSet a owl:ObjectProperty, owl:FunctionalProperty ;
  rdfs:label "ValueAliasSet" ;
  rdfs:comment "The ValueAliasSet having the ValueToAlias mappings."@en ;
  owl:inverseOf cim:ValueAliasSet.Values ;
  rdfs:domain cim:ValueToAlias ;
  rdfs:isDefinedBy :Package_Standard ;
  rdfs:range cim:ValueAliasSet ;
  uml:hasStereotype uml:ofAggregate ;
  uml:id "EAID_1F6C4422_46E6_4353_BEF8_E5FBA1605601-B" .

cim:VoltageLevel.BaseVoltage a owl:ObjectProperty, owl:FunctionalProperty ;
  rdfs:label "BaseVoltage" ;
  rdfs:comment "The base voltage used for all equipment within the voltage level."@en ;
  owl:inverseOf cim:BaseVoltage.VoltageLevel ;
  rdfs:domain cim:VoltageLevel ;
  rdfs:isDefinedBy :Package_Standard ;
  rdfs:range cim:BaseVoltage ;
  uml:id "EAID_B6CD04E3_BF6F_4e11_9354_61425EDE1CAD-A" .

cim:VoltageLevel.Substation a owl:ObjectProperty, owl:FunctionalProperty ;
  rdfs:label "Substation" ;
  rdfs:comment "The association is used in the naming hierarchy."@en ;
  rdfs:domain cim:VoltageLevel ;
  rdfs:isDefinedBy :Package_Standard ;
  rdfs:range cim:Substation ;
  uml:hasStereotype uml:ofAggregate ;
  uml:id "EAID_8DD934CF_30CB_4556_ABA9_7F28B452AB0E-A" .

cim:VoltageLimit.value a owl:ObjectProperty, owl:DatatypeProperty, owl:FunctionalProperty ;
  rdfs:label "value" ;
  rdfs:comment "Limit on voltage. High or low limit nature of the limit depends upon the properties of the operational limit type."@en ;
  rdfs:domain cim:VoltageLimit ;
  rdfs:isDefinedBy :Package_Standard ;
  rdfs:range cim:Voltage ;
  uml:hasStereotype uml:attribute ;
  uml:id "EAID_C7EC0364_B3BC_4ccc_BDD8_9EE2656E6ABA" .

cim:WindGeneratingUnit.windGenUnitType a owl:ObjectProperty, owl:FunctionalProperty ;
  rdfs:label "windGenUnitType" ;
  rdfs:comment "The kind of wind generating unit"@en ;
  rdfs:domain cim:WindGeneratingUnit ;
  rdfs:isDefinedBy :Package_Standard ;
  rdfs:range cim:WindGenUnitKind ;
  uml:hasStereotype uml:attribute ;
  uml:id "EAID_6017AF33_9696_46ee_9192_76C2FAC36ADE" .

entsoe:ENTSOEOperationalLimitType.limitType a owl:ObjectProperty, owl:FunctionalProperty ;
  rdfs:label "limitType" ;
  rdfs:comment "Types of limits defined in the ENTSO-E Operational Handbook Policy 3."@en ;
  rdfs:domain entsoe:ENTSOEOperationalLimitType ;
  rdfs:isDefinedBy :Package_EntsoeExtensions ;
  rdfs:range entsoe:LimitTypeKind ;
  uml:hasStereotype uml:attribute, uml:entsoe ;
  uml:id "EAID_6BFC4669_7814_444e_B240_AD6D46F141EC" .

md:DifferenceModel.forwardDifferences a owl:ObjectProperty, owl:FunctionalProperty ;
  rdfs:label "forwardDifferences" ;
  rdfs:domain md:DifferenceModel ;
  rdfs:isDefinedBy :Package_ModelDescription ;
  rdfs:range md:Statements ;
  uml:id "EAID_4F33C8FB_FF1D_42aa_918E_407C825CC412-B" .

md:DifferenceModel.reverseDifferences a owl:ObjectProperty, owl:FunctionalProperty ;
  rdfs:label "reverseDifferences" ;
  rdfs:domain md:DifferenceModel ;
  rdfs:isDefinedBy :Package_ModelDescription ;
  rdfs:range md:Statements ;
  uml:id "EAID_84439CAF_AF31_4da5_9D0F_EA6311EF9054-B" .

md:Model.DependentOn a owl:ObjectProperty ;
  rdfs:label "DependentOn" ;
  owl:inverseOf md:Model.Depending ;
  rdfs:domain md:Model ;
  rdfs:isDefinedBy :Package_ModelDescription ;
  rdfs:range md:Model ;
  uml:id "EAID_151476FC_7E20_41d2_AE3F_224B91D88006-B" .

md:Model.Depending a owl:ObjectProperty ;
  rdfs:label "Depending" ;
  owl:inverseOf md:Model.DependentOn ;
  rdfs:domain md:Model ;
  rdfs:isDefinedBy :Package_ModelDescription ;
  rdfs:range md:Model ;
  uml:id "EAID_151476FC_7E20_41d2_AE3F_224B91D88006-A" .

md:Model.SupersededBy a owl:ObjectProperty ;
  rdfs:label "SupersededBy" ;
  owl:inverseOf md:Model.Supersedes ;
  rdfs:domain md:Model ;
  rdfs:isDefinedBy :Package_ModelDescription ;
  rdfs:range md:Model ;
  uml:id "EAID_DDBEB57C_03E6_4aab_B8A4_E5A2E2C2E3CF-A" .

md:Model.Supersedes a owl:ObjectProperty ;
  rdfs:label "Supersedes" ;
  owl:inverseOf md:Model.SupersededBy ;
  rdfs:domain md:Model ;
  rdfs:isDefinedBy :Package_ModelDescription ;
  rdfs:range md:Model ;
  uml:id "EAID_DDBEB57C_03E6_4aab_B8A4_E5A2E2C2E3CF-B" .

md:Model.modelingAuthoritySet a owl:ObjectProperty, owl:DatatypeProperty, owl:FunctionalProperty ;
  rdfs:label "modelingAuthoritySet" ;
  rdfs:domain md:Model ;
  rdfs:isDefinedBy :Package_ModelDescription ;
  rdfs:range :URI ;
  uml:hasStereotype uml:attribute ;
  uml:id "EAID_933B0F39_959D_4fe4_B6EF_D25BF8CDA8CC" .

md:Model.profile a owl:ObjectProperty, owl:DatatypeProperty, owl:FunctionalProperty ;
  rdfs:label "profile" ;
  rdfs:domain md:Model ;
  rdfs:isDefinedBy :Package_ModelDescription ;
  rdfs:range :URI ;
  uml:hasStereotype uml:attribute ;
  uml:id "EAID_5FC10413_4CB8_4041_A5C5_39DBCE569A80" .

next2:EquipmentContainerEx.WeatherStation a owl:ObjectProperty ;
  rdfs:label "WeatherStation" ;
  owl:inverseOf next2:WeatherStation.EquipmentContainer ;
  rdfs:domain next2:EquipmentContainerEx ;
  rdfs:isDefinedBy :Package_CIMExtensions ;
  rdfs:range next3:WeatherStation ;
  uml:id "EAID_BA03E565_ACBD_451e_A7A9_63A407A73E3F-B" .

next2:WeatherStation.EquipmentContainer a owl:ObjectProperty ;
  rdfs:label "EquipmentContainer" ;
  owl:inverseOf next2:EquipmentContainerEx.WeatherStation ;
  rdfs:domain next3:WeatherStation ;
  rdfs:isDefinedBy :Package_CIMExtensions ;
  rdfs:range next2:EquipmentContainerEx ;
  uml:id "EAID_BA03E565_ACBD_451e_A7A9_63A407A73E3F-A" .

:PowerSystemProjectSchedule.actualEnd a owl:DatatypeProperty, owl:FunctionalProperty ;
  rdfs:label "actualEnd" ;
  rdfs:comment "Actual date and time for when the project is commissioned and committed to the network model."@en ;
  rdfs:domain :PowerSystemProjectSchedule ;
  rdfs:isDefinedBy :Package_PowerSystemProject ;
  rdfs:range xsd:dateTime ;
  uml:hasStereotype uml:attribute ;
  uml:id "EAID_33C0A687_BB3C_4e0b_B2B3_82D4C137641B" .

:PowerSystemProjectSchedule.actualStart a owl:DatatypeProperty, owl:FunctionalProperty ;
  rdfs:label "actualStart" ;
  rdfs:comment "Actual date and time for when the project is commissioned and committed to the network model."@en ;
  rdfs:domain :PowerSystemProjectSchedule ;
  rdfs:isDefinedBy :Package_PowerSystemProject ;
  rdfs:range xsd:dateTime ;
  uml:hasStereotype uml:attribute ;
  uml:id "EAID_4EDBCAA8_AF79_4b4c_B36A_B3003FC9689D" .

:PowerSystemProjectSchedule.scheduledEnd a owl:DatatypeProperty, owl:FunctionalProperty ;
  rdfs:label "scheduledEnd" ;
  rdfs:comment "Estimated date and time for when the project will be commissioned and committed to the network model."@en ;
  rdfs:domain :PowerSystemProjectSchedule ;
  rdfs:isDefinedBy :Package_PowerSystemProject ;
  rdfs:range xsd:dateTime ;
  uml:hasStereotype uml:attribute ;
  uml:id "EAID_62039392_12EC_47c9_AC63_22F9A0CEA639" .

:PowerSystemProjectSchedule.scheduledStart a owl:DatatypeProperty, owl:FunctionalProperty ;
  rdfs:label "scheduledStart" ;
  rdfs:comment "Estimated date and time for when the project will be commissioned and committed to the network model."@en ;
  rdfs:domain :PowerSystemProjectSchedule ;
  rdfs:isDefinedBy :Package_PowerSystemProject ;
  rdfs:range xsd:dateTime ;
  uml:hasStereotype uml:attribute ;
  uml:id "EAID_60AFA573_DE21_4205_A33F_0FF74871E407" .

:ProjectStep.actualEnd a owl:DatatypeProperty, owl:FunctionalProperty ;
  rdfs:label "actualEnd" ;
  rdfs:comment "Actual date and time for when the project is commissioned and committed to the network model."@en ;
  rdfs:domain :ProjectStep ;
  rdfs:isDefinedBy :Package_PowerSystemProject ;
  rdfs:range xsd:dateTime ;
  uml:hasStereotype uml:attribute ;
  uml:id "EAID_EC8B0A80_0258_479a_9B0D_F35BBCFDE375" .

:ProjectStep.actualStart a owl:DatatypeProperty, owl:FunctionalProperty ;
  rdfs:label "actualStart" ;
  rdfs:comment "Actual date and time for when the project is commissioned and committed to the network model."@en ;
  rdfs:domain :ProjectStep ;
  rdfs:isDefinedBy :Package_PowerSystemProject ;
  rdfs:range xsd:dateTime ;
  uml:hasStereotype uml:attribute ;
  uml:id "EAID_DBF1A91C_4DE8_4424_A85C_B910C938A7C7" .

:ProjectStep.scheduledEnd a owl:DatatypeProperty, owl:FunctionalProperty ;
  rdfs:label "scheduledEnd" ;
  rdfs:comment "Estimated date and time for when the project will be commissioned and committed to the network model."@en ;
  rdfs:domain :ProjectStep ;
  rdfs:isDefinedBy :Package_PowerSystemProject ;
  rdfs:range xsd:dateTime ;
  uml:hasStereotype uml:attribute ;
  uml:id "EAID_F82A3F17_7783_4cde_8D47_EE8AF38A6BF6" .

:ProjectStep.scheduledStart a owl:DatatypeProperty, owl:FunctionalProperty ;
  rdfs:label "scheduledStart" ;
  rdfs:comment "Estimated date and time for when the project will be commissioned and committed to the network model."@en ;
  rdfs:domain :ProjectStep ;
  rdfs:isDefinedBy :Package_PowerSystemProject ;
  rdfs:range xsd:dateTime ;
  uml:hasStereotype uml:attribute ;
  uml:id "EAID_F7E1A2ED_891A_4649_9389_B2BA5C2B4AC9" .

cim:ACDCTerminal.sequenceNumber a owl:DatatypeProperty, owl:FunctionalProperty ;
  rdfs:label "sequenceNumber" ;
  rdfs:comment "The orientation of the terminal connections for a multiple terminal conducting equipment.  The sequence numbering starts with 1 and additional terminals should follow in increasing order.   The first terminal is the \"starting point\" for a two terminal branch."@en ;
  rdfs:domain cim:ACDCTerminal ;
  rdfs:isDefinedBy :Package_Standard ;
  rdfs:range xsd:integer ;
  uml:hasStereotype uml:attribute ;
  uml:id "EAID_80113DD8_FC93_471f_911E_C156CCC35865" .

cim:AccumulatorLimit.value a owl:DatatypeProperty, owl:FunctionalProperty ;
  rdfs:label "value" ;
  rdfs:comment "The value to supervise against. The value is positive."@en ;
  rdfs:domain cim:AccumulatorLimit ;
  rdfs:isDefinedBy :Package_Standard ;
  rdfs:range xsd:integer ;
  uml:hasStereotype uml:attribute ;
  uml:id "EAID_2766BE90_05DB_4af9_BFDA_0A4869DF248E" .

cim:AccumulatorValue.value a owl:DatatypeProperty, owl:FunctionalProperty ;
  rdfs:label "value" ;
  rdfs:comment "The value to supervise. The value is positive."@en ;
  rdfs:domain cim:AccumulatorValue ;
  rdfs:isDefinedBy :Package_Standard ;
  rdfs:range xsd:integer ;
  uml:hasStereotype uml:attribute ;
  uml:id "EAID_72155120_CC38_46c0_91C6_595EFD59BEF1" .

cim:Analog.maxValue a owl:DatatypeProperty, owl:FunctionalProperty ;
  rdfs:label "maxValue" ;
  rdfs:comment "Normal value range maximum for any of the MeasurementValue.values. Used for scaling, e.g. in bar graphs or of telemetered raw values."@en ;
  rdfs:domain cim:Analog ;
  rdfs:isDefinedBy :Package_Standard ;
  rdfs:range xsd:float ;
  uml:hasStereotype uml:attribute ;
  uml:id "EAID_28D31F85_9916_4f3f_9D94_569B1CEDF806" .

cim:Analog.minValue a owl:DatatypeProperty, owl:FunctionalProperty ;
  rdfs:label "minValue" ;
  rdfs:comment "Normal value range minimum for any of the MeasurementValue.values. Used for scaling, e.g. in bar graphs or of telemetered raw values"@en ;
  rdfs:domain cim:Analog ;
  rdfs:isDefinedBy :Package_Standard ;
  rdfs:range xsd:float ;
  uml:hasStereotype uml:attribute ;
  uml:id "EAID_82F5E19B_DA8F_4f84_8012_4C4C1B36F374" .

cim:Analog.normalValue a owl:DatatypeProperty, owl:FunctionalProperty ;
  rdfs:label "normalValue" ;
  rdfs:comment "Normal measurement value, e.g., used for percentage calculations."@en ;
  rdfs:domain cim:Analog ;
  rdfs:isDefinedBy :Package_Standard ;
  rdfs:range xsd:float ;
  uml:hasStereotype uml:attribute ;
  uml:id "EAID_A26D95FC_DC0B_4402_BD97_67899BB7E598" .

cim:Analog.positiveFlowIn a owl:DatatypeProperty, owl:FunctionalProperty ;
  rdfs:label "positiveFlowIn" ;
  rdfs:comment "If true then this measurement is an active power, reactive power or current with the convention that a positive value measured at the Terminal means power is flowing into the related PowerSystemResource."@en ;
  rdfs:domain cim:Analog ;
  rdfs:isDefinedBy :Package_Standard ;
  rdfs:range xsd:boolean ;
  uml:hasStereotype uml:attribute ;
  uml:id "EAID_129C96B7_C3AA_477b_975D_448B75A28C32" .

cim:AnalogControl.maxValue a owl:DatatypeProperty, owl:FunctionalProperty ;
  rdfs:label "maxValue" ;
  rdfs:comment "Normal value range maximum for any of the Control.value. Used for scaling, e.g. in bar graphs."@en ;
  rdfs:domain cim:AnalogControl ;
  rdfs:isDefinedBy :Package_Standard ;
  rdfs:range xsd:float ;
  uml:hasStereotype uml:attribute ;
  uml:id "EAID_E2D62846_089B_4e23_AA11_F94CA4D37E9D" .

cim:AnalogControl.minValue a owl:DatatypeProperty, owl:FunctionalProperty ;
  rdfs:label "minValue" ;
  rdfs:comment "Normal value range minimum for any of the Control.value. Used for scaling, e.g. in bar graphs."@en ;
  rdfs:domain cim:AnalogControl ;
  rdfs:isDefinedBy :Package_Standard ;
  rdfs:range xsd:float ;
  uml:hasStereotype uml:attribute ;
  uml:id "EAID_7CF1169E_5683_4408_AAB0_9665D589AEA0" .

cim:AnalogLimit.value a owl:DatatypeProperty, owl:FunctionalProperty ;
  rdfs:label "value" ;
  rdfs:comment "The value to supervise against."@en ;
  rdfs:domain cim:AnalogLimit ;
  rdfs:isDefinedBy :Package_Standard ;
  rdfs:range xsd:float ;
  uml:hasStereotype uml:attribute ;
  uml:id "EAID_B166D469_E09B_4b00_8726_89B978C68595" .

cim:AnalogValue.value a owl:DatatypeProperty, owl:FunctionalProperty ;
  rdfs:label "value" ;
  rdfs:comment "The value to supervise."@en ;
  rdfs:domain cim:AnalogValue ;
  rdfs:isDefinedBy :Package_Standard ;
  rdfs:range xsd:float ;
  uml:hasStereotype uml:attribute ;
  uml:id "EAID_FCD31E82_1FA5_49d6_B6F0_E54AC2F5EBBC" .

cim:BasicIntervalSchedule.startTime a owl:DatatypeProperty, owl:FunctionalProperty ;
  rdfs:label "startTime" ;
  rdfs:comment "The time for the first time point."@en ;
  rdfs:domain cim:BasicIntervalSchedule ;
  rdfs:isDefinedBy :Package_Standard ;
  rdfs:range xsd:dateTime ;
  uml:hasStereotype uml:attribute ;
  uml:id "EAID_B2293058_38B0_4b6a_99E1_E92BF855F521" .

cim:CDPSMVersion.baseIec61968 a owl:DatatypeProperty, owl:FunctionalProperty ;
  rdfs:label "baseIec61968" ;
  rdfs:comment "Base UML provided by CIM model manager, submodel 61968."@en ;
  rdfs:domain cim:CDPSMVersion ;
  rdfs:isDefinedBy :Package_Extensions ;
  rdfs:range xsd:string ;
  uml:hasInitialValue "iec61968cim13v09" ;
  uml:hasStereotype uml:attribute ;
  uml:id "EAID_1970E2C0_DACC_4a56_93E0_64EFD94A9EAE" .

cim:CDPSMVersion.baseIec61970 a owl:DatatypeProperty, owl:FunctionalProperty ;
  rdfs:label "baseIec61970" ;
  rdfs:comment "Base UML provided by CIM model manager, submodel 61970."@en ;
  rdfs:domain cim:CDPSMVersion ;
  rdfs:isDefinedBy :Package_Extensions ;
  rdfs:range xsd:string ;
  uml:hasInitialValue "iec61970cim17v19" ;
  uml:hasStereotype uml:attribute ;
  uml:id "EAID_A840C944_510F_46d8_8CFE_FEB825CA3494" .

cim:CDPSMVersion.baseURI a owl:DatatypeProperty, owl:FunctionalProperty ;
  rdfs:label "baseURI" ;
  rdfs:comment "Profile URI used in the Model Exchange header and defined in IEC standards.  It uniquely identifies the Profile and its version. It is given for information only and to identify the closest IEC profile to which this CGMES profile is based on."@en ;
  rdfs:domain cim:CDPSMVersion ;
  rdfs:isDefinedBy :Package_Extensions ;
  rdfs:range xsd:string ;
  uml:hasInitialValue "none" ;
  uml:hasStereotype uml:attribute ;
  uml:id "EAID_D8A307FA_4BAA_4f07_8F0A_8B5C3D86C6A1" .

cim:CDPSMVersion.date a owl:DatatypeProperty, owl:FunctionalProperty ;
  rdfs:label "date" ;
  rdfs:comment """Profile creation date
Form is YYYY-MM-DD for example for January 5, 2009 it is 2009-01-05."""@en ;
  rdfs:domain cim:CDPSMVersion ;
  rdfs:isDefinedBy :Package_Extensions ;
  rdfs:range xsd:date ;
  uml:hasInitialValue "2017-05-15" ;
  uml:hasStereotype uml:attribute ;
  uml:id "EAID_DF772018_A2E0_4d6c_9BB4_C3E163783425" .

cim:CDPSMVersion.differenceModelURI a owl:DatatypeProperty, owl:FunctionalProperty ;
  rdfs:label "differenceModelURI" ;
  rdfs:comment "Difference model URI defined by IEC 61970-552."@en ;
  rdfs:domain cim:CDPSMVersion ;
  rdfs:isDefinedBy :Package_Extensions ;
  rdfs:range xsd:string ;
  uml:hasInitialValue "none" ;
  uml:hasStereotype uml:attribute ;
  uml:id "EAID_DB86C423_0254_438b_B485_F7737ED12D7A" .

cim:CDPSMVersion.namespaceRDF a owl:DatatypeProperty, owl:FunctionalProperty ;
  rdfs:label "namespaceRDF" ;
  rdfs:comment "RDF namespace."@en ;
  rdfs:domain cim:CDPSMVersion ;
  rdfs:isDefinedBy :Package_Extensions ;
  rdfs:range xsd:string ;
  uml:hasInitialValue "http://www.w3.org/1999/02/22-rdf-syntax-ns#" ;
  uml:hasStereotype uml:attribute ;
  uml:id "EAID_DFA95D2C_8997_4791_B719_FA6E6F31AEF5" .

cim:CDPSMVersion.namespace_CDPSM_UML a owl:DatatypeProperty, owl:FunctionalProperty ;
  rdfs:label "namespace_CDPSM_UML" ;
  rdfs:comment "UML extensions version (format cdpsm_vXX) (obsolete namespace)"@en ;
  rdfs:domain cim:CDPSMVersion ;
  rdfs:isDefinedBy :Package_Extensions ;
  rdfs:range xsd:string ;
  uml:hasInitialValue "http://edf.fr/CDPSM/2016/cdpsm2015#" ;
  uml:hasStereotype uml:attribute ;
  uml:id "EAID_56D65BBE_EB99_4585_8CAE_CC4B9BE0B5D5" .

cim:CDPSMVersion.namespace_CIMEXT_UML a owl:DatatypeProperty, owl:FunctionalProperty ;
  rdfs:label "namespace_CIMEXT_UML" ;
  rdfs:comment "namespace for components extensions to CIM, used in CDPSM (not defined in CIM but used by CDPSM should be added to CIM in a next release)"@en ;
  rdfs:domain cim:CDPSMVersion ;
  rdfs:isDefinedBy :Package_Extensions ;
  rdfs:range xsd:string ;
  uml:hasInitialValue "http://edf.fr/draft/cim17-ext#" ;
  uml:hasStereotype uml:attribute ;
  uml:id "EAID_A54C4F1D_4EA1_42d8_8986_CA3254221EA9" .

cim:CDPSMVersion.namespace_CIMINFO_UML a owl:DatatypeProperty, owl:FunctionalProperty ;
  rdfs:label "namespace_CIMINFO_UML" ;
  rdfs:comment "namespace for CIM informative components used in CDPSM (defined in CIM but not considered stabilized and noty part of the standard)"@en ;
  rdfs:domain cim:CDPSMVersion ;
  rdfs:isDefinedBy :Package_Extensions ;
  rdfs:range xsd:string ;
  uml:hasInitialValue "http://edf.fr/draft/cim17-info#" ;
  uml:hasStereotype uml:attribute ;
  uml:id "EAID_A454E13E_854C_4928_AF86_D20C5DE7912D" .

cim:CDPSMVersion.namespace_CIM_UML a owl:DatatypeProperty, owl:FunctionalProperty ;
  rdfs:label "namespace_CIM_UML" ;
  rdfs:comment "CIM UML namespace.  for elements considered as standard (not informative or extension)."@en ;
  rdfs:domain cim:CDPSMVersion ;
  rdfs:isDefinedBy :Package_Extensions ;
  rdfs:range xsd:string ;
  uml:hasInitialValue "https://cim.ucaiug.io/ns#" ;
  uml:hasStereotype uml:attribute ;
  uml:id "EAID_2431B278_EAB3_409d_8EDF_31CF3B06EBB6" .

cim:CDPSMVersion.namespace_EDFEXT_UML a owl:DatatypeProperty, owl:FunctionalProperty ;
  rdfs:label "namespace_EDFEXT_UML" ;
  rdfs:comment "namespace for components extensions to CIM, used in CDPSM (not defined in CIM but used by CDPSM should be added to CIM in a next release)"@en ;
  rdfs:domain cim:CDPSMVersion ;
  rdfs:isDefinedBy :Package_Extensions ;
  rdfs:range xsd:string ;
  uml:hasInitialValue "http://der.edf.fr/mire/MSite-v3.1.a#" ;
  uml:hasStereotype uml:attribute ;
  uml:id "EAID_71A33F21_3B47_40c5_B402_5759D2AD459C" .

cim:CDPSMVersion.namespace_ENTSOE_UML a owl:DatatypeProperty, owl:FunctionalProperty ;
  rdfs:label "namespace_ENTSOE_UML" ;
  rdfs:comment "namespace for components extensions to CIM, used in CGMES and CDPSM"@en ;
  rdfs:domain cim:CDPSMVersion ;
  rdfs:isDefinedBy :Package_Extensions ;
  rdfs:range xsd:string ;
  uml:hasInitialValue "http://entsoe.eu/CIM/SchemaExtension/3/1#" ;
  uml:hasStereotype uml:attribute ;
  uml:id "EAID_AD939A3B_164A_4ef1_A322_9B323EAC9AC7" .

cim:CDPSMVersion.version a owl:DatatypeProperty, owl:FunctionalProperty ;
  rdfs:label "version" ;
  rdfs:comment "working in progress to construct profiles."@en ;
  rdfs:domain cim:CDPSMVersion ;
  rdfs:isDefinedBy :Package_Extensions ;
  rdfs:range xsd:string ;
  uml:hasInitialValue "cdpsm2015 v1.2.5" ;
  uml:hasStereotype uml:attribute ;
  uml:id "EAID_58C81E00_5CD5_4ea2_AFA9_D97052FBA0ED" .

cim:Command.normalValue a owl:DatatypeProperty, owl:FunctionalProperty ;
  rdfs:label "normalValue" ;
  rdfs:comment "Normal value for Control.value e.g. used for percentage scaling."@en ;
  rdfs:domain cim:Command ;
  rdfs:isDefinedBy :Package_Standard ;
  rdfs:range xsd:integer ;
  uml:hasStereotype uml:attribute ;
  uml:id "EAID_0A6D3BCB_DAD4_48b5_BBF8_69CC8E7FB5AD" .

cim:Command.value a owl:DatatypeProperty, owl:FunctionalProperty ;
  rdfs:label "value" ;
  rdfs:comment "The value representing the actuator output."@en ;
  rdfs:domain cim:Command ;
  rdfs:isDefinedBy :Package_Standard ;
  rdfs:range xsd:integer ;
  uml:hasStereotype uml:attribute ;
  uml:id "EAID_BC01F247_D315_4228_AE63_7DCC7ED0D3FB" .

cim:Control.controlType a owl:DatatypeProperty, owl:FunctionalProperty ;
  rdfs:label "controlType" ;
  rdfs:comment "Specifies the type of Control, e.g. BreakerOn/Off, GeneratorVoltageSetPoint, TieLineFlow etc. The ControlType.name shall be unique among all specified types and describe the type."@en ;
  rdfs:domain cim:Control ;
  rdfs:isDefinedBy :Package_Standard ;
  rdfs:range xsd:string ;
  uml:hasStereotype uml:attribute ;
  uml:id "EAID_69F2D4DF_EAE8_4f90_97E5_76668E9464A2" .

cim:Control.operationInProgress a owl:DatatypeProperty, owl:FunctionalProperty ;
  rdfs:label "operationInProgress" ;
  rdfs:comment "Indicates that a client is currently sending control commands that has not completed."@en ;
  rdfs:domain cim:Control ;
  rdfs:isDefinedBy :Package_Standard ;
  rdfs:range xsd:boolean ;
  uml:hasStereotype uml:attribute ;
  uml:id "EAID_41263C28_2F9A_424c_9A5D_C1206B1A49AF" .

cim:Control.timeStamp a owl:DatatypeProperty, owl:FunctionalProperty ;
  rdfs:label "timeStamp" ;
  rdfs:comment "The last time a control output was sent."@en ;
  rdfs:domain cim:Control ;
  rdfs:isDefinedBy :Package_Standard ;
  rdfs:range xsd:dateTime ;
  uml:hasStereotype uml:attribute ;
  uml:id "EAID_6FF288AF_D715_42d7_9B37_EFEC80095FE4" .

cim:DateTimeInterval.end a owl:DatatypeProperty, owl:FunctionalProperty ;
  rdfs:label "end" ;
  rdfs:comment "End date and time of this interval."@en ;
  rdfs:domain cim:DateTimeInterval ;
  rdfs:isDefinedBy :Package_CompoundTypes ;
  rdfs:range xsd:dateTime ;
  uml:hasStereotype uml:attribute ;
  uml:id "EAID_0ABC99C4_CBB4_45f5_8A37_418A0411A32D" .

cim:DateTimeInterval.start a owl:DatatypeProperty, owl:FunctionalProperty ;
  rdfs:label "start" ;
  rdfs:comment "Start date and time of this interval."@en ;
  rdfs:domain cim:DateTimeInterval ;
  rdfs:isDefinedBy :Package_CompoundTypes ;
  rdfs:range xsd:dateTime ;
  uml:hasStereotype uml:attribute ;
  uml:id "EAID_1541ACE8_204E_4f8c_ADED_0C21681F617D" .

cim:Discrete.maxValue a owl:DatatypeProperty, owl:FunctionalProperty ;
  rdfs:label "maxValue" ;
  rdfs:comment "Normal value range maximum for any of the MeasurementValue.values. Used for scaling, e.g. in bar graphs or of telemetered raw values."@en ;
  rdfs:domain cim:Discrete ;
  rdfs:isDefinedBy :Package_Standard ;
  rdfs:range xsd:integer ;
  uml:hasStereotype uml:attribute ;
  uml:id "EAID_EF794F96_052C_4dd5_909F_19D54E36CEEC" .

cim:Discrete.minValue a owl:DatatypeProperty, owl:FunctionalProperty ;
  rdfs:label "minValue" ;
  rdfs:comment "Normal value range minimum for any of the MeasurementValue.values. Used for scaling, e.g. in bar graphs or of telemetered raw values"@en ;
  rdfs:domain cim:Discrete ;
  rdfs:isDefinedBy :Package_Standard ;
  rdfs:range xsd:integer ;
  uml:hasStereotype uml:attribute ;
  uml:id "EAID_00394036_6CC1_4f72_8409_B7389253B028" .

cim:Discrete.normalValue a owl:DatatypeProperty, owl:FunctionalProperty ;
  rdfs:label "normalValue" ;
  rdfs:comment "Normal measurement value, e.g., used for percentage calculations."@en ;
  rdfs:domain cim:Discrete ;
  rdfs:isDefinedBy :Package_Standard ;
  rdfs:range xsd:integer ;
  uml:hasStereotype uml:attribute ;
  uml:id "EAID_D32F2F6C_05F4_4833_91B5_2055778F3272" .

cim:DiscreteValue.value a owl:DatatypeProperty, owl:FunctionalProperty ;
  rdfs:label "value" ;
  rdfs:comment "The value to supervise."@en ;
  rdfs:domain cim:DiscreteValue ;
  rdfs:isDefinedBy :Package_Standard ;
  rdfs:range xsd:integer ;
  uml:hasStereotype uml:attribute ;
  uml:id "EAID_292261BB_5846_4507_BBDA_BDE2C42DF707" .

cim:Equipment.normallyInService a owl:DatatypeProperty, owl:FunctionalProperty ;
  rdfs:label "normallyInService" ;
  rdfs:comment "If true, the equipment is normally in service."@en ;
  rdfs:domain cim:Equipment ;
  rdfs:isDefinedBy :Package_Standard ;
  rdfs:range xsd:boolean ;
  uml:hasStereotype uml:attribute ;
  uml:id "EAID_8A26EDE9_88D6_4736_9A7E_7872904E5167" .

cim:IEC61968CIMVersion.date a owl:DatatypeProperty, owl:FunctionalProperty ;
  rdfs:label "date" ;
  rdfs:comment "Form is YYYY-MM-DD for example for January 5, 2009 it is 2009-01-05."@en ;
  rdfs:domain cim:IEC61968CIMVersion ;
  rdfs:isDefinedBy :Package_CDPSM2015_Versions ;
  rdfs:range xsd:date ;
  uml:hasInitialValue "2016-06-22" ;
  uml:hasStereotype uml:attribute ;
  uml:id "EAID_41AEDCC5_85BE_4aa8_9858_AFA1476927C0" .

cim:IEC61968CIMVersion.version a owl:DatatypeProperty, owl:FunctionalProperty ;
  rdfs:label "version" ;
  rdfs:comment "Form is IEC61968CIMXXvYY where XX is the major CIM package version and the YY is the minor version. For example IEC61968CIM10v17."@en ;
  rdfs:domain cim:IEC61968CIMVersion ;
  rdfs:isDefinedBy :Package_CDPSM2015_Versions ;
  rdfs:range xsd:string ;
  uml:hasInitialValue "IEC61968CIM13v09" ;
  uml:hasStereotype uml:attribute ;
  uml:id "EAID_856CD9B1_8D25_409e_9443_BC7BD9970C40" .

cim:IEC61970CIMVersion.date a owl:DatatypeProperty, owl:FunctionalProperty ;
  rdfs:label "date" ;
  rdfs:comment "Form is YYYY-MM-DD for example for January 5, 2009 it is 2009-01-05."@en ;
  rdfs:domain cim:IEC61970CIMVersion ;
  rdfs:isDefinedBy :Package_CDPSM2015_Versions ;
  rdfs:range xsd:date ;
  uml:hasInitialValue "2016-10-28" ;
  uml:hasStereotype uml:attribute ;
  uml:id "EAID_73319DDD_3044_4b10_BF3F_B98F7D4335FB" .

cim:IEC61970CIMVersion.version a owl:DatatypeProperty, owl:FunctionalProperty ;
  rdfs:label "version" ;
  rdfs:comment "Form is IEC61970CIMXXvYY where XX is the major CIM package version and the YY is the minor version. For example IEC61970CIM13v18."@en ;
  rdfs:domain cim:IEC61970CIMVersion ;
  rdfs:isDefinedBy :Package_CDPSM2015_Versions ;
  rdfs:range xsd:string ;
  uml:hasInitialValue "IEC61970CIM17v19" ;
  uml:hasStereotype uml:attribute ;
  uml:id "EAID_A34E3511_2B8B_47f5_83E6_23564E48933C" .

cim:IdentifiedObject.aliasName a owl:DatatypeProperty, owl:FunctionalProperty ;
  rdfs:label "aliasName" ;
  rdfs:comment """The aliasName is free text human readable name of the object alternative to IdentifiedObject.name. It may be non unique and may not correlate to a naming hierarchy.
The attribute aliasName is retained because of backwards compatibility between CIM relases. It is however recommended to replace aliasName with the Name class as aliasName is planned for retirement at a future time."""@en ;
  rdfs:domain cim:IdentifiedObject ;
  rdfs:isDefinedBy :Package_Standard ;
  rdfs:range xsd:string ;
  uml:hasStereotype uml:attribute ;
  uml:id "EAID_85373F6D_E3F5_489c_B6E9_5871A6048FD8" .

cim:IdentifiedObject.description a owl:DatatypeProperty, owl:FunctionalProperty ;
  rdfs:label "description" ;
  rdfs:comment "The description is a free human readable text describing or naming the object. It may be non unique and may not correlate to a naming hierarchy."@en ;
  rdfs:domain cim:IdentifiedObject ;
  rdfs:isDefinedBy :Package_Standard ;
  rdfs:range xsd:string ;
  uml:hasStereotype uml:attribute ;
  uml:id "EAID_A82DC097_F3B4_4687_8609_6693D6AA765C" .

cim:IdentifiedObject.mRID a owl:DatatypeProperty, owl:FunctionalProperty ;
  rdfs:label "mRID" ;
  rdfs:comment """Master resource identifier issued by a model authority. The mRID is globally unique within an exchange context. Global uniqueness is easily achieved by using a UUID,  as specified in RFC 4122, for the mRID.  The use of UUID is strongly recommended.
For CIMXML data files in RDF syntax conforming to IEC 61970-552 Edition 1, the mRID is mapped to rdf:ID or rdf:about attributes that identify CIM object elements."""@en ;
  rdfs:domain cim:IdentifiedObject ;
  rdfs:isDefinedBy :Package_Standard ;
  rdfs:range xsd:string ;
  uml:hasStereotype uml:attribute ;
  uml:id "EAID_71B3EE1D_B8CD_4fbe_90B2_7F7C844400E9" .

cim:IdentifiedObject.name a owl:DatatypeProperty, owl:FunctionalProperty ;
  rdfs:label "name" ;
  rdfs:comment "The name is any free human readable and possibly non unique text naming the object."@en ;
  rdfs:domain cim:IdentifiedObject ;
  rdfs:isDefinedBy :Package_Standard ;
  rdfs:range xsd:string ;
  uml:hasStereotype uml:attribute ;
  uml:id "EAID_9476DE5B_170C_4b9e_B93D_A821C562FBBE" .

cim:LifecycleDate.installationDate a owl:DatatypeProperty, owl:FunctionalProperty ;
  rdfs:label "installationDate" ;
  rdfs:comment "(if applicable) Date current installation was completed, which may not be the same as the in-service date. Asset may have been installed at other locations previously. Ignored if asset is (1) not currently installed (e.g., stored in a depot) or (2) not intended to be installed (e.g., vehicle, tool)."@en ;
  rdfs:domain cim:LifecycleDate ;
  rdfs:isDefinedBy :Package_CompoundTypes ;
  rdfs:range xsd:date ;
  uml:hasStereotype uml:attribute ;
  uml:id "EAID_F217E2B7_A6EF_4ac2_BBD4_43C83B8B995E" .

cim:LifecycleDate.manufacturedDate a owl:DatatypeProperty, owl:FunctionalProperty ;
  rdfs:label "manufacturedDate" ;
  rdfs:comment "Date the asset was manufactured."@en ;
  rdfs:domain cim:LifecycleDate ;
  rdfs:isDefinedBy :Package_CompoundTypes ;
  rdfs:range xsd:date ;
  uml:hasStereotype uml:attribute ;
  uml:id "EAID_FB93BCF2_1C59_4f75_A5BF_EA1A77E2DDA2" .

cim:LifecycleDate.purchaseDate a owl:DatatypeProperty, owl:FunctionalProperty ;
  rdfs:label "purchaseDate" ;
  rdfs:comment "Date the asset was purchased. Note that even though an asset may have been purchased, it may not have been received into inventory at the time of purchase."@en ;
  rdfs:domain cim:LifecycleDate ;
  rdfs:isDefinedBy :Package_CompoundTypes ;
  rdfs:range xsd:date ;
  uml:hasStereotype uml:attribute ;
  uml:id "EAID_67A99AE2_0EC4_4726_AA84_6932D5342E0F" .

cim:LifecycleDate.receivedDate a owl:DatatypeProperty, owl:FunctionalProperty ;
  rdfs:label "receivedDate" ;
  rdfs:comment "Date the asset was received and first placed into inventory."@en ;
  rdfs:domain cim:LifecycleDate ;
  rdfs:isDefinedBy :Package_CompoundTypes ;
  rdfs:range xsd:date ;
  uml:hasStereotype uml:attribute ;
  uml:id "EAID_4AC4E0C8_145C_4ea3_AC43_59DD55DC0B76" .

cim:LifecycleDate.removalDate a owl:DatatypeProperty, owl:FunctionalProperty ;
  rdfs:label "removalDate" ;
  rdfs:comment "(if applicable) Date when the asset was last removed from service. Ignored if (1) not intended to be in service, or (2) currently in service."@en ;
  rdfs:domain cim:LifecycleDate ;
  rdfs:isDefinedBy :Package_CompoundTypes ;
  rdfs:range xsd:date ;
  uml:hasStereotype uml:attribute ;
  uml:id "EAID_DA08E6B4_43FF_4bb1_87C6_267E1E2E8257" .

cim:LifecycleDate.retiredDate a owl:DatatypeProperty, owl:FunctionalProperty ;
  rdfs:label "retiredDate" ;
  rdfs:comment "(if applicable) Date the asset is permanently retired from service and may be scheduled for disposal. Ignored if asset is (1) currently in service, or (2) permanently removed from service."@en ;
  rdfs:domain cim:LifecycleDate ;
  rdfs:isDefinedBy :Package_CompoundTypes ;
  rdfs:range xsd:date ;
  uml:hasStereotype uml:attribute ;
  uml:id "EAID_227AFC69_980F_45c2_A789_5ED9B056F9CA" .

cim:LimitSet.isPercentageLimits a owl:DatatypeProperty, owl:FunctionalProperty ;
  rdfs:label "isPercentageLimits" ;
  rdfs:comment "Tells if the limit values are in percentage of normalValue or the specified Unit for Measurements and Controls."@en ;
  rdfs:domain cim:LimitSet ;
  rdfs:isDefinedBy :Package_Standard ;
  rdfs:range xsd:boolean ;
  uml:hasStereotype uml:attribute ;
  uml:id "EAID_64E20EBC_964F_496d_BC24_742F788DD36E" .

cim:Measurement.measurementType a owl:DatatypeProperty, owl:FunctionalProperty ;
  rdfs:label "measurementType" ;
  rdfs:comment "Specifies the type of Measurement, e.g. IndoorTemperature, OutDoorTemperature, BusVoltage, GeneratorVoltage, LineFlow etc."@en ;
  rdfs:domain cim:Measurement ;
  rdfs:isDefinedBy :Package_Standard ;
  rdfs:range xsd:string ;
  uml:hasStereotype uml:attribute ;
  uml:id "EAID_7BD1DAD8_5639_44ba_A8BC_C936BA1D8913" .

cim:MeasurementValue.timeStamp a owl:DatatypeProperty, owl:FunctionalProperty ;
  rdfs:label "timeStamp" ;
  rdfs:comment "The time when the value was last updated"@en ;
  rdfs:domain cim:MeasurementValue ;
  rdfs:isDefinedBy :Package_Standard ;
  rdfs:range xsd:dateTime ;
  uml:hasStereotype uml:attribute ;
  uml:id "EAID_A4975DDC_85A3_4029_B410_DC37CB64B030" .

cim:Name.name a owl:DatatypeProperty, owl:FunctionalProperty ;
  rdfs:label "name" ;
  rdfs:comment "Any free text that name the object."@en ;
  rdfs:domain cim:Name ;
  rdfs:isDefinedBy :Package_Standard ;
  rdfs:range xsd:string ;
  uml:hasStereotype uml:attribute ;
  uml:id "EAID_B6ED19EA_05FB_43d5_BCD6_8BC4C5304335" .

cim:NameType.description a owl:DatatypeProperty, owl:FunctionalProperty ;
  rdfs:label "description" ;
  rdfs:comment "Description of the name type."@en ;
  rdfs:domain cim:NameType ;
  rdfs:isDefinedBy :Package_Standard ;
  rdfs:range xsd:string ;
  uml:hasStereotype uml:attribute ;
  uml:id "EAID_15B011AB_ACB4_4f70_9975_314AC49DB5FE" .

cim:NameType.name a owl:DatatypeProperty, owl:FunctionalProperty ;
  rdfs:label "name" ;
  rdfs:comment "Name of the name type."@en ;
  rdfs:domain cim:NameType ;
  rdfs:isDefinedBy :Package_Standard ;
  rdfs:range xsd:string ;
  uml:hasStereotype uml:attribute ;
  uml:id "EAID_FA12CC23_5F4E_47a0_9B53_A74CDEA962B4" .

cim:NameTypeAuthority.description a owl:DatatypeProperty, owl:FunctionalProperty ;
  rdfs:label "description" ;
  rdfs:comment "Description of the name type authority."@en ;
  rdfs:domain cim:NameTypeAuthority ;
  rdfs:isDefinedBy :Package_Standard ;
  rdfs:range xsd:string ;
  uml:hasStereotype uml:attribute ;
  uml:id "EAID_88A7A6AD_39D8_4818_AB35_9448066F2831" .

cim:NameTypeAuthority.name a owl:DatatypeProperty, owl:FunctionalProperty ;
  rdfs:label "name" ;
  rdfs:comment "Name of the name type authority."@en ;
  rdfs:domain cim:NameTypeAuthority ;
  rdfs:isDefinedBy :Package_Standard ;
  rdfs:range xsd:string ;
  uml:hasStereotype uml:attribute ;
  uml:id "EAID_F366DF55_BDD2_4380_86B5_AAB87116F194" .

cim:PowerTransformer.vectorGroup a owl:DatatypeProperty, owl:FunctionalProperty ;
  rdfs:label "vectorGroup" ;
  rdfs:comment """Vector group of the transformer for protective relaying, e.g., Dyn1. For unbalanced transformers, this may not be simply determined from the constituent winding connections and phase angle dispacements.

The vectorGroup string consists of the following components in the order listed: high voltage winding connection, mid voltage winding connection (for three winding transformers), phase displacement clock number from 0 to 11,  low voltage winding connection 
phase displacement clock number from 0 to 11.   The winding connections are D (delta), Y (wye), YN (wye with neutral), Z (zigzag), ZN (zigzag with neutral), A (auto transformer). Upper case means the high voltage, lower case mid or low. The high voltage winding always has clock postion 0 and is not included in the vector group string.  Some examples: YNy0 (two winding wye to wye with no phase displacement), YNd11 (two winding wye to delta with 330 degrees phase displacement), YNyn0d5 (three winding transformer wye with neutral high voltgage, wye with neutral mid voltgage and no phase displacement, delta low voltage with 150 degrees displacement).

Phase displacement is defined as the angular difference between the phasors representing the voltages between the neutral point (real or imaginary) and the corresponding terminals of two windings, a positive sequence voltage system being applied to the high-voltage terminals, following each other in alphabetical sequence if they are lettered, or in numerical sequence if they are numbered: the phasors are assumed to rotate in a counter-clockwise sense."""@en ;
  rdfs:domain cim:PowerTransformer ;
  rdfs:isDefinedBy :Package_Standard ;
  rdfs:range xsd:string ;
  uml:hasStereotype uml:attribute ;
  uml:id "EAID_D4479242_6042_413b_85EC_8667ADA26CBD" .

cim:RegularIntervalSchedule.endTime a owl:DatatypeProperty, owl:FunctionalProperty ;
  rdfs:label "endTime" ;
  rdfs:comment "The time for the last time point."@en ;
  rdfs:domain cim:RegularIntervalSchedule ;
  rdfs:isDefinedBy :Package_Standard ;
  rdfs:range xsd:dateTime ;
  uml:hasStereotype uml:attribute ;
  uml:id "EAID_A63E0404_2C88_47ff_8373_D3E6C85AF81B" .

cim:RegularTimePoint.sequenceNumber a owl:DatatypeProperty, owl:FunctionalProperty ;
  rdfs:label "sequenceNumber" ;
  rdfs:comment "The position of the regular time point in the sequence. Note that time points don't have to be sequential, i.e. time points may be omitted. The actual time for a RegularTimePoint is computed by multiplying the associated regular interval schedule's time step with the regular time point sequence number and adding the associated schedules start time."@en ;
  rdfs:domain cim:RegularTimePoint ;
  rdfs:isDefinedBy :Package_Standard ;
  rdfs:range xsd:integer ;
  uml:hasStereotype uml:attribute ;
  uml:id "EAID_9540E035_C407_45f4_93FF_7030F87C32F4" .

cim:RegularTimePoint.value1 a owl:DatatypeProperty, owl:FunctionalProperty ;
  rdfs:label "value1" ;
  rdfs:comment "The first value at the time. The meaning of the value is defined by the derived type of the associated schedule."@en ;
  rdfs:domain cim:RegularTimePoint ;
  rdfs:isDefinedBy :Package_Standard ;
  rdfs:range xsd:float ;
  uml:hasStereotype uml:attribute ;
  uml:id "EAID_4AA74F16_8CA9_4360_AE8A_DB0D82D8CA95" .

cim:RegularTimePoint.value2 a owl:DatatypeProperty, owl:FunctionalProperty ;
  rdfs:label "value2" ;
  rdfs:comment "The second value at the time. The meaning of the value is defined by the derived type of the associated schedule."@en ;
  rdfs:domain cim:RegularTimePoint ;
  rdfs:isDefinedBy :Package_Standard ;
  rdfs:range xsd:float ;
  uml:hasStereotype uml:attribute ;
  uml:id "EAID_C51FF151_783F_44a3_A7F9_9372DE484926" .

cim:RemoteControl.remoteControlled a owl:DatatypeProperty, owl:FunctionalProperty ;
  rdfs:label "remoteControlled" ;
  rdfs:comment "Set to true if the actuator is remotely controlled."@en ;
  rdfs:domain cim:RemoteControl ;
  rdfs:isDefinedBy :Package_Standard ;
  rdfs:range xsd:boolean ;
  uml:hasStereotype uml:attribute ;
  uml:id "EAID_EEB1737C_F11E_4b9b_9962_62406BC3A1B1" .

cim:SetPoint.normalValue a owl:DatatypeProperty, owl:FunctionalProperty ;
  rdfs:label "normalValue" ;
  rdfs:comment "Normal value for Control.value e.g. used for percentage scaling."@en ;
  rdfs:domain cim:SetPoint ;
  rdfs:isDefinedBy :Package_Standard ;
  rdfs:range xsd:float ;
  uml:hasStereotype uml:attribute ;
  uml:id "EAID_D2BC916F_9291_4f68_ADE0_5B6218DDC5D8" .

cim:SetPoint.value a owl:DatatypeProperty, owl:FunctionalProperty ;
  rdfs:label "value" ;
  rdfs:comment "The value representing the actuator output."@en ;
  rdfs:domain cim:SetPoint ;
  rdfs:isDefinedBy :Package_Standard ;
  rdfs:range xsd:float ;
  uml:hasStereotype uml:attribute ;
  uml:id "EAID_B7E412FC_AF76_49b8_A88C_1C0642C24E87" .

cim:Status.dateTime a owl:DatatypeProperty, owl:FunctionalProperty ;
  rdfs:label "dateTime" ;
  rdfs:comment "Date and time for which status 'value' applies."@en ;
  rdfs:domain cim:Status ;
  rdfs:isDefinedBy :Package_CompoundTypes ;
  rdfs:range xsd:dateTime ;
  uml:hasStereotype uml:attribute ;
  uml:id "EAID_286829E9_8B62_471f_8507_68D03E2B9A3F" .

cim:Status.reason a owl:DatatypeProperty, owl:FunctionalProperty ;
  rdfs:label "reason" ;
  rdfs:comment "Reason code or explanation for why an object went to the current status 'value'."@en ;
  rdfs:domain cim:Status ;
  rdfs:isDefinedBy :Package_CompoundTypes ;
  rdfs:range xsd:string ;
  uml:hasStereotype uml:attribute ;
  uml:id "EAID_51E12DAD_FC37_4dfe_A8E4_A273F0EFD65C" .

cim:Status.remark a owl:DatatypeProperty, owl:FunctionalProperty ;
  rdfs:label "remark" ;
  rdfs:comment "Pertinent information regarding the current 'value', as free form text."@en ;
  rdfs:domain cim:Status ;
  rdfs:isDefinedBy :Package_CompoundTypes ;
  rdfs:range xsd:string ;
  uml:hasStereotype uml:attribute ;
  uml:id "EAID_8B7584AD_FB53_4d76_BBFE_72EE31608485" .

cim:Status.value a owl:DatatypeProperty, owl:FunctionalProperty ;
  rdfs:label "value" ;
  rdfs:comment "Status value at 'dateTime'; prior status changes may have been kept in instances of activity records associated with the object to which this status applies."@en ;
  rdfs:domain cim:Status ;
  rdfs:isDefinedBy :Package_CompoundTypes ;
  rdfs:range xsd:string ;
  uml:hasStereotype uml:attribute ;
  uml:id "EAID_0184B3DA_228D_41b3_AD2F_7C17DD4041D0" .

cim:StreetDetail.addressGeneral a owl:DatatypeProperty, owl:FunctionalProperty ;
  rdfs:label "addressGeneral" ;
  rdfs:comment "Additional address information, for example a mailstop."@en ;
  rdfs:domain cim:StreetDetail ;
  rdfs:isDefinedBy :Package_CompoundTypes ;
  rdfs:range xsd:string ;
  uml:hasStereotype uml:attribute ;
  uml:id "EAID_8A85C8D2_C0B9_4107_A0FC_B7B9EF07C4E9" .

cim:StreetDetail.name a owl:DatatypeProperty, owl:FunctionalProperty ;
  rdfs:label "name" ;
  rdfs:comment "Name of the street."@en ;
  rdfs:domain cim:StreetDetail ;
  rdfs:isDefinedBy :Package_CompoundTypes ;
  rdfs:range xsd:string ;
  uml:hasStereotype uml:attribute ;
  uml:id "EAID_947A58E8_F9CE_4429_BD6F_C705D885681C" .

cim:StreetDetail.number a owl:DatatypeProperty, owl:FunctionalProperty ;
  rdfs:label "number" ;
  rdfs:comment "Designator of the specific location on the street."@en ;
  rdfs:domain cim:StreetDetail ;
  rdfs:isDefinedBy :Package_CompoundTypes ;
  rdfs:range xsd:string ;
  uml:hasStereotype uml:attribute ;
  uml:id "EAID_64B56973_8008_434f_8AF7_03FE55395188" .

cim:StreetDetail.type a owl:DatatypeProperty, owl:FunctionalProperty ;
  rdfs:label "type" ;
  rdfs:comment "Type of street. Examples include: street, circle, boulevard, avenue, road, drive, etc."@en ;
  rdfs:domain cim:StreetDetail ;
  rdfs:isDefinedBy :Package_CompoundTypes ;
  rdfs:range xsd:string ;
  uml:hasStereotype uml:attribute ;
  uml:id "EAID_965CC979_ED3B_41f2_AAFF_3FFAE2035C15" .

cim:StringMeasurementValue.value a owl:DatatypeProperty, owl:FunctionalProperty ;
  rdfs:label "value" ;
  rdfs:comment "The value to supervise."@en ;
  rdfs:domain cim:StringMeasurementValue ;
  rdfs:isDefinedBy :Package_Standard ;
  rdfs:range xsd:string ;
  uml:hasStereotype uml:attribute ;
  uml:id "EAID_EA0F539C_1A09_4031_9B9A_15B322562042" .

cim:Switch.normalOpen a owl:DatatypeProperty, owl:FunctionalProperty ;
  rdfs:label "normalOpen" ;
  rdfs:comment "The attribute is used in cases when no Measurement for the status value is present. If the Switch has a status measurment the Discrete.normalValue is expected to match with the Switch.normalOpen."@en ;
  rdfs:domain cim:Switch ;
  rdfs:isDefinedBy :Package_Standard ;
  rdfs:range xsd:boolean ;
  uml:hasStereotype uml:attribute ;
  uml:id "EAID_8D671AB0_E2B8_43fe_83EF_FA46AA165B44" .

cim:TownDetail.code a owl:DatatypeProperty, owl:FunctionalProperty ;
  rdfs:label "code" ;
  rdfs:comment "Town code."@en ;
  rdfs:domain cim:TownDetail ;
  rdfs:isDefinedBy :Package_CompoundTypes ;
  rdfs:range xsd:string ;
  uml:hasStereotype uml:attribute ;
  uml:id "EAID_CA70DEEB_1A1A_4719_8887_E0397E8ED173" .

cim:TownDetail.name a owl:DatatypeProperty, owl:FunctionalProperty ;
  rdfs:label "name" ;
  rdfs:comment "Town name."@en ;
  rdfs:domain cim:TownDetail ;
  rdfs:isDefinedBy :Package_CompoundTypes ;
  rdfs:range xsd:string ;
  uml:hasStereotype uml:attribute ;
  uml:id "EAID_111467DB_41AF_40c7_8D2A_800EA073C678" .

cim:TransformerEnd.endNumber a owl:DatatypeProperty, owl:FunctionalProperty ;
  rdfs:label "endNumber" ;
  rdfs:comment "Number for this transformer end, corresponding to the end's order in the PowerTransformer.vectorGroup attribute. Highest voltage winding should be 1."@en ;
  rdfs:domain cim:TransformerEnd ;
  rdfs:isDefinedBy :Package_Standard ;
  rdfs:range xsd:integer ;
  uml:hasStereotype uml:attribute ;
  uml:id "EAID_326FBA85_F66F_4c56_8716_FC15A7E01B44" .

cim:ValueToAlias.value a owl:DatatypeProperty, owl:FunctionalProperty ;
  rdfs:label "value" ;
  rdfs:comment "The value that is mapped."@en ;
  rdfs:domain cim:ValueToAlias ;
  rdfs:isDefinedBy :Package_Standard ;
  rdfs:range xsd:integer ;
  uml:hasStereotype uml:attribute ;
  uml:id "EAID_45BEC207_4261_41a9_A864_B1B89DA6F020" .

md:Description.description a owl:DatatypeProperty, owl:FunctionalProperty ;
  rdfs:label "description" ;
  rdfs:domain md:Description ;
  rdfs:isDefinedBy :Package_ModelDescription ;
  rdfs:range xsd:string ;
  uml:hasStereotype uml:attribute ;
  uml:id "EAID_77D4EA3B_765E_4535_8798_19A334B793CD" .

md:Description.name a owl:DatatypeProperty, owl:FunctionalProperty ;
  rdfs:label "name" ;
  rdfs:domain md:Description ;
  rdfs:isDefinedBy :Package_ModelDescription ;
  rdfs:range xsd:string ;
  uml:hasStereotype uml:attribute ;
  uml:id "EAID_2112E71B_4C0E_42fe_B846_0C25245AD4AA" .

md:Description.version a owl:DatatypeProperty, owl:FunctionalProperty ;
  rdfs:label "version" ;
  rdfs:domain md:Description ;
  rdfs:isDefinedBy :Package_ModelDescription ;
  rdfs:range xsd:integer ;
  uml:hasStereotype uml:attribute ;
  uml:id "EAID_FF52CCA3_DC42_415b_B3DC_1896EDF5D285" .

md:DescriptionID.uri a owl:DatatypeProperty, owl:FunctionalProperty ;
  rdfs:label "uri" ;
  rdfs:domain md:DescriptionID ;
  rdfs:isDefinedBy :Package_ModelDescription ;
  rdfs:range xsd:string ;
  uml:hasStereotype uml:attribute ;
  uml:id "EAID_3CE77DD2_B3AC_4276_8CD1_5C88ACFD6925" .

md:Model.created a owl:DatatypeProperty, owl:FunctionalProperty ;
  rdfs:label "created" ;
  rdfs:domain md:Model ;
  rdfs:isDefinedBy :Package_ModelDescription ;
  rdfs:range xsd:dateTime ;
  uml:hasStereotype uml:attribute ;
  uml:id "EAID_D9AA16E6_6140_43bb_8AE1_6BB4690421D5" .

md:Model.description a owl:DatatypeProperty, owl:FunctionalProperty ;
  rdfs:label "description" ;
  rdfs:domain md:Model ;
  rdfs:isDefinedBy :Package_ModelDescription ;
  rdfs:range xsd:string ;
  uml:hasStereotype uml:attribute ;
  uml:id "EAID_2D2FD5B2_D2E1_4f18_B2A6_C344E4F8F056" .

md:Model.scenarioTime a owl:DatatypeProperty, owl:FunctionalProperty ;
  rdfs:label "scenarioTime" ;
  rdfs:domain md:Model ;
  rdfs:isDefinedBy :Package_ModelDescription ;
  rdfs:range xsd:dateTime ;
  uml:hasStereotype uml:attribute ;
  uml:id "EAID_93B61862_8552_4d68_982A_5988CF10A5CE" .

md:Model.version a owl:DatatypeProperty, owl:FunctionalProperty ;
  rdfs:label "version" ;
  rdfs:domain md:Model ;
  rdfs:isDefinedBy :Package_ModelDescription ;
  rdfs:range xsd:string ;
  uml:hasStereotype uml:attribute ;
  uml:id "EAID_5C9430BF_6E71_4a91_93D8_4EE62DF835AF" .

md:ModelDescriptionCIMVersion.date a owl:DatatypeProperty, owl:FunctionalProperty ;
  rdfs:label "date" ;
  rdfs:domain md:ModelDescriptionCIMVersion ;
  rdfs:isDefinedBy :Package_ModelDescription ;
  rdfs:range xsd:date ;
  uml:hasStereotype uml:attribute ;
  uml:id "EAID_3D4AE5F1_0F47_469a_88ED_6CA88FE74BAC" .

md:ModelDescriptionCIMVersion.version a owl:DatatypeProperty, owl:FunctionalProperty ;
  rdfs:label "version" ;
  rdfs:domain md:ModelDescriptionCIMVersion ;
  rdfs:isDefinedBy :Package_ModelDescription ;
  rdfs:range xsd:string ;
  uml:hasStereotype uml:attribute ;
  uml:id "EAID_E4CE2321_4D4C_4ff2_B28D_9379D107022B" .

next:EnergyConsumerEx.specialNeed a owl:DatatypeProperty, owl:FunctionalProperty ;
  rdfs:label "specialNeed" ;
  rdfs:comment "Special service needs for the person (contact) are described; examples include life support, etc."@en ;
  rdfs:domain next:EnergyConsumerEx ;
  rdfs:isDefinedBy :Package_EDFExtensionsFunctional ;
  rdfs:range xsd:string ;
  uml:hasStereotype uml:attribute ;
  uml:id "EAID_6A147458_DAFE_44c2_9E13_689E74082838" .

next:ProtectedSwitchEx.remoteControlled a owl:DatatypeProperty, owl:FunctionalProperty ;
  rdfs:label "remoteControlled" ;
  rdfs:comment """Tell if the switch is remote controlled.
A shortcut to express what should otherwise be through Control, remoteControl,RemoteUnit"""@en ;
  rdfs:domain next:ProtectedSwitchEx ;
  rdfs:isDefinedBy :Package_EDFExtensionsFunctional ;
  rdfs:range xsd:boolean ;
  uml:hasStereotype uml:attribute ;
  uml:id "EAID_A052F450_A377_432b_BE7F_F314549CC496" .

rdfs:comment a owl:AnnotationProperty ;
  rdfs:label "description", "documentation" ;
  uml:id "EAID_0445C12E_7D38_4f50_BF6D_99FD3A203143", "EAID_1699E23F_8411_4351_A573_4D126B4F01CE", "EAID_6BCD175E_328D_46e8_91AD_AC97399BFB53", "EAID_95ACFDE2_427F_4b8d_9C30_575783CB7FD0" .

uml:baseprefix a owl:AnnotationProperty .

uml:baseuri a owl:AnnotationProperty .

uml:hasInitialValue a owl:AnnotationProperty .

uml:hasMaxCardinality a owl:AnnotationProperty .

uml:hasMinCardinality a owl:AnnotationProperty .

uml:hasMultiplier a owl:AnnotationProperty .

uml:hasStereotype a owl:AnnotationProperty .

uml:hasUnits a owl:AnnotationProperty .

uml:id a owl:AnnotationProperty .

uml:roleALabel a owl:AnnotationProperty .

uml:roleAOf a owl:AnnotationProperty .

uml:roleBLabel a owl:AnnotationProperty .

uml:roleBOf a owl:AnnotationProperty .

uml:uriHasPrefix a owl:AnnotationProperty .

:Package_CDPSM2015_Versions a uml:Package ;
  rdfs:label "CDPSM2015_Versions" ;
  uml:baseuri "https://cim.ucaiug.io/ns#" ;
  uml:id "EAPK_28BCB051_6D19_4a4c_A476_FEFCD7150943" .

:Package_CIMDataTypes a uml:Package ;
  rdfs:label "CIMDataTypes" ;
  rdfs:isDefinedBy :Package_DataTypes ;
  uml:baseuri "https://cim.ucaiug.io/ns#" ;
  uml:id "EAPK_C17AEB8B_8DB4_4c39_96D7_03E08C4E5EB1" .

:Package_CIMEnumerations a uml:Package ;
  rdfs:label "CIMEnumerations" ;
  rdfs:isDefinedBy :Package_DataTypes ;
  uml:baseuri "https://cim.ucaiug.io/ns#" ;
  uml:id "EAPK_D246256B_B69C_47df_BDD3_52D0BDB191EB" .

:Package_CIMExtensions a uml:Package ;
  rdfs:label "CIMExtensions" ;
  rdfs:isDefinedBy :Package_Functional ;
  uml:baseuri "http://edf.fr/draft/cim17-ext#" ;
  uml:id "EAPK_910FC11B_2DDD_4691_89BA_A6FD3C3F154D" .

:Package_CompoundTypes a uml:Package ;
  rdfs:label "CompoundTypes" ;
  rdfs:isDefinedBy :Package_DataTypes ;
  uml:baseuri "https://cim.ucaiug.io/ns#" ;
  uml:id "EAPK_6F438211_9449_4fd0_AEF2_6A7898B85CE6" .

:Package_DataTypes a uml:Package ;
  rdfs:label "DataTypes" ;
  uml:baseuri "https://cim.ucaiug.io/ns#" ;
  uml:id "EAPK_4C6C1B78_A35E_4e1a_8FE7_00B567EEE34A" .

:Package_EDFExtensionsFunctional a uml:Package ;
  rdfs:label "EDFExtensionsFunctional" ;
  rdfs:isDefinedBy :Package_Functional ;
  uml:baseuri "http://der.edf.fr/mire/MSite-v3.1.a#" ;
  uml:id "EAPK_B53AFFAE_EE59_4443_A190_A78AD96DFEF7" .

:Package_EntsoeExtensions a uml:Package ;
  rdfs:label "EntsoeExtensions" ;
  rdfs:isDefinedBy :Package_DataTypes, :Package_Functional ;
  uml:baseuri "http://entsoe.eu/CIM/SchemaExtension/3/1#" ;
  uml:id "EAPK_5AA34A0A_7B1B_4772_96AF_359B62E14C2E", "EAPK_EE2998DE_07CF_4256_B7E6_3232BA2EEC47" .

:Package_Extensions a uml:Package ;
  rdfs:label "Extensions" ;
  rdfs:isDefinedBy :Package_CDPSM2015_Versions ;
  uml:baseuri "https://cim.ucaiug.io/ns#" ;
  uml:id "EAPK_CA794E24_0958_4a83_B276_9765B963AE7D" .

:Package_Feeder a uml:Package ;
  rdfs:label "Feeder" ;
  rdfs:isDefinedBy :Package_Standard ;
  uml:baseuri "https://cim.ucaiug.io/ns#" ;
  uml:id "EAPK_E7D01ED7_89ED_470e_A585_8F9F4EDFD181" .

:Package_Functional a uml:Package ;
  rdfs:label "Functional" ;
  uml:baseuri "https://cim.ucaiug.io/ns#" ;
  uml:id "EAPK_F25EAAE9_0909_48fb_9549_A9C6B54C1683" .

:Package_InfIEC61970 a uml:Package ;
  rdfs:label "InfIEC61970" ;
  rdfs:isDefinedBy :Package_Functional ;
  uml:baseuri "http://edf.fr/draft/cim17-info#" ;
  uml:id "EAPK_ED345C90_BD4C_4237_8E5F_56AFBE5B6193" .

:Package_ModelAuthority a uml:Package ;
  rdfs:label "ModelAuthority" ;
  rdfs:comment "The package describes meta data for partitioning  power system models into non overlapping subsets of objects managed by a model authority."@en ;
  uml:id "EAPK_FA58BD12_D4BA_4e34_A13E_A26DB6C4EF17" .

:Package_ModelDescription a uml:Package ;
  rdfs:label "ModelDescription" ;
  rdfs:comment "The package describes meta data for the exchange of power system model data."@en ;
  uml:baseuri "http://iec.ch/TC57/61970-552/ModelDescription/1#" ;
  uml:id "EAPK_1FE6534D_F250_4ef7_9343_02B5C21DB333" .

:Package_PowerSystemProject a uml:Package ;
  rdfs:label "PowerSystemProject" ;
  rdfs:comment "The package describes how power system model data is managed and evolve over time in projects."@en ;
  uml:id "EAPK_1813910E_9451_4ae3_BA8D_4DDFC1035E40" .

:Package_PrimitiveTypes a uml:Package ;
  rdfs:label "PrimitiveTypes" ;
  rdfs:isDefinedBy :Package_DataTypes ;
  uml:baseuri "https://cim.ucaiug.io/ns#" ;
  uml:id "EAPK_7B8DB810_3F0E_4dfd_9ED4_5ABBA3E9F7E1" .

:Package_Standard a uml:Package ;
  rdfs:label "Standard" ;
  rdfs:isDefinedBy :Package_Functional ;
  uml:baseuri "https://cim.ucaiug.io/ns#" ;
  uml:id "EAPK_48C40629_816E_4bae_930C_2855F73F4B2A" .

:URI a rdfs:Datatype ;
  rdfs:label "URI" ;
  uml:id "eaxmiid2" .

cim:ActivePower a rdfs:Datatype ;
  rdfs:label "ActivePower" ;
  rdfs:comment "Product of RMS value of the voltage and the RMS value of the in-phase component of the current."@en ;
  owl:equivalentClass xsd:float ;
  rdfs:isDefinedBy :Package_CIMDataTypes ;
  uml:hasMultiplier "M" ;
  uml:hasStereotype uml:cimdatatype ;
  uml:hasUnits "W" ;
  uml:id "EAID_9FDEB934_262D_4e7b_9551_75C9D20BA5C2" .

cim:ActivePowerPerCurrentFlow a rdfs:Datatype ;
  rdfs:label "ActivePowerPerCurrentFlow" ;
  owl:equivalentClass xsd:float ;
  rdfs:isDefinedBy :Package_CIMDataTypes ;
  uml:hasStereotype uml:cimdatatype ;
  uml:hasUnits "WPerA" ;
  uml:id "EAID_EF95FD0D_F934_44ee_94FC_E5318EDA6DB1" .

cim:ActivePowerPerFrequency a rdfs:Datatype ;
  rdfs:label "ActivePowerPerFrequency" ;
  rdfs:comment "Active power variation with frequency."@en ;
  owl:equivalentClass xsd:float ;
  rdfs:isDefinedBy :Package_CIMDataTypes ;
  uml:hasStereotype uml:cimdatatype ;
  uml:hasUnits "WPerHz" ;
  uml:id "EAID_3E3062AA_5BD3_43dd_9D18_3D96BCC10784" .

cim:AngleDegrees a rdfs:Datatype ;
  rdfs:label "AngleDegrees" ;
  rdfs:comment "Measurement of angle in degrees"@en ;
  owl:equivalentClass xsd:float ;
  rdfs:isDefinedBy :Package_CIMDataTypes ;
  uml:hasMultiplier "none" ;
  uml:hasStereotype uml:cimdatatype ;
  uml:hasUnits "deg" ;
  uml:id "EAID_8E77941D_A918_4ca6_B37B_2C3671D68B4D" .

cim:AngleRadians a rdfs:Datatype ;
  rdfs:label "AngleRadians" ;
  rdfs:comment "Phase angle in radians"@en ;
  owl:equivalentClass xsd:float ;
  rdfs:isDefinedBy :Package_CIMDataTypes ;
  uml:hasMultiplier "none" ;
  uml:hasStereotype uml:cimdatatype ;
  uml:hasUnits "rad" ;
  uml:id "EAID_A3F15E20_66CA_44bc_AD64_03BD90A30F48" .

cim:ApparentPower a rdfs:Datatype ;
  rdfs:label "ApparentPower" ;
  rdfs:comment "Product of the RMS value of the voltage and the RMS value of the current"@en ;
  owl:equivalentClass xsd:float ;
  rdfs:isDefinedBy :Package_CIMDataTypes ;
  uml:hasMultiplier "M" ;
  uml:hasStereotype uml:cimdatatype ;
  uml:hasUnits "VA" ;
  uml:id "EAID_42FA3B9C_DD19_4c11_B9D4_7C9BAA7BBAB0" .

cim:AssetModelUsageKind.customerSubstation a cim:AssetModelUsageKind ;
  rdfs:label "customerSubstation" ;
  rdfs:comment "Asset model is intended for use in customer substation."@en ;
  rdfs:isDefinedBy :Package_CIMEnumerations ;
  uml:id "EAID_451D749A_35B8_46d2_ACF1_0B1846EC4F16" .

cim:AssetModelUsageKind.distributionOverhead a cim:AssetModelUsageKind ;
  rdfs:label "distributionOverhead" ;
  rdfs:comment "Asset model is intended for use in distribution overhead network."@en ;
  rdfs:isDefinedBy :Package_CIMEnumerations ;
  uml:id "EAID_5400E932_09E5_49dd_85FB_51AD27E1712D" .

cim:AssetModelUsageKind.distributionUnderground a cim:AssetModelUsageKind ;
  rdfs:label "distributionUnderground" ;
  rdfs:comment "Asset model is intended for use in underground distribution network."@en ;
  rdfs:isDefinedBy :Package_CIMEnumerations ;
  uml:id "EAID_DD733D41_C7D4_4966_8072_47CB63BF3A0F" .

cim:AssetModelUsageKind.other a cim:AssetModelUsageKind ;
  rdfs:label "other" ;
  rdfs:comment "Other kind of asset model usage."@en ;
  rdfs:isDefinedBy :Package_CIMEnumerations ;
  uml:id "EAID_13EBDC0B_CF44_4b89_9BEB_85CF9D6DC67E" .

cim:AssetModelUsageKind.streetlight a cim:AssetModelUsageKind ;
  rdfs:label "streetlight" ;
  rdfs:comment "Asset model is intended for use as streetlight."@en ;
  rdfs:isDefinedBy :Package_CIMEnumerations ;
  uml:id "EAID_641028DE_403E_4bb9_8B7F_39B620D4F3FC" .

cim:AssetModelUsageKind.substation a cim:AssetModelUsageKind ;
  rdfs:label "substation" ;
  rdfs:comment "Asset model is intended for use in substation."@en ;
  rdfs:isDefinedBy :Package_CIMEnumerations ;
  uml:id "EAID_CF8F68FF_8613_469b_8A5B_A58FD4F7F700" .

cim:AssetModelUsageKind.transmission a cim:AssetModelUsageKind ;
  rdfs:label "transmission" ;
  rdfs:comment "Asset model is intended for use in transmission network."@en ;
  rdfs:isDefinedBy :Package_CIMEnumerations ;
  uml:id "EAID_64CBD772_2ABF_417b_8980_C446B73E3E04" .

cim:AssetModelUsageKind.unknown a cim:AssetModelUsageKind ;
  rdfs:label "unknown" ;
  rdfs:comment "Usage of the asset model is unknown."@en ;
  rdfs:isDefinedBy :Package_CIMEnumerations ;
  uml:id "EAID_87E82A02_3DC6_45d2_B406_BC4825202653" .

cim:AsynchronousMachineKind.generator a cim:AsynchronousMachineKind ;
  rdfs:label "generator" ;
  rdfs:comment "The Asynchronous Machine is a generator."@en ;
  rdfs:isDefinedBy :Package_CIMEnumerations ;
  uml:id "EAID_48ECF68C_AA4D_41a2_93AC_7C4AE196D72C" .

cim:AsynchronousMachineKind.motor a cim:AsynchronousMachineKind ;
  rdfs:label "motor" ;
  rdfs:comment "The Asynchronous Machine is a motor."@en ;
  rdfs:isDefinedBy :Package_CIMEnumerations ;
  uml:id "EAID_D1B93705_F30F_4184_BF0B_FC18CB4858D7" .

cim:CableConstructionKind.compacted a cim:CableConstructionKind ;
  rdfs:label "compacted" ;
  rdfs:isDefinedBy :Package_CIMEnumerations ;
  uml:id "EAID_C0717798_61AF_4496_8BA8_38D10255C7A9" .

cim:CableConstructionKind.compressed a cim:CableConstructionKind ;
  rdfs:label "compressed" ;
  rdfs:isDefinedBy :Package_CIMEnumerations ;
  uml:id "EAID_FA9CFB9A_9F62_4cbc_8C2A_81D004AAA4E4" .

cim:CableConstructionKind.other a cim:CableConstructionKind ;
  rdfs:label "other" ;
  rdfs:isDefinedBy :Package_CIMEnumerations ;
  uml:id "EAID_CEB1C1A6_B7A6_4c99_B25C_6B66983FD648" .

cim:CableConstructionKind.sector a cim:CableConstructionKind ;
  rdfs:label "sector" ;
  rdfs:isDefinedBy :Package_CIMEnumerations ;
  uml:id "EAID_99FC9376_9C9C_4bc7_8B39_E62604FCCFA7" .

cim:CableConstructionKind.segmental a cim:CableConstructionKind ;
  rdfs:label "segmental" ;
  rdfs:isDefinedBy :Package_CIMEnumerations ;
  uml:id "EAID_2E3FB6B0_CEC7_4600_92D4_A462B3FDDBFA" .

cim:CableConstructionKind.solid a cim:CableConstructionKind ;
  rdfs:label "solid" ;
  rdfs:isDefinedBy :Package_CIMEnumerations ;
  uml:id "EAID_CF90FB65_CD5F_4633_98EB_C464FD91647D" .

cim:CableConstructionKind.stranded a cim:CableConstructionKind ;
  rdfs:label "stranded" ;
  rdfs:isDefinedBy :Package_CIMEnumerations ;
  uml:id "EAID_BBCF9A7A_9F9C_45a8_9F2A_0456347BF6B5" .

cim:CableOuterJacketKind.insulating a cim:CableOuterJacketKind ;
  rdfs:label "insulating" ;
  rdfs:isDefinedBy :Package_CIMEnumerations ;
  uml:id "EAID_2BB5ADE6_DA74_4393_971F_04230E58B706" .

cim:CableOuterJacketKind.linearLowDensityPolyethylene a cim:CableOuterJacketKind ;
  rdfs:label "linearLowDensityPolyethylene" ;
  rdfs:isDefinedBy :Package_CIMEnumerations ;
  uml:id "EAID_8CD68AED_196B_4cd5_B2D0_18699B55ACC8" .

cim:CableOuterJacketKind.none a cim:CableOuterJacketKind ;
  rdfs:label "none" ;
  rdfs:isDefinedBy :Package_CIMEnumerations ;
  uml:id "EAID_348F20DD_324D_475f_A5A9_D0CA956ED5BE" .

cim:CableOuterJacketKind.other a cim:CableOuterJacketKind ;
  rdfs:label "other" ;
  rdfs:isDefinedBy :Package_CIMEnumerations ;
  uml:id "EAID_F2278A86_0174_4eab_B8F8_77A16EC9F3D4" .

cim:CableOuterJacketKind.polyethylene a cim:CableOuterJacketKind ;
  rdfs:label "polyethylene" ;
  rdfs:isDefinedBy :Package_CIMEnumerations ;
  uml:id "EAID_EBB5CF78_2E47_4b11_92AF_781E4B6C112A" .

cim:CableOuterJacketKind.pvc a cim:CableOuterJacketKind ;
  rdfs:label "pvc" ;
  rdfs:isDefinedBy :Package_CIMEnumerations ;
  uml:id "EAID_7F6A242E_80BC_43c9_B2BB_7C3C457AEC2F" .

cim:CableOuterJacketKind.semiconducting a cim:CableOuterJacketKind ;
  rdfs:label "semiconducting" ;
  rdfs:isDefinedBy :Package_CIMEnumerations ;
  uml:id "EAID_CE02D32E_12DE_4f93_AA13_529DB2C22FAD" .

cim:CableShieldMaterialKind.aluminum a cim:CableShieldMaterialKind ;
  rdfs:label "aluminum" ;
  rdfs:isDefinedBy :Package_CIMEnumerations ;
  uml:id "EAID_27223C05_A901_477e_9A43_A318054B08CD" .

cim:CableShieldMaterialKind.copper a cim:CableShieldMaterialKind ;
  rdfs:label "copper" ;
  rdfs:isDefinedBy :Package_CIMEnumerations ;
  uml:id "EAID_46872655_CF94_4810_9F51_DFE4C1E1F792" .

cim:CableShieldMaterialKind.lead a cim:CableShieldMaterialKind ;
  rdfs:label "lead" ;
  rdfs:isDefinedBy :Package_CIMEnumerations ;
  uml:id "EAID_16A14442_8C0F_44cb_B4E9_258923FC2C6E" .

cim:CableShieldMaterialKind.other a cim:CableShieldMaterialKind ;
  rdfs:label "other" ;
  rdfs:isDefinedBy :Package_CIMEnumerations ;
  uml:id "EAID_93554E7F_79B3_41e1_9550_D9375B247B4D" .

cim:CableShieldMaterialKind.steel a cim:CableShieldMaterialKind ;
  rdfs:label "steel" ;
  rdfs:isDefinedBy :Package_CIMEnumerations ;
  uml:id "EAID_BD9D47D6_7A5F_4716_9A6F_4C150CC3BB54" .

cim:Capacitance a rdfs:Datatype ;
  rdfs:label "Capacitance" ;
  rdfs:comment "Capacitive part of reactance (imaginary part of impedance), at rated frequency."@en ;
  owl:equivalentClass xsd:float ;
  rdfs:isDefinedBy :Package_CIMDataTypes ;
  uml:hasMultiplier "none" ;
  uml:hasStereotype uml:cimdatatype ;
  uml:hasUnits "F" ;
  uml:id "EAID_5C5D9592_92D6_4e93_BAD5_32AEFCC3A33E" .

cim:Conductance a rdfs:Datatype ;
  rdfs:label "Conductance" ;
  rdfs:comment "Factor by which voltage must be multiplied to give corresponding power lost from a circuit. Real part of admittance."@en ;
  owl:equivalentClass xsd:float ;
  rdfs:isDefinedBy :Package_CIMDataTypes ;
  uml:hasMultiplier "none" ;
  uml:hasStereotype uml:cimdatatype ;
  uml:hasUnits "S" ;
  uml:id "EAID_2D9C2F58_EAA8_4657_82BE_EF3D0ED215BA" .

cim:ConductancePerLength a rdfs:Datatype ;
  rdfs:label "ConductancePerLength" ;
  rdfs:comment "Real part of admittance per unit of length."@en ;
  owl:equivalentClass xsd:float ;
  rdfs:isDefinedBy :Package_CIMDataTypes ;
  uml:hasMultiplier "none" ;
  uml:hasStereotype uml:cimdatatype ;
  uml:hasUnits "SPerm" ;
  uml:id "EAID_C18C3C34_C763_4d73_8F43_E10FC386C747" .

cim:CurrentFlow a rdfs:Datatype ;
  rdfs:label "CurrentFlow" ;
  rdfs:comment "Electrical current (positive flow is out of the ConductingEquipment into the ConnectivityNode)"@en ;
  owl:equivalentClass xsd:float ;
  rdfs:isDefinedBy :Package_CIMDataTypes ;
  uml:hasMultiplier "none" ;
  uml:hasStereotype uml:cimdatatype ;
  uml:hasUnits "A" ;
  uml:id "EAID_773E16D8_9DF8_426e_BF97_853428CF78C2" .

cim:CurveStyle.constantYValue a cim:CurveStyle ;
  rdfs:label "constantYValue" ;
  rdfs:comment "The Y-axis values are assumed constant until the next curve point and prior to the first curve point."@en ;
  rdfs:isDefinedBy :Package_CIMEnumerations ;
  uml:id "EAID_FFC73338_9482_461e_9CCE_E8396F4793FB" .

cim:CurveStyle.straightLineYValues a cim:CurveStyle ;
  rdfs:label "straightLineYValues" ;
  rdfs:comment "The Y-axis values are assumed to be a straight line between values.  Also known as linear interpolation."@en ;
  rdfs:isDefinedBy :Package_CIMEnumerations ;
  uml:id "EAID_419C93CE_8818_4c89_AB63_BE01921FE30D" .

cim:Displacement a rdfs:Datatype ;
  rdfs:label "Displacement" ;
  rdfs:comment "Unit of displacement relative a reference position, hence can be negative."@en ;
  owl:equivalentClass xsd:float ;
  rdfs:isDefinedBy :Package_CIMDataTypes ;
  uml:hasMultiplier "none" ;
  uml:hasStereotype uml:cimdatatype ;
  uml:hasUnits "m" ;
  uml:id "EAID_FB005E54_4701_40e6_91DA_831E171484D9" .

cim:Frequency a rdfs:Datatype ;
  rdfs:label "Frequency" ;
  rdfs:comment "Cycles per second"@en ;
  owl:equivalentClass xsd:float ;
  rdfs:isDefinedBy :Package_CIMDataTypes ;
  uml:hasMultiplier "none" ;
  uml:hasStereotype uml:cimdatatype ;
  uml:hasUnits "Hz" ;
  uml:id "EAID_56ECB3D9_7270_43de_B868_B58829BE32E3" .

cim:GeneratorControlSource.offAGC a cim:GeneratorControlSource ;
  rdfs:label "offAGC" ;
  rdfs:isDefinedBy :Package_CIMEnumerations ;
  uml:id "EAID_9B681FE4_4EFB_4189_8B15_04468E5A4E44" .

cim:GeneratorControlSource.onAGC a cim:GeneratorControlSource ;
  rdfs:label "onAGC" ;
  rdfs:isDefinedBy :Package_CIMEnumerations ;
  uml:id "EAID_BC2966CC_CA2E_4bc9_B468_0A57C6ACB21D" .

cim:GeneratorControlSource.plantControl a cim:GeneratorControlSource ;
  rdfs:label "plantControl" ;
  rdfs:isDefinedBy :Package_CIMEnumerations ;
  uml:id "EAID_81877073_0748_4220_B78E_718AA49C7C7D" .

cim:GeneratorControlSource.unavailable a cim:GeneratorControlSource ;
  rdfs:label "unavailable" ;
  rdfs:isDefinedBy :Package_CIMEnumerations ;
  uml:id "EAID_CBE18143_8ADE_4074_906E_6157C49E8F73" .

cim:HydroPlantStorageKind.pumpedStorage a cim:HydroPlantStorageKind ;
  rdfs:label "pumpedStorage" ;
  rdfs:comment "Pumped storage."@en ;
  rdfs:isDefinedBy :Package_CIMEnumerations ;
  uml:id "EAID_02F84625_D5BF_466e_A802_4B000C3FEA03" .

cim:HydroPlantStorageKind.runOfRiver a cim:HydroPlantStorageKind ;
  rdfs:label "runOfRiver" ;
  rdfs:comment "Run of river."@en ;
  rdfs:isDefinedBy :Package_CIMEnumerations ;
  uml:id "EAID_D976AA49_42B9_456a_9FC9_4DB3058DCD4D" .

cim:HydroPlantStorageKind.storage a cim:HydroPlantStorageKind ;
  rdfs:label "storage" ;
  rdfs:comment "Storage."@en ;
  rdfs:isDefinedBy :Package_CIMEnumerations ;
  uml:id "EAID_2BE1561B_3DF2_41d7_BD06_39C870998D6E" .

cim:Impedance a rdfs:Datatype ;
  rdfs:label "Impedance" ;
  rdfs:comment "Ratio of voltage to current."@en ;
  owl:equivalentClass xsd:float ;
  rdfs:isDefinedBy :Package_CIMDataTypes ;
  uml:hasMultiplier "none" ;
  uml:hasStereotype uml:cimdatatype ;
  uml:hasUnits "ohm" ;
  uml:id "EAID_4BA91B36_C874_42f0_BC71_222AFD772FE6" .

cim:Inductance a rdfs:Datatype ;
  rdfs:label "Inductance" ;
  rdfs:comment "Inductance."@en ;
  owl:equivalentClass xsd:float ;
  rdfs:isDefinedBy :Package_CIMDataTypes ;
  uml:hasMultiplier "none" ;
  uml:hasStereotype uml:cimdatatype ;
  uml:hasUnits "H" ;
  uml:id "EAID_2DAF36DA_B9EC_4a29_AF09_6CF5F22E0F39" .

cim:KiloActivePower a rdfs:Datatype ;
  rdfs:label "KiloActivePower" ;
  rdfs:comment "Active power in kilowatts."@en ;
  owl:equivalentClass xsd:float ;
  rdfs:isDefinedBy :Package_CIMDataTypes ;
  uml:hasMultiplier "k" ;
  uml:hasStereotype uml:cimdatatype ;
  uml:hasUnits "W" ;
  uml:id "EAID_9DA985D0_F816_45e4_B16D_1C9443499FC4" .

cim:Length a rdfs:Datatype ;
  rdfs:label "Length" ;
  rdfs:comment "Unit of length."@en ;
  owl:equivalentClass xsd:float ;
  rdfs:isDefinedBy :Package_CIMDataTypes ;
  uml:hasMultiplier "none" ;
  uml:hasStereotype uml:cimdatatype ;
  uml:hasUnits "m" ;
  uml:id "EAID_3957F899_DF24_4f2b_9800_255B6433079C" .

cim:MonthDay a rdfs:Datatype ;
  rdfs:label "MonthDay" ;
  rdfs:comment "MonthDay format as \"--mm-dd\", which conforms with XSD data type gMonthDay."@en ;
  rdfs:isDefinedBy :Package_PrimitiveTypes ;
  uml:hasStereotype uml:primitive ;
  uml:id "EAID_83956FD6_B8C0_480f_AB7D_ED3C03B8124A" .

cim:OperationalLimitDirectionKind.absoluteValue a cim:OperationalLimitDirectionKind ;
  rdfs:label "absoluteValue" ;
  rdfs:comment "An absoluteValue limit means that a monitored absolute value above the limit value is a violation."@en ;
  rdfs:isDefinedBy :Package_CIMEnumerations ;
  uml:id "EAID_8E09B578_BBFF_4092_BF37_53C1F42A9429" .

cim:OperationalLimitDirectionKind.high a cim:OperationalLimitDirectionKind ;
  rdfs:label "high" ;
  rdfs:comment "High means that a monitored value above the limit value is a violation.   If applied to a terminal flow, the positive direction is into the terminal."@en ;
  rdfs:isDefinedBy :Package_CIMEnumerations ;
  uml:id "EAID_55F0B56D_2715_45fd_B494_E78450B8FE51" .

cim:OperationalLimitDirectionKind.low a cim:OperationalLimitDirectionKind ;
  rdfs:label "low" ;
  rdfs:comment "Low means a monitored value below the limit is a violation.  If applied to a terminal flow, the positive direction is into the terminal."@en ;
  rdfs:isDefinedBy :Package_CIMEnumerations ;
  uml:id "EAID_D7E34FE7_5F5F_4d22_B14A_9FB9459033A8" .

cim:OrientationKind.negative a cim:OrientationKind ;
  rdfs:label "negative" ;
  rdfs:comment "For 2D diagrams, a negative orientation gives the left-hand orientation (favoured by computer graphics displays) with X values increasing from left to right and Y values increasing from top to bottom.   This is also known as a left hand orientation."@en ;
  rdfs:isDefinedBy :Package_CIMEnumerations ;
  uml:id "EAID_83B1FCEC_F370_4286_958D_530C1B06B4A8" .

cim:OrientationKind.positive a cim:OrientationKind ;
  rdfs:label "positive" ;
  rdfs:comment "For 2D diagrams, a positive orientation will result in X values increasing from left to right and Y values increasing from bottom to top.  This is also known as a right hand orientation."@en ;
  rdfs:isDefinedBy :Package_CIMEnumerations ;
  uml:id "EAID_DE6A1FBB_1A91_41a9_8505_B6954F7E55B3" .

cim:PSREventKind.inService a cim:PSREventKind ;
  rdfs:label "inService" ;
  rdfs:comment "Power system resource state change to in service."@en ;
  rdfs:isDefinedBy :Package_CIMEnumerations ;
  uml:id "EAID_980B47DD_1501_466b_A527_889EDA30BA04" .

cim:PSREventKind.other a cim:PSREventKind ;
  rdfs:label "other" ;
  rdfs:comment "Other power system resource state change."@en ;
  rdfs:isDefinedBy :Package_CIMEnumerations ;
  uml:id "EAID_D78F1B92_633C_4d84_A16A_680AAEAC7DD4" .

cim:PSREventKind.outOfService a cim:PSREventKind ;
  rdfs:label "outOfService" ;
  rdfs:comment "Power system resource state change to out of service."@en ;
  rdfs:isDefinedBy :Package_CIMEnumerations ;
  uml:id "EAID_93ED4D01_62F2_4f61_A295_51F30E4E6350" .

cim:PSREventKind.pendingAdd a cim:PSREventKind ;
  rdfs:label "pendingAdd" ;
  rdfs:comment "Power system resource state change to pending add."@en ;
  rdfs:isDefinedBy :Package_CIMEnumerations ;
  uml:id "EAID_4F4B64B4_FE91_4811_84EE_6412E8E06917" .

cim:PSREventKind.pendingRemove a cim:PSREventKind ;
  rdfs:label "pendingRemove" ;
  rdfs:comment "Power system resource state change to pending remove."@en ;
  rdfs:isDefinedBy :Package_CIMEnumerations ;
  uml:id "EAID_0C0E4C88_6E79_459c_81B3_44111E00022C" .

cim:PSREventKind.pendingReplace a cim:PSREventKind ;
  rdfs:label "pendingReplace" ;
  rdfs:comment "Power system resource state change to pending replace."@en ;
  rdfs:isDefinedBy :Package_CIMEnumerations ;
  uml:id "EAID_9C71A044_A673_4f60_A2BE_1C5B7156E786" .

cim:PSREventKind.unknown a cim:PSREventKind ;
  rdfs:label "unknown" ;
  rdfs:comment "Unknown power system resource state change."@en ;
  rdfs:isDefinedBy :Package_CIMEnumerations ;
  uml:id "EAID_95F1E3E1_029C_458a_A504_EE84D4D543A1" .

cim:PU a rdfs:Datatype ;
  rdfs:label "PU" ;
  rdfs:comment "Per Unit - a positive or negative value referred to a defined base. Values typically range from -10 to +10."@en ;
  owl:equivalentClass xsd:float ;
  rdfs:isDefinedBy :Package_CIMDataTypes ;
  uml:hasMultiplier "none" ;
  uml:hasStereotype uml:cimdatatype ;
  uml:hasUnits "none" ;
  uml:id "EAID_B95B85BC_F780_44a7_9FA5_230945D6D405" .

cim:PerCent a rdfs:Datatype ;
  rdfs:label "PerCent" ;
  rdfs:comment "Normally 0 - 100 on a defined base"@en ;
  owl:equivalentClass xsd:float ;
  rdfs:isDefinedBy :Package_CIMDataTypes ;
  uml:hasMultiplier "none" ;
  uml:hasStereotype uml:cimdatatype ;
  uml:hasUnits "none" ;
  uml:id "EAID_7D7C80E0_6F8B_4edb_A772_B9E3A8BC10B1" .

cim:PhaseCode.A a cim:PhaseCode ;
  rdfs:label "A" ;
  rdfs:comment "Phase A."@en ;
  rdfs:isDefinedBy :Package_CIMEnumerations ;
  uml:id "EAID_DA8D8889_2672_43a0_9C5B_8B41C1685CF0" .

cim:PhaseCode.AB a cim:PhaseCode ;
  rdfs:label "AB" ;
  rdfs:comment "Phases A and B."@en ;
  rdfs:isDefinedBy :Package_CIMEnumerations ;
  uml:id "EAID_C2D378B0_1CC6_42b9_BAD1_4D0FC944338C" .

cim:PhaseCode.ABC a cim:PhaseCode ;
  rdfs:label "ABC" ;
  rdfs:comment "Phases A, B, and C."@en ;
  rdfs:isDefinedBy :Package_CIMEnumerations ;
  uml:id "EAID_1E471668_30E7_4bfa_809B_49A962CFF418" .

cim:PhaseCode.ABCN a cim:PhaseCode ;
  rdfs:label "ABCN" ;
  rdfs:comment "Phases A, B, C, and N."@en ;
  rdfs:isDefinedBy :Package_CIMEnumerations ;
  uml:id "EAID_8A6E5842_BB8C_4e01_8606_3F461DE8C5D0" .

cim:PhaseCode.ABN a cim:PhaseCode ;
  rdfs:label "ABN" ;
  rdfs:comment "Phases A, B, and neutral."@en ;
  rdfs:isDefinedBy :Package_CIMEnumerations ;
  uml:id "EAID_4B392DBC_EE18_4978_A1A7_419604B59AAD" .

cim:PhaseCode.AC a cim:PhaseCode ;
  rdfs:label "AC" ;
  rdfs:comment "Phases A and C."@en ;
  rdfs:isDefinedBy :Package_CIMEnumerations ;
  uml:id "EAID_CB0F6C14_5343_4697_91AD_586CFAF714A5" .

cim:PhaseCode.ACN a cim:PhaseCode ;
  rdfs:label "ACN" ;
  rdfs:comment "Phases A, C and neutral."@en ;
  rdfs:isDefinedBy :Package_CIMEnumerations ;
  uml:id "EAID_FABAE345_1D4E_471a_8834_6AE0B42EE2ED" .

cim:PhaseCode.AN a cim:PhaseCode ;
  rdfs:label "AN" ;
  rdfs:comment "Phases A and neutral."@en ;
  rdfs:isDefinedBy :Package_CIMEnumerations ;
  uml:id "EAID_A2322207_4C93_4111_9B2F_3AE95D68B826" .

cim:PhaseCode.B a cim:PhaseCode ;
  rdfs:label "B" ;
  rdfs:comment "Phase B."@en ;
  rdfs:isDefinedBy :Package_CIMEnumerations ;
  uml:id "EAID_FCAA2C0A_22BE_444d_BDBF_970246E69C58" .

cim:PhaseCode.BC a cim:PhaseCode ;
  rdfs:label "BC" ;
  rdfs:comment "Phases B and C."@en ;
  rdfs:isDefinedBy :Package_CIMEnumerations ;
  uml:id "EAID_D42E600C_F3C4_4230_A063_C00048897B7A" .

cim:PhaseCode.BCN a cim:PhaseCode ;
  rdfs:label "BCN" ;
  rdfs:comment "Phases B, C, and neutral."@en ;
  rdfs:isDefinedBy :Package_CIMEnumerations ;
  uml:id "EAID_FABE2547_CACC_4cd6_8351_77FA867EBE9C" .

cim:PhaseCode.BN a cim:PhaseCode ;
  rdfs:label "BN" ;
  rdfs:comment "Phases B and neutral."@en ;
  rdfs:isDefinedBy :Package_CIMEnumerations ;
  uml:id "EAID_995787A5_B742_4a0e_9466_46E63D6B5061" .

cim:PhaseCode.C a cim:PhaseCode ;
  rdfs:label "C" ;
  rdfs:comment "Phase C."@en ;
  rdfs:isDefinedBy :Package_CIMEnumerations ;
  uml:id "EAID_8611466E_A157_4815_AEC3_4AA783A3AE39" .

cim:PhaseCode.CN a cim:PhaseCode ;
  rdfs:label "CN" ;
  rdfs:comment "Phases C and neutral."@en ;
  rdfs:isDefinedBy :Package_CIMEnumerations ;
  uml:id "EAID_9B346D24_2794_4ad5_AB0F_A6807FEB2A1B" .

cim:PhaseCode.N a cim:PhaseCode ;
  rdfs:label "N" ;
  rdfs:comment "Neutral phase."@en ;
  rdfs:isDefinedBy :Package_CIMEnumerations ;
  uml:id "EAID_1CE522F3_6334_48e8_870E_ACD413EF9BC1" .

cim:PhaseCode.X a cim:PhaseCode ;
  rdfs:label "X" ;
  rdfs:comment "Unknown non-neutral phase."@en ;
  rdfs:isDefinedBy :Package_CIMEnumerations ;
  uml:id "EAID_D69AC548_42A5_4933_BA3A_92954DACD646" .

cim:PhaseCode.XN a cim:PhaseCode ;
  rdfs:label "XN" ;
  rdfs:comment "Unknown non-neutral phase plus neutral."@en ;
  rdfs:isDefinedBy :Package_CIMEnumerations ;
  uml:id "EAID_0814677D_555E_4964_BD82_04622C6CCA19" .

cim:PhaseCode.XY a cim:PhaseCode ;
  rdfs:label "XY" ;
  rdfs:comment "Two unknown non-neutral phases."@en ;
  rdfs:isDefinedBy :Package_CIMEnumerations ;
  uml:id "EAID_B223C117_334E_4d72_B952_FDB86AB35EDE" .

cim:PhaseCode.XYN a cim:PhaseCode ;
  rdfs:label "XYN" ;
  rdfs:comment "Two unknown non-neutral phases plus neutral."@en ;
  rdfs:isDefinedBy :Package_CIMEnumerations ;
  uml:id "EAID_56602A0D_B4C0_445c_B37D_E1BDA94BB926" .

cim:PhaseCode.none a cim:PhaseCode ;
  rdfs:label "none" ;
  rdfs:comment "No phases specified."@en ;
  rdfs:isDefinedBy :Package_CIMEnumerations ;
  uml:id "EAID_52D79C11_0C1C_4160_BEF7_697F7DF934C7" .

cim:PhaseCode.s1 a cim:PhaseCode ;
  rdfs:label "s1" ;
  rdfs:comment "Secondary phase 1."@en ;
  rdfs:isDefinedBy :Package_CIMEnumerations ;
  uml:id "EAID_C49EC80B_B8C4_4c15_A8DF_EBEFCA1F71E3" .

cim:PhaseCode.s12 a cim:PhaseCode ;
  rdfs:label "s12" ;
  rdfs:comment "Secondary phase 1 and 2."@en ;
  rdfs:isDefinedBy :Package_CIMEnumerations ;
  uml:id "EAID_363287F6_BC54_477b_A9B5_99C64490742C" .

cim:PhaseCode.s12N a cim:PhaseCode ;
  rdfs:label "s12N" ;
  rdfs:comment "Secondary phases 1, 2, and neutral."@en ;
  rdfs:isDefinedBy :Package_CIMEnumerations ;
  uml:id "EAID_D2B0CAFC_BDB5_413b_910B_79C398C4F267" .

cim:PhaseCode.s1N a cim:PhaseCode ;
  rdfs:label "s1N" ;
  rdfs:comment "Secondary phase 1 and neutral."@en ;
  rdfs:isDefinedBy :Package_CIMEnumerations ;
  uml:id "EAID_BF0EA903_4E83_438b_8B23_85939CB1FC35" .

cim:PhaseCode.s2 a cim:PhaseCode ;
  rdfs:label "s2" ;
  rdfs:comment "Secondary phase 2."@en ;
  rdfs:isDefinedBy :Package_CIMEnumerations ;
  uml:id "EAID_C98B6AF7_876C_462c_A09F_07F3A44EBE0D" .

cim:PhaseCode.s2N a cim:PhaseCode ;
  rdfs:label "s2N" ;
  rdfs:comment "Secondary phase 2 and neutral."@en ;
  rdfs:isDefinedBy :Package_CIMEnumerations ;
  uml:id "EAID_B859D225_16B7_4cf4_B648_30154EB4E959" .

cim:RE_UnitMultiplier.G a cim:RE_UnitMultiplier ;
  rdfs:label "G" ;
  rdfs:comment "Giga 10**9"@en ;
  rdfs:isDefinedBy :Package_CIMEnumerations ;
  uml:id "EAID_CD30195D_01AD_4731_BC64_4DAB4FEB34C2" .

cim:RE_UnitMultiplier.M a cim:RE_UnitMultiplier ;
  rdfs:label "M" ;
  rdfs:comment "Mega 10**6"@en ;
  rdfs:isDefinedBy :Package_CIMEnumerations ;
  uml:id "EAID_3D4E19C6_4FA3_417a_9A64_58F651496443" .

cim:RE_UnitMultiplier.T a cim:RE_UnitMultiplier ;
  rdfs:label "T" ;
  rdfs:comment "Tera 10**12"@en ;
  rdfs:isDefinedBy :Package_CIMEnumerations ;
  uml:id "EAID_6441E4ED_2DB7_4bf9_9947_F7BBF541CDE2" .

cim:RE_UnitMultiplier.c a cim:RE_UnitMultiplier ;
  rdfs:label "c" ;
  rdfs:comment "Centi 10**-2"@en ;
  rdfs:isDefinedBy :Package_CIMEnumerations ;
  uml:id "EAID_33523CA1_9FBB_4dda_A41F_8CCD01A705E3" .

cim:RE_UnitMultiplier.d a cim:RE_UnitMultiplier ;
  rdfs:label "d" ;
  rdfs:comment "Deci 10**-1"@en ;
  rdfs:isDefinedBy :Package_CIMEnumerations ;
  uml:id "EAID_2C6B01E8_EE7F_47b4_B17A_D52718E9FDB5" .

cim:RE_UnitMultiplier.k a cim:RE_UnitMultiplier ;
  rdfs:label "k" ;
  rdfs:comment "Kilo 10**3"@en ;
  rdfs:isDefinedBy :Package_CIMEnumerations ;
  uml:id "EAID_FC3463E2_B7B7_42df_ADC4_0DDCB4417F47" .

cim:RE_UnitMultiplier.m a cim:RE_UnitMultiplier ;
  rdfs:label "m" ;
  rdfs:comment "Milli 10**-3"@en ;
  rdfs:isDefinedBy :Package_CIMEnumerations ;
  uml:id "EAID_333CE2A7_BC1E_48f5_8955_8705073ABD46" .

cim:RE_UnitMultiplier.micro a cim:RE_UnitMultiplier ;
  rdfs:label "micro" ;
  rdfs:comment "Micro 10**-6"@en ;
  rdfs:isDefinedBy :Package_CIMEnumerations ;
  uml:id "EAID_D5C77816_5F76_44ca_AE11_4404B1C626CE" .

cim:RE_UnitMultiplier.n a cim:RE_UnitMultiplier ;
  rdfs:label "n" ;
  rdfs:comment "Nano 10**-9"@en ;
  rdfs:isDefinedBy :Package_CIMEnumerations ;
  uml:id "EAID_A51AD183_AF2F_4128_95DB_53F4363F6E20" .

cim:RE_UnitMultiplier.none a cim:RE_UnitMultiplier ;
  rdfs:label "none" ;
  rdfs:isDefinedBy :Package_CIMEnumerations ;
  uml:id "EAID_3C34E45A_34BC_4055_8DB3_552E3F1DB230" .

cim:RE_UnitMultiplier.p a cim:RE_UnitMultiplier ;
  rdfs:label "p" ;
  rdfs:comment "Pico 10**-12"@en ;
  rdfs:isDefinedBy :Package_CIMEnumerations ;
  uml:id "EAID_DCAC6BAA_8A53_441b_AB8E_7211863F9C0B" .

cim:RE_UnitSymbol.A a cim:RE_UnitSymbol ;
  rdfs:label "A" ;
  rdfs:comment "Current in ampere"@en ;
  rdfs:isDefinedBy :Package_CIMEnumerations ;
  uml:id "EAID_1D066952_C39F_4ab3_A500_001D3487B377" .

cim:RE_UnitSymbol.F a cim:RE_UnitSymbol ;
  rdfs:label "F" ;
  rdfs:comment "Capacitance in farad"@en ;
  rdfs:isDefinedBy :Package_CIMEnumerations ;
  uml:id "EAID_9C4F2B00_7A94_47f1_AE53_8D57669E9234" .

cim:RE_UnitSymbol.H a cim:RE_UnitSymbol ;
  rdfs:label "H" ;
  rdfs:comment "Inductance in henry"@en ;
  rdfs:isDefinedBy :Package_CIMEnumerations ;
  uml:id "EAID_349F9A6B_85C9_48ef_A9A4_2178DCA64AAF" .

cim:RE_UnitSymbol.Hz a cim:RE_UnitSymbol ;
  rdfs:label "Hz" ;
  rdfs:comment "Frequency in hertz"@en ;
  rdfs:isDefinedBy :Package_CIMEnumerations ;
  uml:id "EAID_58CA784B_0269_4106_97FA_F5EB062AFFB9" .

cim:RE_UnitSymbol.J a cim:RE_UnitSymbol ;
  rdfs:label "J" ;
  rdfs:comment "Energy in joule"@en ;
  rdfs:isDefinedBy :Package_CIMEnumerations ;
  uml:id "EAID_C7326BBD_7290_481f_9500_1C58C3A0681F" .

cim:RE_UnitSymbol.N a cim:RE_UnitSymbol ;
  rdfs:label "N" ;
  rdfs:comment "Force in newton"@en ;
  rdfs:isDefinedBy :Package_CIMEnumerations ;
  uml:id "EAID_EB9F7450_2A34_41ad_A957_198C340CB7EC" .

cim:RE_UnitSymbol.Pa a cim:RE_UnitSymbol ;
  rdfs:label "Pa" ;
  rdfs:comment "Pressure in pascal (n/m2)"@en ;
  rdfs:isDefinedBy :Package_CIMEnumerations ;
  uml:id "EAID_8EE37224_377D_4e72_8043_C3FC38B2E352" .

cim:RE_UnitSymbol.S a cim:RE_UnitSymbol ;
  rdfs:label "S" ;
  rdfs:comment "Conductance in siemens"@en ;
  rdfs:isDefinedBy :Package_CIMEnumerations ;
  uml:id "EAID_330922ED_3925_477b_BFAF_D7535B654A0F" .

cim:RE_UnitSymbol.V a cim:RE_UnitSymbol ;
  rdfs:label "V" ;
  rdfs:comment "Voltage in volt"@en ;
  rdfs:isDefinedBy :Package_CIMEnumerations ;
  uml:id "EAID_C6839724_BD18_4045_A3BA_A580EC9F9B4B" .

cim:RE_UnitSymbol.VA a cim:RE_UnitSymbol ;
  rdfs:label "VA" ;
  rdfs:comment "Apparent power in volt ampere"@en ;
  rdfs:isDefinedBy :Package_CIMEnumerations ;
  uml:id "EAID_7A46A41D_3A37_4a42_A6AA_BF9BD2164E23" .

cim:RE_UnitSymbol.VAh a cim:RE_UnitSymbol ;
  rdfs:label "VAh" ;
  rdfs:comment "Apparent energy in volt ampere hours"@en ;
  rdfs:isDefinedBy :Package_CIMEnumerations ;
  uml:id "EAID_A0E46D67_DAE3_41dd_8BBE_1E0EE42F37EE" .

cim:RE_UnitSymbol.VAr a cim:RE_UnitSymbol ;
  rdfs:label "VAr" ;
  rdfs:comment "Reactive power in volt ampere reactive"@en ;
  rdfs:isDefinedBy :Package_CIMEnumerations ;
  uml:id "EAID_4E613429_EDA8_4115_94A0_B010172B04AE" .

cim:RE_UnitSymbol.VArh a cim:RE_UnitSymbol ;
  rdfs:label "VArh" ;
  rdfs:comment "Reactive energy in volt ampere reactive hours"@en ;
  rdfs:isDefinedBy :Package_CIMEnumerations ;
  uml:id "EAID_226C8BBE_FE49_4fdb_AC07_CA17B1C461AE" .

cim:RE_UnitSymbol.W a cim:RE_UnitSymbol ;
  rdfs:label "W" ;
  rdfs:comment "Active power in watt"@en ;
  rdfs:isDefinedBy :Package_CIMEnumerations ;
  uml:id "EAID_09BD8937_7E80_460f_9AC6_5B2BF8ADC9D5" .

cim:RE_UnitSymbol.Wh a cim:RE_UnitSymbol ;
  rdfs:label "Wh" ;
  rdfs:comment "Real energy in what hours"@en ;
  rdfs:isDefinedBy :Package_CIMEnumerations ;
  uml:id "EAID_64930AB6_FB66_4c1e_9917_F90C9526314A" .

cim:RE_UnitSymbol.deg a cim:RE_UnitSymbol ;
  rdfs:label "deg" ;
  rdfs:comment "Plane angle in degrees"@en ;
  rdfs:isDefinedBy :Package_CIMEnumerations ;
  uml:id "EAID_8ECA4E7A_9070_4265_9505_97D3146376BB" .

cim:RE_UnitSymbol.degC a cim:RE_UnitSymbol ;
  rdfs:label "degC" ;
  rdfs:comment "Relative temperature in degrees Celsius. In the SI unit system the symbol is C. Electric charge is measured in coulomb that has the unit symbol C. To destinguish degree Celsius form coulomb the symbol used in the UML is degC. Reason for not using C is the special character  is difficult to manage in software."@en ;
  rdfs:isDefinedBy :Package_CIMEnumerations ;
  uml:id "EAID_EF2C967F_E4D4_4656_9A21_9267BDC24BCA" .

cim:RE_UnitSymbol.g a cim:RE_UnitSymbol ;
  rdfs:label "g" ;
  rdfs:comment "Mass in gram"@en ;
  rdfs:isDefinedBy :Package_CIMEnumerations ;
  uml:id "EAID_424CCF55_3D24_473a_82EC_A0446E2CA414" .

cim:RE_UnitSymbol.h a cim:RE_UnitSymbol ;
  rdfs:label "h" ;
  rdfs:comment "Time in hours"@en ;
  rdfs:isDefinedBy :Package_CIMEnumerations ;
  uml:id "EAID_96F30304_0F6F_4598_9929_9A4CECF6E22D" .

cim:RE_UnitSymbol.m a cim:RE_UnitSymbol ;
  rdfs:label "m" ;
  rdfs:comment "Length in meter"@en ;
  rdfs:isDefinedBy :Package_CIMEnumerations ;
  uml:id "EAID_D8A30C24_5F82_48f4_B86A_890D5C2F30A3" .

cim:RE_UnitSymbol.m2 a cim:RE_UnitSymbol ;
  rdfs:label "m2" ;
  rdfs:comment "Area in square meters"@en ;
  rdfs:isDefinedBy :Package_CIMEnumerations ;
  uml:id "EAID_9BBE63B4_C05B_4566_A763_263D08546340" .

cim:RE_UnitSymbol.m3 a cim:RE_UnitSymbol ;
  rdfs:label "m3" ;
  rdfs:comment "Volume in cubic meters"@en ;
  rdfs:isDefinedBy :Package_CIMEnumerations ;
  uml:id "EAID_EE9B9D81_A019_4894_99C6_C5632D448263" .

cim:RE_UnitSymbol.min a cim:RE_UnitSymbol ;
  rdfs:label "min" ;
  rdfs:comment "Time in minutes"@en ;
  rdfs:isDefinedBy :Package_CIMEnumerations ;
  uml:id "EAID_52EB81C6_1328_4835_9811_63F87A239CA5" .

cim:RE_UnitSymbol.none a cim:RE_UnitSymbol ;
  rdfs:label "none" ;
  rdfs:comment "Dimension less quantity, e.g. count, per unit, etc."@en ;
  rdfs:isDefinedBy :Package_CIMEnumerations ;
  uml:id "EAID_EA1B87C1_2C08_4775_90E8_00D871C9ADD3" .

cim:RE_UnitSymbol.ohm a cim:RE_UnitSymbol ;
  rdfs:label "ohm" ;
  rdfs:comment "Resistance in ohm"@en ;
  rdfs:isDefinedBy :Package_CIMEnumerations ;
  uml:id "EAID_6AE6208E_8576_47c0_A9DD_4AD4BC7C09C3" .

cim:RE_UnitSymbol.rad a cim:RE_UnitSymbol ;
  rdfs:label "rad" ;
  rdfs:comment "Plane angle in radians"@en ;
  rdfs:isDefinedBy :Package_CIMEnumerations ;
  uml:id "EAID_802E57FC_3F95_4304_A50B_3AA26E56E9A2" .

cim:RE_UnitSymbol.s a cim:RE_UnitSymbol ;
  rdfs:label "s" ;
  rdfs:comment "Time in seconds"@en ;
  rdfs:isDefinedBy :Package_CIMEnumerations ;
  uml:id "EAID_714C8194_3A05_407f_89EA_EA3D5568BD7A" .

cim:Reactance a rdfs:Datatype ;
  rdfs:label "Reactance" ;
  rdfs:comment "Reactance (imaginary part of impedance), at rated frequency."@en ;
  owl:equivalentClass xsd:float ;
  rdfs:isDefinedBy :Package_CIMDataTypes ;
  uml:hasMultiplier "none" ;
  uml:hasStereotype uml:cimdatatype ;
  uml:hasUnits "ohm" ;
  uml:id "EAID_E6647C55_B9C1_4641_96F0_A37531B351F8" .

cim:ReactancePerLength a rdfs:Datatype ;
  rdfs:label "ReactancePerLength" ;
  rdfs:comment "Reactance (imaginary part of impedance) per unit of length, at rated frequency."@en ;
  owl:equivalentClass xsd:float ;
  rdfs:isDefinedBy :Package_CIMDataTypes ;
  uml:hasMultiplier "none" ;
  uml:hasStereotype uml:cimdatatype ;
  uml:hasUnits "ohmPerm" ;
  uml:id "EAID_A7E9997F_4062_4cea_9A9B_9E8616B1B10B" .

cim:ReactivePower a rdfs:Datatype ;
  rdfs:label "ReactivePower" ;
  rdfs:comment "Product of RMS value of the voltage and the RMS value of the quadrature component of the current."@en ;
  owl:equivalentClass xsd:float ;
  rdfs:isDefinedBy :Package_CIMDataTypes ;
  uml:hasMultiplier "M" ;
  uml:hasStereotype uml:cimdatatype ;
  uml:hasUnits "VAr" ;
  uml:id "EAID_CC96E5EA_D0AB_40e4_B38C_0AFD3AC137A2" .

cim:RegulatingControlModeKind.activePower a cim:RegulatingControlModeKind ;
  rdfs:label "activePower" ;
  rdfs:comment "Active power is specified."@en ;
  rdfs:isDefinedBy :Package_CIMEnumerations ;
  uml:id "EAID_3A242210_5241_4aee_BDCC_B2EEC46D7526" .

cim:RegulatingControlModeKind.admittance a cim:RegulatingControlModeKind ;
  rdfs:label "admittance" ;
  rdfs:comment "Admittance is specified."@en ;
  rdfs:isDefinedBy :Package_CIMEnumerations ;
  uml:id "EAID_CC9BFCC8_FD49_4d34_8C86_6AB669472FBB" .

cim:RegulatingControlModeKind.currentFlow a cim:RegulatingControlModeKind ;
  rdfs:label "currentFlow" ;
  rdfs:comment "Current flow is specified."@en ;
  rdfs:isDefinedBy :Package_CIMEnumerations ;
  uml:id "EAID_DA6E8D1B_AAAB_443b_9D74_3CFD4D3CF2F7" .

cim:RegulatingControlModeKind.powerFactor a cim:RegulatingControlModeKind ;
  rdfs:label "powerFactor" ;
  rdfs:comment "Power factor is specified."@en ;
  rdfs:isDefinedBy :Package_CIMEnumerations ;
  uml:id "EAID_BBDBB729_3252_48bf_9021_4F9C7B27DABE" .

cim:RegulatingControlModeKind.reactivePower a cim:RegulatingControlModeKind ;
  rdfs:label "reactivePower" ;
  rdfs:comment "Reactive power is specified."@en ;
  rdfs:isDefinedBy :Package_CIMEnumerations ;
  uml:id "EAID_8F976702_2290_4ecc_8CC2_15D5D9E2B5C8" .

cim:RegulatingControlModeKind.temperature a cim:RegulatingControlModeKind ;
  rdfs:label "temperature" ;
  rdfs:comment "Control switches on/off based on the local temperature (i.e., a thermostat)."@en ;
  rdfs:isDefinedBy :Package_CIMEnumerations ;
  uml:id "EAID_ECDE8AEF_767A_4271_BC3E_9BCF890AC483" .

cim:RegulatingControlModeKind.timeScheduled a cim:RegulatingControlModeKind ;
  rdfs:label "timeScheduled" ;
  rdfs:comment "Control switches on/off by time of day. The times may change on the weekend, or in different seasons."@en ;
  rdfs:isDefinedBy :Package_CIMEnumerations ;
  uml:id "EAID_1F1704CF_ED40_4818_9990_F2DF43E570DC" .

cim:RegulatingControlModeKind.voltage a cim:RegulatingControlModeKind ;
  rdfs:label "voltage" ;
  rdfs:comment "Voltage is specified."@en ;
  rdfs:isDefinedBy :Package_CIMEnumerations ;
  uml:id "EAID_503A9670_BF42_4f3f_9B69_A219D154073D" .

cim:Resistance a rdfs:Datatype ;
  rdfs:label "Resistance" ;
  rdfs:comment "Resistance (real part of impedance)."@en ;
  owl:equivalentClass xsd:float ;
  rdfs:isDefinedBy :Package_CIMDataTypes ;
  uml:hasMultiplier "none" ;
  uml:hasStereotype uml:cimdatatype ;
  uml:hasUnits "ohm" ;
  uml:id "EAID_FA3E94AC_639D_4c8b_AB87_191BFC0FF0D9" .

cim:ResistancePerLength a rdfs:Datatype ;
  rdfs:label "ResistancePerLength" ;
  rdfs:comment "Resistance (real part of impedance) per unit of length."@en ;
  owl:equivalentClass xsd:float ;
  rdfs:isDefinedBy :Package_CIMDataTypes ;
  uml:hasMultiplier "none" ;
  uml:hasStereotype uml:cimdatatype ;
  uml:hasUnits "ohmPerm" ;
  uml:id "EAID_6C1F662A_01FC_4ac9_9E3C_79831BA6475C" .

cim:Seconds a rdfs:Datatype ;
  rdfs:label "Seconds" ;
  rdfs:comment "Time, in seconds"@en ;
  owl:equivalentClass xsd:float ;
  rdfs:isDefinedBy :Package_CIMDataTypes ;
  uml:hasMultiplier "none" ;
  uml:hasStereotype uml:cimdatatype ;
  uml:hasUnits "s" ;
  uml:id "EAID_A31852A6_6FB6_42f5_89BE_1436C133DF02" .

cim:SinglePhaseKind.A a cim:SinglePhaseKind ;
  rdfs:label "A" ;
  rdfs:comment "Phase A."@en ;
  rdfs:isDefinedBy :Package_CIMEnumerations ;
  uml:id "EAID_DB6D14A1_A992_40c2_9ADC_98E77A562976" .

cim:SinglePhaseKind.B a cim:SinglePhaseKind ;
  rdfs:label "B" ;
  rdfs:comment "Phase B."@en ;
  rdfs:isDefinedBy :Package_CIMEnumerations ;
  uml:id "EAID_9201A3D3_AED5_4e24_B6B9_DADA199BEB44" .

cim:SinglePhaseKind.C a cim:SinglePhaseKind ;
  rdfs:label "C" ;
  rdfs:comment "Phase C."@en ;
  rdfs:isDefinedBy :Package_CIMEnumerations ;
  uml:id "EAID_A16526E7_12C4_459f_AEFB_BF71DBA05A20" .

cim:SinglePhaseKind.N a cim:SinglePhaseKind ;
  rdfs:label "N" ;
  rdfs:comment "Neutral."@en ;
  rdfs:isDefinedBy :Package_CIMEnumerations ;
  uml:id "EAID_15D88944_D797_4fb7_B472_9B08783989DD" .

cim:SinglePhaseKind.s1 a cim:SinglePhaseKind ;
  rdfs:label "s1" ;
  rdfs:comment "Secondary phase 1."@en ;
  rdfs:isDefinedBy :Package_CIMEnumerations ;
  uml:id "EAID_2A8A3118_9520_451a_B36F_9FDA42EED05D" .

cim:SinglePhaseKind.s2 a cim:SinglePhaseKind ;
  rdfs:label "s2" ;
  rdfs:comment "Secondary phase 2."@en ;
  rdfs:isDefinedBy :Package_CIMEnumerations ;
  uml:id "EAID_A309AF87_34D9_4666_88BF_E181D87835CA" .

cim:Source.DEFAULTED a cim:Source ;
  rdfs:label "DEFAULTED" ;
  rdfs:comment "The value contains a default value."@en ;
  rdfs:isDefinedBy :Package_CIMEnumerations ;
  uml:id "EAID_370C51F9_6A1C_46d9_8249_B180DC1C8B19" .

cim:Source.PROCESS a cim:Source ;
  rdfs:label "PROCESS" ;
  rdfs:comment "The value is provided by input from the process I/O or being calculated from some function."@en ;
  rdfs:isDefinedBy :Package_CIMEnumerations ;
  uml:id "EAID_C84C8FE1_DD0B_4ad1_9029_FD7E5B67FC32" .

cim:Source.SUBSTITUTED a cim:Source ;
  rdfs:label "SUBSTITUTED" ;
  rdfs:comment "The value is provided by input of an operator or by an automatic source."@en ;
  rdfs:isDefinedBy :Package_CIMEnumerations ;
  uml:id "EAID_F4E73941_BB66_4305_9EA8_B143906FA010" .

cim:Susceptance a rdfs:Datatype ;
  rdfs:label "Susceptance" ;
  rdfs:comment "Imaginary part of admittance."@en ;
  owl:equivalentClass xsd:float ;
  rdfs:isDefinedBy :Package_CIMDataTypes ;
  uml:hasMultiplier "none" ;
  uml:hasStereotype uml:cimdatatype ;
  uml:hasUnits "S" ;
  uml:id "EAID_103215C2_533F_402a_8F81_CC945A4D81E2" .

cim:SusceptancePerLength a rdfs:Datatype ;
  rdfs:label "SusceptancePerLength" ;
  rdfs:comment "Imaginary part of admittance per unit of length."@en ;
  owl:equivalentClass xsd:float ;
  rdfs:isDefinedBy :Package_CIMDataTypes ;
  uml:hasMultiplier "none" ;
  uml:hasStereotype uml:cimdatatype ;
  uml:hasUnits "SPerm" ;
  uml:id "EAID_71A6BB9C_53CC_488a_A79F_CCA69267D61E" .

cim:SynchronousMachineKind.condenser a cim:SynchronousMachineKind ;
  rdfs:label "condenser" ;
  rdfs:isDefinedBy :Package_CIMEnumerations ;
  uml:id "EAID_00750BBA_4AD4_4e59_BCF9_83D1E5C5CB86" .

cim:SynchronousMachineKind.generator a cim:SynchronousMachineKind ;
  rdfs:label "generator" ;
  rdfs:isDefinedBy :Package_CIMEnumerations ;
  uml:id "EAID_627E55C1_C38A_4dbc_8F56_DCFE8AC55DDE" .

cim:SynchronousMachineKind.generatorOrCondenser a cim:SynchronousMachineKind ;
  rdfs:label "generatorOrCondenser" ;
  rdfs:isDefinedBy :Package_CIMEnumerations ;
  uml:id "EAID_D97A2F0C_8961_44a5_889D_1A5184FB8877" .

cim:SynchronousMachineKind.generatorOrCondenserOrMotor a cim:SynchronousMachineKind ;
  rdfs:label "generatorOrCondenserOrMotor" ;
  rdfs:isDefinedBy :Package_CIMEnumerations ;
  uml:id "EAID_F2DA14F7_3AEA_40ce_A8B0_1D48A1BB0C33" .

cim:SynchronousMachineKind.generatorOrMotor a cim:SynchronousMachineKind ;
  rdfs:label "generatorOrMotor" ;
  rdfs:isDefinedBy :Package_CIMEnumerations ;
  uml:id "EAID_3B8665CF_C9C2_406b_ABC7_F422D211FD74" .

cim:SynchronousMachineKind.motor a cim:SynchronousMachineKind ;
  rdfs:label "motor" ;
  rdfs:isDefinedBy :Package_CIMEnumerations ;
  uml:id "EAID_D5DD2C3F_51DB_422d_A374_37E1E485FFBB" .

cim:SynchronousMachineKind.motorOrCondenser a cim:SynchronousMachineKind ;
  rdfs:label "motorOrCondenser" ;
  rdfs:isDefinedBy :Package_CIMEnumerations ;
  uml:id "EAID_E375A69E_0415_4f6d_A3F0_054109E5F696" .

cim:SynchronousMachineOperatingMode.condenser a cim:SynchronousMachineOperatingMode ;
  rdfs:label "condenser" ;
  rdfs:isDefinedBy :Package_CIMEnumerations ;
  uml:id "EAID_6F8D9A9E_FDB1_4008_B152_034D447C1B16" .

cim:SynchronousMachineOperatingMode.generator a cim:SynchronousMachineOperatingMode ;
  rdfs:label "generator" ;
  rdfs:isDefinedBy :Package_CIMEnumerations ;
  uml:id "EAID_A7C24167_4F73_4f82_8EFC_C047BE2B1A89" .

cim:SynchronousMachineOperatingMode.motor a cim:SynchronousMachineOperatingMode ;
  rdfs:label "motor" ;
  rdfs:isDefinedBy :Package_CIMEnumerations ;
  uml:id "EAID_65FD9F19_65B2_4654_93EA_F3FEA630C765" .

cim:Temperature a rdfs:Datatype ;
  rdfs:label "Temperature" ;
  rdfs:comment "Value of temperature in degrees Celsius."@en ;
  owl:equivalentClass xsd:float ;
  rdfs:isDefinedBy :Package_CIMDataTypes ;
  uml:hasMultiplier "none" ;
  uml:hasStereotype uml:cimdatatype ;
  uml:hasUnits "degC" ;
  uml:id "EAID_93052F5B_A392_42f6_AD2B_BBD13DD080B6" .

cim:TransformerControlMode.reactive a cim:TransformerControlMode ;
  rdfs:label "reactive" ;
  rdfs:comment "Reactive power flow control"@en ;
  rdfs:isDefinedBy :Package_CIMEnumerations ;
  uml:id "EAID_F76A9BEF_6CA9_4073_BF18_10F8A39A3C54" .

cim:TransformerControlMode.volt a cim:TransformerControlMode ;
  rdfs:label "volt" ;
  rdfs:comment "Voltage control"@en ;
  rdfs:isDefinedBy :Package_CIMEnumerations ;
  uml:id "EAID_46309B1F_4C1C_468a_9D9A_CC189525BBFA" .

cim:UnitMultiplier.E a cim:UnitMultiplier ;
  rdfs:label "E" ;
  rdfs:comment "Exa 10**18."@en ;
  rdfs:isDefinedBy :Package_CIMEnumerations ;
  uml:id "EAID_C5C15442_BFDE_4707_9E9B_614F0960086A" .

cim:UnitMultiplier.G a cim:UnitMultiplier ;
  rdfs:label "G" ;
  rdfs:comment "Giga 10**9"@en ;
  rdfs:isDefinedBy :Package_CIMEnumerations ;
  uml:id "EAID_AFD1C533_8EFC_4ef1_86AA_320EE060BDAE" .

cim:UnitMultiplier.M a cim:UnitMultiplier ;
  rdfs:label "M" ;
  rdfs:comment "Mega 10**6"@en ;
  rdfs:isDefinedBy :Package_CIMEnumerations ;
  uml:id "EAID_E1B011DE_672C_4e2c_8FCB_9EC7FECE85B9" .

cim:UnitMultiplier.P a cim:UnitMultiplier ;
  rdfs:label "P" ;
  rdfs:comment "Peta 10**15"@en ;
  rdfs:isDefinedBy :Package_CIMEnumerations ;
  uml:id "EAID_051C3A9E_75DC_4df2_AA07_31E381BD7D51" .

cim:UnitMultiplier.T a cim:UnitMultiplier ;
  rdfs:label "T" ;
  rdfs:comment "Tera 10**12"@en ;
  rdfs:isDefinedBy :Package_CIMEnumerations ;
  uml:id "EAID_61A4565B_982A_44cb_B8E4_5DA4D5F2BDE5" .

cim:UnitMultiplier.Y a cim:UnitMultiplier ;
  rdfs:label "Y" ;
  rdfs:comment "Yotta 10**24"@en ;
  rdfs:isDefinedBy :Package_CIMEnumerations ;
  uml:id "EAID_AD5C72FE_4530_4239_A2FF_83193695B3AE" .

cim:UnitMultiplier.Z a cim:UnitMultiplier ;
  rdfs:label "Z" ;
  rdfs:comment "Zetta 10**21"@en ;
  rdfs:isDefinedBy :Package_CIMEnumerations ;
  uml:id "EAID_11BDF9ED_D8FD_431b_B0F5_77B3B4C899AC" .

cim:UnitMultiplier.a a cim:UnitMultiplier ;
  rdfs:label "a" ;
  rdfs:comment "atto 10**-18."@en ;
  rdfs:isDefinedBy :Package_CIMEnumerations ;
  uml:id "EAID_FE6505E5_A528_449e_B404_DB453AE4F04D" .

cim:UnitMultiplier.c a cim:UnitMultiplier ;
  rdfs:label "c" ;
  rdfs:comment "Centi 10**-2"@en ;
  rdfs:isDefinedBy :Package_CIMEnumerations ;
  uml:id "EAID_DD0B514D_88B5_44b2_8E1E_F38548EF1473" .

cim:UnitMultiplier.d a cim:UnitMultiplier ;
  rdfs:label "d" ;
  rdfs:comment "Deci 10**-1"@en ;
  rdfs:isDefinedBy :Package_CIMEnumerations ;
  uml:id "EAID_1D7A475A_3750_4608_936F_490FE8D92D3E" .

cim:UnitMultiplier.da a cim:UnitMultiplier ;
  rdfs:label "da" ;
  rdfs:comment "deca 10**1."@en ;
  rdfs:isDefinedBy :Package_CIMEnumerations ;
  uml:id "EAID_471A251F_92B6_4af8_9FCC_5202BD959D96" .

cim:UnitMultiplier.f a cim:UnitMultiplier ;
  rdfs:label "f" ;
  rdfs:comment "femto 10**-15."@en ;
  rdfs:isDefinedBy :Package_CIMEnumerations ;
  uml:id "EAID_AFEE121A_F906_46e1_8313_92514C1A4678" .

cim:UnitMultiplier.h a cim:UnitMultiplier ;
  rdfs:label "h" ;
  rdfs:comment "hecto 10**2."@en ;
  rdfs:isDefinedBy :Package_CIMEnumerations ;
  uml:id "EAID_65E1E0A8_6EC4_4d33_814B_865C6F119C90" .

cim:UnitMultiplier.k a cim:UnitMultiplier ;
  rdfs:label "k" ;
  rdfs:comment "Kilo 10**3"@en ;
  rdfs:isDefinedBy :Package_CIMEnumerations ;
  uml:id "EAID_E948AAE1_01BD_4043_BDB1_68635BF460F3" .

cim:UnitMultiplier.m a cim:UnitMultiplier ;
  rdfs:label "m" ;
  rdfs:comment "Milli 10**-3"@en ;
  rdfs:isDefinedBy :Package_CIMEnumerations ;
  uml:id "EAID_507BCDCB_B560_4b11_98E7_3FDB7F7FEE60" .

cim:UnitMultiplier.micro a cim:UnitMultiplier ;
  rdfs:label "micro" ;
  rdfs:comment "Micro 10**-6"@en ;
  rdfs:isDefinedBy :Package_CIMEnumerations ;
  uml:id "EAID_A240E6A3_C9CD_491c_8CF0_5F937DAF8133" .

cim:UnitMultiplier.n a cim:UnitMultiplier ;
  rdfs:label "n" ;
  rdfs:comment "Nano 10**-9"@en ;
  rdfs:isDefinedBy :Package_CIMEnumerations ;
  uml:id "EAID_002AEB7F_EFD4_4961_9EA4_10425961D0F2" .

cim:UnitMultiplier.none a cim:UnitMultiplier ;
  rdfs:label "none" ;
  rdfs:isDefinedBy :Package_CIMEnumerations ;
  uml:id "EAID_CE1AC3A2_D62E_4168_9909_E4298D28933D" .

cim:UnitMultiplier.p a cim:UnitMultiplier ;
  rdfs:label "p" ;
  rdfs:comment "Pico 10**-12"@en ;
  rdfs:isDefinedBy :Package_CIMEnumerations ;
  uml:id "EAID_816E050B_5E00_418d_A9DA_9CA703C98E30" .

cim:UnitMultiplier.y a cim:UnitMultiplier ;
  rdfs:label "y" ;
  rdfs:comment "yocto 10**-24."@en ;
  rdfs:isDefinedBy :Package_CIMEnumerations ;
  uml:id "EAID_F3FD1886_B7ED_4c9b_8747_9BD316B4E631" .

cim:UnitMultiplier.z a cim:UnitMultiplier ;
  rdfs:label "z" ;
  rdfs:comment "zepto 10**-21."@en ;
  rdfs:isDefinedBy :Package_CIMEnumerations ;
  uml:id "EAID_F2E5D8DC_AAA2_4e84_830B_C1260BAE9B3F" .

cim:UnitSymbol.A a cim:UnitSymbol ;
  rdfs:label "A" ;
  rdfs:comment "Current in Ampere."@en ;
  rdfs:isDefinedBy :Package_CIMEnumerations ;
  uml:id "EAID_73192209_46C4_4236_A93F_622B9B20B1D2" .

cim:UnitSymbol.A2 a cim:UnitSymbol ;
  rdfs:label "A2" ;
  rdfs:comment "Ampere squared (A)."@en ;
  rdfs:isDefinedBy :Package_CIMEnumerations ;
  uml:id "EAID_18F91DF9_5F02_4fcc_8718_6F1B172B69A6" .

cim:UnitSymbol.A2h a cim:UnitSymbol ;
  rdfs:label "A2h" ;
  rdfs:comment "ampere-squared hour, Ampere-squared hour."@en ;
  rdfs:isDefinedBy :Package_CIMEnumerations ;
  uml:id "EAID_01289D24_5F6D_41ec_94BF_393D18E0BDF6" .

cim:UnitSymbol.A2s a cim:UnitSymbol ;
  rdfs:label "A2s" ;
  rdfs:comment "Ampere squared time in square ampere (As)."@en ;
  rdfs:isDefinedBy :Package_CIMEnumerations ;
  uml:id "EAID_EABC3521_23CB_4f06_8DF2_FCB922207D3D" .

cim:UnitSymbol.APerA a cim:UnitSymbol ;
  rdfs:label "APerA" ;
  rdfs:comment "Current, Ratio of Amperages  Note: Users may need to supply a prefix such as m to show rates such as mA/A."@en ;
  rdfs:isDefinedBy :Package_CIMEnumerations ;
  uml:id "EAID_0981015A_8462_486a_B3F8_BDE9BF366589" .

cim:UnitSymbol.APerm a cim:UnitSymbol ;
  rdfs:label "APerm" ;
  rdfs:comment "A/m, magnetic field strength, Ampere per metre."@en ;
  rdfs:isDefinedBy :Package_CIMEnumerations ;
  uml:id "EAID_D3199EFD_A62A_4880_BAD2_C8C7DBB980D3" .

cim:UnitSymbol.Ah a cim:UnitSymbol ;
  rdfs:label "Ah" ;
  rdfs:comment "Ampere-hours, Ampere-hours."@en ;
  rdfs:isDefinedBy :Package_CIMEnumerations ;
  uml:id "EAID_CE9B8EC3_3129_42df_87A0_36D042ABD54B" .

cim:UnitSymbol.As a cim:UnitSymbol ;
  rdfs:label "As" ;
  rdfs:comment "Ampere seconds (As)."@en ;
  rdfs:isDefinedBy :Package_CIMEnumerations ;
  uml:id "EAID_49C928A6_F4C8_4393_B349_B7C3E333DCAF" .

cim:UnitSymbol.Bq a cim:UnitSymbol ;
  rdfs:label "Bq" ;
  rdfs:comment "Radioactivity in Becquerel (1/s)."@en ;
  rdfs:isDefinedBy :Package_CIMEnumerations ;
  uml:id "EAID_30B53BA7_AE34_4baa_B893_2C10F799CFA1" .

cim:UnitSymbol.Btu a cim:UnitSymbol ;
  rdfs:label "Btu" ;
  rdfs:comment "Energy, British Thermal Unit."@en ;
  rdfs:isDefinedBy :Package_CIMEnumerations ;
  uml:id "EAID_1B4C1E78_59D4_4d29_A7A1_71CBC49EE405" .

cim:UnitSymbol.C a cim:UnitSymbol ;
  rdfs:label "C" ;
  rdfs:comment "Electric charge in Coulomb (As)."@en ;
  rdfs:isDefinedBy :Package_CIMEnumerations ;
  uml:id "EAID_C61A2A7C_DF02_44c5_9FC1_A47B7645816E" .

cim:UnitSymbol.CPerkg a cim:UnitSymbol ;
  rdfs:label "CPerkg" ;
  rdfs:comment "exposure (x rays), Coulomb per kilogram."@en ;
  rdfs:isDefinedBy :Package_CIMEnumerations ;
  uml:id "EAID_BE648D60_3104_4798_9AF2_ADD5F3BECC9A" .

cim:UnitSymbol.CPerm2 a cim:UnitSymbol ;
  rdfs:label "CPerm2" ;
  rdfs:comment "surface charge density, Coulomb per square metre."@en ;
  rdfs:isDefinedBy :Package_CIMEnumerations ;
  uml:id "EAID_3283D3E6_1A08_4008_BDCB_DCA8752664A4" .

cim:UnitSymbol.CPerm3 a cim:UnitSymbol ;
  rdfs:label "CPerm3" ;
  rdfs:comment "electric charge density, Coulomb per cubic metre."@en ;
  rdfs:isDefinedBy :Package_CIMEnumerations ;
  uml:id "EAID_8F77778C_0BD6_446b_B67C_10683180E189" .

cim:UnitSymbol.F a cim:UnitSymbol ;
  rdfs:label "F" ;
  rdfs:comment "Electric capacitance in Farad (C/V)."@en ;
  rdfs:isDefinedBy :Package_CIMEnumerations ;
  uml:id "EAID_D70AA740_B956_43a8_99CF_6DB3A5AA09B1" .

cim:UnitSymbol.FPerm a cim:UnitSymbol ;
  rdfs:label "FPerm" ;
  rdfs:comment "permittivity, Farad per metre."@en ;
  rdfs:isDefinedBy :Package_CIMEnumerations ;
  uml:id "EAID_C04572EA_C3F3_4517_99AE_C2CEA71B58C8" .

cim:UnitSymbol.G a cim:UnitSymbol ;
  rdfs:label "G" ;
  rdfs:comment "Magnetic flux density, Gauss (1 G = 10-4 T)."@en ;
  rdfs:isDefinedBy :Package_CIMEnumerations ;
  uml:id "EAID_FE8F4D96_0B8D_4ffb_88F9_6443451F7424" .

cim:UnitSymbol.Gy a cim:UnitSymbol ;
  rdfs:label "Gy" ;
  rdfs:comment "Absorbed dose in Gray (J/kg)."@en ;
  rdfs:isDefinedBy :Package_CIMEnumerations ;
  uml:id "EAID_8CE82932_8CA9_4160_9446_17BED2B1E815" .

cim:UnitSymbol.GyPers a cim:UnitSymbol ;
  rdfs:label "GyPers" ;
  rdfs:comment "absorbed dose rate, Gray per second."@en ;
  rdfs:isDefinedBy :Package_CIMEnumerations ;
  uml:id "EAID_78EF1199_DA54_4191_ADE0_E5D68B8F605A" .

cim:UnitSymbol.H a cim:UnitSymbol ;
  rdfs:label "H" ;
  rdfs:comment "Electric inductance in Henry (Wb/A)."@en ;
  rdfs:isDefinedBy :Package_CIMEnumerations ;
  uml:id "EAID_8040E2D3_A5E3_4bf8_B171_DC7FA9E864B9" .

cim:UnitSymbol.HPerm a cim:UnitSymbol ;
  rdfs:label "HPerm" ;
  rdfs:comment "permeability, Henry per metre."@en ;
  rdfs:isDefinedBy :Package_CIMEnumerations ;
  uml:id "EAID_0AFE859F_EC8D_4f7d_B7DA_B9770716017B" .

cim:UnitSymbol.Hz a cim:UnitSymbol ;
  rdfs:label "Hz" ;
  rdfs:comment "Frequency in Hertz (1/s)."@en ;
  rdfs:isDefinedBy :Package_CIMEnumerations ;
  uml:id "EAID_12FFE4AD_4859_47dd_A5F9_3AD564FCD8FC" .

cim:UnitSymbol.HzPerHz a cim:UnitSymbol ;
  rdfs:label "HzPerHz" ;
  rdfs:comment "Frequency, Rate of frequency change  Note: Users may need to supply a prefix such as m to show rates such as mHz/Hz."@en ;
  rdfs:isDefinedBy :Package_CIMEnumerations ;
  uml:id "EAID_34F2F478_6864_4ddc_9F2E_C31BAF85AC60" .

cim:UnitSymbol.HzPers a cim:UnitSymbol ;
  rdfs:label "HzPers" ;
  rdfs:comment "Rate of change of frequency in Hertz per second."@en ;
  rdfs:isDefinedBy :Package_CIMEnumerations ;
  uml:id "EAID_AEEED7A8_50C6_4856_ACF4_A280D57EB110" .

cim:UnitSymbol.J a cim:UnitSymbol ;
  rdfs:label "J" ;
  rdfs:comment "Energy in joule (Nm = CV = Ws)."@en ;
  rdfs:isDefinedBy :Package_CIMEnumerations ;
  uml:id "EAID_4FE8744A_7C5F_4fc7_8FFB_5B9A05F0EF19" .

cim:UnitSymbol.JPerK a cim:UnitSymbol ;
  rdfs:label "JPerK" ;
  rdfs:comment "Heat capacity in Joule/Kelvin."@en ;
  rdfs:isDefinedBy :Package_CIMEnumerations ;
  uml:id "EAID_FF36C817_7511_422c_A716_6C89E08ACBC4" .

cim:UnitSymbol.JPerkg a cim:UnitSymbol ;
  rdfs:label "JPerkg" ;
  rdfs:comment "Specific energy, Joule / kg."@en ;
  rdfs:isDefinedBy :Package_CIMEnumerations ;
  uml:id "EAID_9AF99907_30CB_43b3_91AA_CB01E39EEBA1" .

cim:UnitSymbol.JPerkgK a cim:UnitSymbol ;
  rdfs:label "JPerkgK" ;
  rdfs:comment "Specific heat capacity, specific entropy, Joule per kilogram Kelvin."@en ;
  rdfs:isDefinedBy :Package_CIMEnumerations ;
  uml:id "EAID_39ADD645_66F8_4b70_96D8_1D4EC7778020" .

cim:UnitSymbol.JPerm2 a cim:UnitSymbol ;
  rdfs:label "JPerm2" ;
  rdfs:comment "Insulation energy density, Joule per square metre or watt second per square metre."@en ;
  rdfs:isDefinedBy :Package_CIMEnumerations ;
  uml:id "EAID_212F940C_F1E4_4eaa_B1D3_5102896EEB35" .

cim:UnitSymbol.JPerm3 a cim:UnitSymbol ;
  rdfs:label "JPerm3" ;
  rdfs:comment "energy density, Joule per cubic metre."@en ;
  rdfs:isDefinedBy :Package_CIMEnumerations ;
  uml:id "EAID_3C842C47_4B64_4c2e_9427_46ADCDCE35F0" .

cim:UnitSymbol.JPermol a cim:UnitSymbol ;
  rdfs:label "JPermol" ;
  rdfs:comment "molar energy, Joule per mole."@en ;
  rdfs:isDefinedBy :Package_CIMEnumerations ;
  uml:id "EAID_353C895C_47E1_4914_B6E1_BD5BCAB94594" .

cim:UnitSymbol.JPermolK a cim:UnitSymbol ;
  rdfs:label "JPermolK" ;
  rdfs:comment "molar entropy, molar heat capacity, Joule per mole kelvin."@en ;
  rdfs:isDefinedBy :Package_CIMEnumerations ;
  uml:id "EAID_F882002C_6A67_4257_BDBE_6CCC013B9AB3" .

cim:UnitSymbol.JPers a cim:UnitSymbol ;
  rdfs:label "JPers" ;
  rdfs:comment "Energy rate joule per second (J/s),"@en ;
  rdfs:isDefinedBy :Package_CIMEnumerations ;
  uml:id "EAID_634EDCB8_AD8B_41e9_90BE_5505F97851D9" .

cim:UnitSymbol.K a cim:UnitSymbol ;
  rdfs:label "K" ;
  rdfs:comment "Temperature in Kelvin."@en ;
  rdfs:isDefinedBy :Package_CIMEnumerations ;
  uml:id "EAID_1C7019D4_4C0C_4563_BD39_4341656535C3" .

cim:UnitSymbol.KPers a cim:UnitSymbol ;
  rdfs:label "KPers" ;
  rdfs:comment "Temperature change rate in Kelvin per second."@en ;
  rdfs:isDefinedBy :Package_CIMEnumerations ;
  uml:id "EAID_9A2A4DC0_BF90_466e_B784_29EA09352F82" .

cim:UnitSymbol.M a cim:UnitSymbol ;
  rdfs:label "M" ;
  rdfs:comment "Length, nautical mile (1 M = 1852 m)."@en ;
  rdfs:isDefinedBy :Package_CIMEnumerations ;
  uml:id "EAID_968D12C1_180C_4b26_B5DF_012BD53DED80" .

cim:UnitSymbol.Mx a cim:UnitSymbol ;
  rdfs:label "Mx" ;
  rdfs:comment "Magnetic flux, Maxwell (1 Mx = 10-8 Wb)."@en ;
  rdfs:isDefinedBy :Package_CIMEnumerations ;
  uml:id "EAID_D1C8B88C_D6A3_4717_946B_867577DE8009" .

cim:UnitSymbol.N a cim:UnitSymbol ;
  rdfs:label "N" ;
  rdfs:comment "Force in Newton (kgm/s)."@en ;
  rdfs:isDefinedBy :Package_CIMEnumerations ;
  uml:id "EAID_8A741E4F_51FC_4b84_A786_4A9D8C113F9D" .

cim:UnitSymbol.NPerm a cim:UnitSymbol ;
  rdfs:label "NPerm" ;
  rdfs:comment "Surface tension, Newton per metre."@en ;
  rdfs:isDefinedBy :Package_CIMEnumerations ;
  uml:id "EAID_C4D5B098_8516_4a09_9438_021D4673AF64" .

cim:UnitSymbol.Nm a cim:UnitSymbol ;
  rdfs:label "Nm" ;
  rdfs:comment "Moment of force, Newton metre."@en ;
  rdfs:isDefinedBy :Package_CIMEnumerations ;
  uml:id "EAID_81CE58A8_CB0D_4985_95F9_AD61BF9564C2" .

cim:UnitSymbol.Oe a cim:UnitSymbol ;
  rdfs:label "Oe" ;
  rdfs:comment "Magnetic field, rsted (1 Oe = (103/4p) A/m)."@en ;
  rdfs:isDefinedBy :Package_CIMEnumerations ;
  uml:id "EAID_B2481968_BFB0_4b4e_B558_1B5D0ECBEABA" .

cim:UnitSymbol.Pa a cim:UnitSymbol ;
  rdfs:label "Pa" ;
  rdfs:comment "Pressure in Pascal (N/m). Note: the absolute or relative measurement of pressure is implied with this entry. See below for more explicit forms."@en ;
  rdfs:isDefinedBy :Package_CIMEnumerations ;
  uml:id "EAID_91C62CD5_316C_4133_B60C_10B358D0151D" .

cim:UnitSymbol.PaPers a cim:UnitSymbol ;
  rdfs:label "PaPers" ;
  rdfs:comment "Pressure change rate in Pascal per second."@en ;
  rdfs:isDefinedBy :Package_CIMEnumerations ;
  uml:id "EAID_021658D5_DF8F_4227_ADB8_65714453802B" .

cim:UnitSymbol.Pas a cim:UnitSymbol ;
  rdfs:label "Pas" ;
  rdfs:comment "Dynamic viscosity, Pascal second."@en ;
  rdfs:isDefinedBy :Package_CIMEnumerations ;
  uml:id "EAID_D232804D_4191_48f5_B5E7_B71B50AD52DE" .

cim:UnitSymbol.Q a cim:UnitSymbol ;
  rdfs:label "Q" ;
  rdfs:comment "Quantity power, Q."@en ;
  rdfs:isDefinedBy :Package_CIMEnumerations ;
  uml:id "EAID_1BB7A76B_00E0_4d58_AD95_5DCF130E8324" .

cim:UnitSymbol.Qh a cim:UnitSymbol ;
  rdfs:label "Qh" ;
  rdfs:comment "Quantity energy, Qh."@en ;
  rdfs:isDefinedBy :Package_CIMEnumerations ;
  uml:id "EAID_1770F83A_9153_45e4_91DD_DC53260E2843" .

cim:UnitSymbol.S a cim:UnitSymbol ;
  rdfs:label "S" ;
  rdfs:comment "Conductance in Siemens."@en ;
  rdfs:isDefinedBy :Package_CIMEnumerations ;
  uml:id "EAID_957E82E6_ECC7_4bad_857B_40D8EFB98461" .

cim:UnitSymbol.SPerm a cim:UnitSymbol ;
  rdfs:label "SPerm" ;
  rdfs:comment "Conductance per length (F/m)."@en ;
  rdfs:isDefinedBy :Package_CIMEnumerations ;
  uml:id "EAID_53A6D4F2_8E3C_4abb_9F90_D3384CD9F08E" .

cim:UnitSymbol.Sv a cim:UnitSymbol ;
  rdfs:label "Sv" ;
  rdfs:comment "Dose equivalent in Sievert (J/kg)."@en ;
  rdfs:isDefinedBy :Package_CIMEnumerations ;
  uml:id "EAID_14CB198F_E1D3_4622_950B_5553B10C2852" .

cim:UnitSymbol.T a cim:UnitSymbol ;
  rdfs:label "T" ;
  rdfs:comment "Magnetic flux density in Tesla (Wb/m2)."@en ;
  rdfs:isDefinedBy :Package_CIMEnumerations ;
  uml:id "EAID_2EC7E58C_2672_45ac_B70D_B9DB36DC1BBB" .

cim:UnitSymbol.V a cim:UnitSymbol ;
  rdfs:label "V" ;
  rdfs:comment "Electric potential in Volt (W/A)."@en ;
  rdfs:isDefinedBy :Package_CIMEnumerations ;
  uml:id "EAID_3FB55A80_415D_4a6b_8A30_C75CD420B222" .

cim:UnitSymbol.V2 a cim:UnitSymbol ;
  rdfs:label "V2" ;
  rdfs:comment "Volt squared (W/A)."@en ;
  rdfs:isDefinedBy :Package_CIMEnumerations ;
  uml:id "EAID_F50AD8B5_9E99_41fe_BB86_CBC5CA9491B4" .

cim:UnitSymbol.V2h a cim:UnitSymbol ;
  rdfs:label "V2h" ;
  rdfs:comment "volt-squared hour, Volt-squared-hours."@en ;
  rdfs:isDefinedBy :Package_CIMEnumerations ;
  uml:id "EAID_5A34C44C_74CD_4810_B21A_FC8C343AC7C8" .

cim:UnitSymbol.VA a cim:UnitSymbol ;
  rdfs:label "VA" ;
  rdfs:comment "Apparent power in Volt Ampere (See also real power and reactive power.)"@en ;
  rdfs:isDefinedBy :Package_CIMEnumerations ;
  uml:id "EAID_D143576A_D481_4b1f_BDBD_8F388295FFAE" .

cim:UnitSymbol.VAh a cim:UnitSymbol ;
  rdfs:label "VAh" ;
  rdfs:comment "Apparent energy in Volt Ampere hours."@en ;
  rdfs:isDefinedBy :Package_CIMEnumerations ;
  uml:id "EAID_3C54998F_DB57_4682_8152_68D311DD9089" .

cim:UnitSymbol.VAr a cim:UnitSymbol ;
  rdfs:label "VAr" ;
  rdfs:comment """Reactive power in Volt Ampere reactive. The reactive or imaginary component of electrical power (VIsin(phi)). (See also real power and apparent power).
Note: Different meter designs use different methods to arrive at their results. Some meters may compute reactive power as an arithmetic value, while others compute the value vectorially. The data consumer should determine the method in use and the suitability of the measurement for the intended purpose."""@en ;
  rdfs:isDefinedBy :Package_CIMEnumerations ;
  uml:id "EAID_DCEBA4F8_0358_41de_A358_F1B17E674523" .

cim:UnitSymbol.VArh a cim:UnitSymbol ;
  rdfs:label "VArh" ;
  rdfs:comment "Reactive energy in Volt Ampere reactive hours."@en ;
  rdfs:isDefinedBy :Package_CIMEnumerations ;
  uml:id "EAID_46D8AE45_E355_49a2_B804_3ADAC25E50D1" .

cim:UnitSymbol.VPerHz a cim:UnitSymbol ;
  rdfs:label "VPerHz" ;
  rdfs:comment "Magnetic flux in Volt per Hertz."@en ;
  rdfs:isDefinedBy :Package_CIMEnumerations ;
  uml:id "EAID_07982CB2_AB66_430f_81F7_89B4401DAA26" .

cim:UnitSymbol.VPerV a cim:UnitSymbol ;
  rdfs:label "VPerV" ;
  rdfs:comment "Voltage, Ratio of voltages Note: Users may need to supply a prefix such as m to show rates such as mV/V."@en ;
  rdfs:isDefinedBy :Package_CIMEnumerations ;
  uml:id "EAID_2FA931F4_B97C_4478_AA52_CB5B05B1C38A" .

cim:UnitSymbol.VPerVA a cim:UnitSymbol ;
  rdfs:label "VPerVA" ;
  rdfs:comment "Power factor, PF, the ratio of the active power to the apparent power. Note: The sign convention used for power factor will differ between IEC meters and EEI (ANSI) meters. It is assumed that the data consumers understand the type of meter being used and agree on the sign convention in use at any given utility."@en ;
  rdfs:isDefinedBy :Package_CIMEnumerations ;
  uml:id "EAID_84F0EE0E_944C_4c28_AFC7_966E1E8C6ACB" .

cim:UnitSymbol.VPerVAr a cim:UnitSymbol ;
  rdfs:label "VPerVAr" ;
  rdfs:comment "Power factor, PF, the ratio of the active power to the apparent power. Note: The sign convention used for power factor will differ between IEC meters and EEI (ANSI) meters. It is assumed that the data consumers understand the type of meter being used and agree on the sign convention in use at any given utility."@en ;
  rdfs:isDefinedBy :Package_CIMEnumerations ;
  uml:id "EAID_BD05EC25_B9FA_4e2a_A953_D23FEA80E1C8" .

cim:UnitSymbol.VPerm a cim:UnitSymbol ;
  rdfs:label "VPerm" ;
  rdfs:comment "electric field strength, Volt per metre."@en ;
  rdfs:isDefinedBy :Package_CIMEnumerations ;
  uml:id "EAID_AB063AEA_81C2_410c_B41C_B345D7F1868B" .

cim:UnitSymbol.Vh a cim:UnitSymbol ;
  rdfs:label "Vh" ;
  rdfs:comment "Volt-hour, Volt hours."@en ;
  rdfs:isDefinedBy :Package_CIMEnumerations ;
  uml:id "EAID_731A8202_1BD4_44a0_B8E7_C82A6F1B47F4" .

cim:UnitSymbol.Vs a cim:UnitSymbol ;
  rdfs:label "Vs" ;
  rdfs:comment "Volt second (Ws/A)."@en ;
  rdfs:isDefinedBy :Package_CIMEnumerations ;
  uml:id "EAID_50759FC7_EB2D_47b3_833C_7F6B1458D251" .

cim:UnitSymbol.W a cim:UnitSymbol ;
  rdfs:label "W" ;
  rdfs:comment "Real power in Watt (J/s). Electrical power may have real and reactive components. The real portion of electrical power (IR or VIcos(phi)), is expressed in Watts. (See also apparent power and reactive power.)"@en ;
  rdfs:isDefinedBy :Package_CIMEnumerations ;
  uml:id "EAID_C160944D_C9F0_4871_9B2C_2320C1F7C1A2" .

cim:UnitSymbol.WPerA a cim:UnitSymbol ;
  rdfs:label "WPerA" ;
  rdfs:comment "Active power per current flow, watt per Ampere."@en ;
  rdfs:isDefinedBy :Package_CIMEnumerations ;
  uml:id "EAID_F55D6160_9960_4178_BB40_4BC85AFF91E5" .

cim:UnitSymbol.WPerW a cim:UnitSymbol ;
  rdfs:label "WPerW" ;
  rdfs:comment "Signal Strength, Ratio of power  Note: Users may need to supply a prefix such as m to show rates such as mW/W."@en ;
  rdfs:isDefinedBy :Package_CIMEnumerations ;
  uml:id "EAID_23406637_6D26_4426_BD20_1F8B2C5AA515" .

cim:UnitSymbol.WPerm2 a cim:UnitSymbol ;
  rdfs:label "WPerm2" ;
  rdfs:comment "Heat flux density, irradiance, Watt per square metre."@en ;
  rdfs:isDefinedBy :Package_CIMEnumerations ;
  uml:id "EAID_93EAE4BB_9CE4_41e8_9730_D957269533C9" .

cim:UnitSymbol.WPerm2sr a cim:UnitSymbol ;
  rdfs:label "WPerm2sr" ;
  rdfs:comment "radiance, Watt per square metre steradian."@en ;
  rdfs:isDefinedBy :Package_CIMEnumerations ;
  uml:id "EAID_047346B8_71C8_4fda_85A2_6FE1D43D6431" .

cim:UnitSymbol.WPermK a cim:UnitSymbol ;
  rdfs:label "WPermK" ;
  rdfs:comment "Thermal conductivity in Watt/metre Kelvin."@en ;
  rdfs:isDefinedBy :Package_CIMEnumerations ;
  uml:id "EAID_86E9DE8F_B4C7_48b4_8848_6A9B854FC76C" .

cim:UnitSymbol.WPers a cim:UnitSymbol ;
  rdfs:label "WPers" ;
  rdfs:comment "Ramp rate in Watt per second."@en ;
  rdfs:isDefinedBy :Package_CIMEnumerations ;
  uml:id "EAID_F0181C52_D05F_4e50_94AA_C5D348AAF734" .

cim:UnitSymbol.WPersr a cim:UnitSymbol ;
  rdfs:label "WPersr" ;
  rdfs:comment "Radiant intensity, Watt per steradian."@en ;
  rdfs:isDefinedBy :Package_CIMEnumerations ;
  uml:id "EAID_FDF9DAF2_2C0C_4ded_A78F_9CC8068BE2D5" .

cim:UnitSymbol.Wb a cim:UnitSymbol ;
  rdfs:label "Wb" ;
  rdfs:comment "Magnetic flux in Weber (Vs)."@en ;
  rdfs:isDefinedBy :Package_CIMEnumerations ;
  uml:id "EAID_BAD96D9D_91A8_480b_B918_798774EEECBB" .

cim:UnitSymbol.Wh a cim:UnitSymbol ;
  rdfs:label "Wh" ;
  rdfs:comment "Real energy in Watt hours."@en ;
  rdfs:isDefinedBy :Package_CIMEnumerations ;
  uml:id "EAID_A239C761_B67B_4ccb_832E_F299590120AB" .

cim:UnitSymbol.anglemin a cim:UnitSymbol ;
  rdfs:label "anglemin" ;
  rdfs:comment "Plane angle, minute."@en ;
  rdfs:isDefinedBy :Package_CIMEnumerations ;
  uml:id "EAID_AE607533_42D1_4b54_8BA2_B842D9B8A5CD" .

cim:UnitSymbol.anglesec a cim:UnitSymbol ;
  rdfs:label "anglesec" ;
  rdfs:comment "Plane angle, second."@en ;
  rdfs:isDefinedBy :Package_CIMEnumerations ;
  uml:id "EAID_A9E672D6_E895_4ae8_BD5C_9216FE5D1208" .

cim:UnitSymbol.bar a cim:UnitSymbol ;
  rdfs:label "bar" ;
  rdfs:comment "Pressure, bar (1 bar = 100 kPa)."@en ;
  rdfs:isDefinedBy :Package_CIMEnumerations ;
  uml:id "EAID_FAC447D1_CA76_4824_97C8_BC02A71FABF7" .

cim:UnitSymbol.cd a cim:UnitSymbol ;
  rdfs:label "cd" ;
  rdfs:comment "Luminous intensity in candela."@en ;
  rdfs:isDefinedBy :Package_CIMEnumerations ;
  uml:id "EAID_86492824_BA54_4e78_BEA8_DF08A1519540" .

cim:UnitSymbol.charPers a cim:UnitSymbol ;
  rdfs:label "charPers" ;
  rdfs:comment "Data rate (baud) in characters per second."@en ;
  rdfs:isDefinedBy :Package_CIMEnumerations ;
  uml:id "EAID_D03D75BB_9A84_4f44_8DC1_AB7254097464" .

cim:UnitSymbol.character a cim:UnitSymbol ;
  rdfs:label "character" ;
  rdfs:comment "Number of characters."@en ;
  rdfs:isDefinedBy :Package_CIMEnumerations ;
  uml:id "EAID_8B996FC0_89EB_4157_8F63_99A18429B8A7" .

cim:UnitSymbol.cosPhi a cim:UnitSymbol ;
  rdfs:label "cosPhi" ;
  rdfs:comment """Power factor, dimensionless.
Note 1: This definition of power factor only holds for balanced systems. See the alternative definition under code 153.
Note 2: Beware of differing sign conventions in use between the IEC and EEI. It is assumed that the data consumer understands the type of meter in use and the sign convention in use by the utility."""@en ;
  rdfs:isDefinedBy :Package_CIMEnumerations ;
  uml:id "EAID_9A475C35_1BB1_4d24_A1E0_61C8A0DE6542" .

cim:UnitSymbol.count a cim:UnitSymbol ;
  rdfs:label "count" ;
  rdfs:comment "Amount of substance, Counter value."@en ;
  rdfs:isDefinedBy :Package_CIMEnumerations ;
  uml:id "EAID_BFFB42D5_CAE3_49f7_9130_69385D62E5D0" .

cim:UnitSymbol.d a cim:UnitSymbol ;
  rdfs:label "d" ;
  rdfs:comment "Time, day = 24 h = 86400 s."@en ;
  rdfs:isDefinedBy :Package_CIMEnumerations ;
  uml:id "EAID_9DE425D1_8CB8_4b2e_BCDA_D9990ED74533" .

cim:UnitSymbol.dB a cim:UnitSymbol ;
  rdfs:label "dB" ;
  rdfs:comment "Sound pressure level in decibel. Note:  multiplier d is included in this unit symbol for compatibility with IEC 61850-7-3."@en ;
  rdfs:isDefinedBy :Package_CIMEnumerations ;
  uml:id "EAID_33CC17A0_5D8D_44e2_B72E_9668E65C3AE2" .

cim:UnitSymbol.dBm a cim:UnitSymbol ;
  rdfs:label "dBm" ;
  rdfs:comment "Power level (logrithmic ratio of signal strength , Bel-mW), normalized to 1mW. Note:  multiplier d is included in this unit symbol for compatibility with IEC 61850-7-3."@en ;
  rdfs:isDefinedBy :Package_CIMEnumerations ;
  uml:id "EAID_45FE77FA_3D1C_4f61_9328_44099CDB1396" .

cim:UnitSymbol.deg a cim:UnitSymbol ;
  rdfs:label "deg" ;
  rdfs:comment "Plane angle in degrees."@en ;
  rdfs:isDefinedBy :Package_CIMEnumerations ;
  uml:id "EAID_79DF68B3_CFBC_462f_BB36_9D491F5F3D83" .

cim:UnitSymbol.degC a cim:UnitSymbol ;
  rdfs:label "degC" ;
  rdfs:comment """Relative temperature in degrees Celsius.
In the SI unit system the symbol is C. Electric charge is measured in coulomb that has the unit symbol C. To distinguish degree Celsius form coulomb the symbol used in the UML is degC. Reason for not using C is the special character  is difficult to manage in software."""@en ;
  rdfs:isDefinedBy :Package_CIMEnumerations ;
  uml:id "EAID_2BA135D2_0950_48d2_976B_A142C4FB4BD5" .

cim:UnitSymbol.ft3 a cim:UnitSymbol ;
  rdfs:label "ft3" ;
  rdfs:comment "Volume, cubic foot."@en ;
  rdfs:isDefinedBy :Package_CIMEnumerations ;
  uml:id "EAID_EE3DE7DA_7747_4df4_AA96_CB826C159A37" .

cim:UnitSymbol.gPerg a cim:UnitSymbol ;
  rdfs:label "gPerg" ;
  rdfs:comment "Concentration, The ratio of the mass of a solute divided by the mass of  the solution. Note: Users may need use a prefix such a  to express a quantity such as g/g."@en ;
  rdfs:isDefinedBy :Package_CIMEnumerations ;
  uml:id "EAID_4FE2C6F4_252B_478b_81B6_B8A37C2040EA" .

cim:UnitSymbol.gal a cim:UnitSymbol ;
  rdfs:label "gal" ;
  rdfs:comment "Volume, US gallon (1 gal = 231 in3 = 128 fl ounce)."@en ;
  rdfs:isDefinedBy :Package_CIMEnumerations ;
  uml:id "EAID_075573F5_3B3E_413a_A3EE_6EEAD392ACF2" .

cim:UnitSymbol.h a cim:UnitSymbol ;
  rdfs:label "h" ;
  rdfs:comment "Time, hour = 60 min = 3600 s."@en ;
  rdfs:isDefinedBy :Package_CIMEnumerations ;
  uml:id "EAID_2FF7FF26_CE3D_43a3_99E4_7188416EC342" .

cim:UnitSymbol.ha a cim:UnitSymbol ;
  rdfs:label "ha" ;
  rdfs:comment "Area, hectare."@en ;
  rdfs:isDefinedBy :Package_CIMEnumerations ;
  uml:id "EAID_5DAD9F50_364E_4ff1_BC2C_B761442B63C0" .

cim:UnitSymbol.kat a cim:UnitSymbol ;
  rdfs:label "kat" ;
  rdfs:comment "Catalytic activity, katal = mol / s."@en ;
  rdfs:isDefinedBy :Package_CIMEnumerations ;
  uml:id "EAID_834E4B66_2AB3_4795_BDDA_F41BBA345492" .

cim:UnitSymbol.katPerm3 a cim:UnitSymbol ;
  rdfs:label "katPerm3" ;
  rdfs:comment "catalytic activity concentration, katal per cubic metre."@en ;
  rdfs:isDefinedBy :Package_CIMEnumerations ;
  uml:id "EAID_6221E81C_4094_4544_A256_101BFF4D1FC5" .

cim:UnitSymbol.kg a cim:UnitSymbol ;
  rdfs:label "kg" ;
  rdfs:comment "Mass in kilogram.  Note: multiplier k is included in this unit symbol for compatibility with IEC 61850-7-3."@en ;
  rdfs:isDefinedBy :Package_CIMEnumerations ;
  uml:id "EAID_DFBF6B76_BA8D_48f1_B895_3C1F69D191BC" .

cim:UnitSymbol.kgPerJ a cim:UnitSymbol ;
  rdfs:label "kgPerJ" ;
  rdfs:comment "Weigh per energy in kilogram/joule (kg/J). Note: multiplier k is included in this unit symbol for compatibility with IEC 61850-7-3."@en ;
  rdfs:isDefinedBy :Package_CIMEnumerations ;
  uml:id "EAID_CC8F1FA5_7B24_44c6_A882_50C0713C04A5" .

cim:UnitSymbol.kgPerm3 a cim:UnitSymbol ;
  rdfs:label "kgPerm3" ;
  rdfs:comment "Density in kilogram/cubic metre (kg/m). Note: multiplier k is included in this unit symbol for compatibility with IEC 61850-7-3."@en ;
  rdfs:isDefinedBy :Package_CIMEnumerations ;
  uml:id "EAID_501BEC8C_B847_44aa_BD7B_E606CCDBA737" .

cim:UnitSymbol.kgm a cim:UnitSymbol ;
  rdfs:label "kgm" ;
  rdfs:comment "Moment of mass in kilogram metre (kgm) (first moment of mass). Note: multiplier k is included in this unit symbol for compatibility with IEC 61850-7-3."@en ;
  rdfs:isDefinedBy :Package_CIMEnumerations ;
  uml:id "EAID_1DE9FA6B_0179_4e12_B5C4_6ABEB1FC4002" .

cim:UnitSymbol.kgm2 a cim:UnitSymbol ;
  rdfs:label "kgm2" ;
  rdfs:comment "Moment of mass in kilogram square metre (kgm) (Second moment of mass, commonly called the moment of inertia). Note: multiplier k is included in this unit symbol for compatibility with IEC 61850-7-3."@en ;
  rdfs:isDefinedBy :Package_CIMEnumerations ;
  uml:id "EAID_61A641E6_AACB_4084_8033_1F0424D09B3A" .

cim:UnitSymbol.kn a cim:UnitSymbol ;
  rdfs:label "kn" ;
  rdfs:comment "Speed, knot (1 kn = 1852/3600) m/s."@en ;
  rdfs:isDefinedBy :Package_CIMEnumerations ;
  uml:id "EAID_F100EA66_B1BA_4d19_B04F_94A815273DA8" .

cim:UnitSymbol.l a cim:UnitSymbol ;
  rdfs:label "l" ;
  rdfs:comment "Volume, litre = dm3 = m3/1000."@en ;
  rdfs:isDefinedBy :Package_CIMEnumerations ;
  uml:id "EAID_D946A4B2_75F4_456d_8A7B_60D75D8C8C54" .

cim:UnitSymbol.lPerh a cim:UnitSymbol ;
  rdfs:label "lPerh" ;
  rdfs:comment "Volumetric flow rate, litre per hour."@en ;
  rdfs:isDefinedBy :Package_CIMEnumerations ;
  uml:id "EAID_A2D6FCDF_C6C0_4b29_A162_3851CFD8CDFA" .

cim:UnitSymbol.lPerl a cim:UnitSymbol ;
  rdfs:label "lPerl" ;
  rdfs:comment "Concentration, The ratio of the volume of a solute divided by the volume of  the solution. Note: Users may need use a prefix such a  to express a quantity such as L/L."@en ;
  rdfs:isDefinedBy :Package_CIMEnumerations ;
  uml:id "EAID_1734D386_C2FA_4d27_B33B_F56A5B13F07D" .

cim:UnitSymbol.lPers a cim:UnitSymbol ;
  rdfs:label "lPers" ;
  rdfs:comment "Volumetric flow rate in litre per second."@en ;
  rdfs:isDefinedBy :Package_CIMEnumerations ;
  uml:id "EAID_EFE6BF1C_3882_4194_84CF_DB5A333DC816" .

cim:UnitSymbol.lm a cim:UnitSymbol ;
  rdfs:label "lm" ;
  rdfs:comment "Luminous flux in lumen (cdsr)."@en ;
  rdfs:isDefinedBy :Package_CIMEnumerations ;
  uml:id "EAID_CA24CD8D_1AAB_4e25_A5F3_9CE4FF76D150" .

cim:UnitSymbol.lx a cim:UnitSymbol ;
  rdfs:label "lx" ;
  rdfs:comment "Illuminance in lux (lm/m)."@en ;
  rdfs:isDefinedBy :Package_CIMEnumerations ;
  uml:id "EAID_66FD58AD_46BC_40cc_87F2_60012016945E" .

cim:UnitSymbol.m a cim:UnitSymbol ;
  rdfs:label "m" ;
  rdfs:comment "Length in meter."@en ;
  rdfs:isDefinedBy :Package_CIMEnumerations ;
  uml:id "EAID_E115BEB5_4F2D_4394_AF62_EB222FCD4431" .

cim:UnitSymbol.m2 a cim:UnitSymbol ;
  rdfs:label "m2" ;
  rdfs:comment "Area in square metre (m)."@en ;
  rdfs:isDefinedBy :Package_CIMEnumerations ;
  uml:id "EAID_244449A7_27DD_43b1_8A51_C79EFCA98953" .

cim:UnitSymbol.m2Pers a cim:UnitSymbol ;
  rdfs:label "m2Pers" ;
  rdfs:comment "Viscosity in metre square / second (m/s)."@en ;
  rdfs:isDefinedBy :Package_CIMEnumerations ;
  uml:id "EAID_DF3DC5F4_EA0C_4ceb_A28F_32BAD9DFFACD" .

cim:UnitSymbol.m3 a cim:UnitSymbol ;
  rdfs:label "m3" ;
  rdfs:comment "Volume in cubic metre (m)."@en ;
  rdfs:isDefinedBy :Package_CIMEnumerations ;
  uml:id "EAID_51129F02_2AD7_4cf4_A1B2_0429467866FA" .

cim:UnitSymbol.m3Compensated a cim:UnitSymbol ;
  rdfs:label "m3Compensated" ;
  rdfs:comment "Volume, cubic metre, with the value compensated for weather effects."@en ;
  rdfs:isDefinedBy :Package_CIMEnumerations ;
  uml:id "EAID_33690AF4_D81B_47f5_89FE_462996022C7E" .

cim:UnitSymbol.m3Perh a cim:UnitSymbol ;
  rdfs:label "m3Perh" ;
  rdfs:comment "Volumetric flow rate, cubic metre per hour."@en ;
  rdfs:isDefinedBy :Package_CIMEnumerations ;
  uml:id "EAID_96A81015_4806_4f34_8569_AA1432D6B2C8" .

cim:UnitSymbol.m3Perkg a cim:UnitSymbol ;
  rdfs:label "m3Perkg" ;
  rdfs:comment "Specific volume, cubic metre per kilogram, v."@en ;
  rdfs:isDefinedBy :Package_CIMEnumerations ;
  uml:id "EAID_A8364DE1_5E2D_490e_B99A_0D455165E39C" .

cim:UnitSymbol.m3Pers a cim:UnitSymbol ;
  rdfs:label "m3Pers" ;
  rdfs:comment "Volumetric flow rate in cubic metres per second (m/s)."@en ;
  rdfs:isDefinedBy :Package_CIMEnumerations ;
  uml:id "EAID_71D34D30_EE1F_491c_A3CA_1537AFCAE549" .

cim:UnitSymbol.m3Uncompensated a cim:UnitSymbol ;
  rdfs:label "m3Uncompensated" ;
  rdfs:comment "Volume, cubic metre, with the value uncompensated for weather effects."@en ;
  rdfs:isDefinedBy :Package_CIMEnumerations ;
  uml:id "EAID_6EF4A0F2_BA42_4486_B9A9_377C712B992E" .

cim:UnitSymbol.mPerm3 a cim:UnitSymbol ;
  rdfs:label "mPerm3" ;
  rdfs:comment "Fuel efficiency in metre per cubic metre (m/m)."@en ;
  rdfs:isDefinedBy :Package_CIMEnumerations ;
  uml:id "EAID_23C866AE_1454_4cac_B175_5BB2B115F859" .

cim:UnitSymbol.mPers a cim:UnitSymbol ;
  rdfs:label "mPers" ;
  rdfs:comment "Velocity in metre per second (m/s)."@en ;
  rdfs:isDefinedBy :Package_CIMEnumerations ;
  uml:id "EAID_14B945E9_F748_46eb_8316_7E7554218281" .

cim:UnitSymbol.mPers2 a cim:UnitSymbol ;
  rdfs:label "mPers2" ;
  rdfs:comment "Acceleration in metre per second squared (m/s)."@en ;
  rdfs:isDefinedBy :Package_CIMEnumerations ;
  uml:id "EAID_EA7DFD97_B06D_49dc_8726_EF0AF90505EE" .

cim:UnitSymbol.min a cim:UnitSymbol ;
  rdfs:label "min" ;
  rdfs:comment "Time, minute  = 60 s."@en ;
  rdfs:isDefinedBy :Package_CIMEnumerations ;
  uml:id "EAID_3711F440_EF3C_4c2d_8E90_CFC579ED94D1" .

cim:UnitSymbol.mmHg a cim:UnitSymbol ;
  rdfs:label "mmHg" ;
  rdfs:comment "Pressure, millimeter of mercury (1 mmHg is approximately 133.3 Pa)."@en ;
  rdfs:isDefinedBy :Package_CIMEnumerations ;
  uml:id "EAID_2AF0F2E6_FE07_4d0f_96C0_53B160516548" .

cim:UnitSymbol.mol a cim:UnitSymbol ;
  rdfs:label "mol" ;
  rdfs:comment "Amount of substance in mole."@en ;
  rdfs:isDefinedBy :Package_CIMEnumerations ;
  uml:id "EAID_60EE99CE_44B4_4eea_A380_C57B5A599751" .

cim:UnitSymbol.molPerkg a cim:UnitSymbol ;
  rdfs:label "molPerkg" ;
  rdfs:comment "Concentration, Molality, the amount of solute in moles and the amount of solvent in kilograms."@en ;
  rdfs:isDefinedBy :Package_CIMEnumerations ;
  uml:id "EAID_6393AB83_C6B3_4a9f_9014_4922A983270E" .

cim:UnitSymbol.molPerm3 a cim:UnitSymbol ;
  rdfs:label "molPerm3" ;
  rdfs:comment "Concentration, The amount of substance concentration, (c), the amount of solvent in moles divided by the volume of solution in m."@en ;
  rdfs:isDefinedBy :Package_CIMEnumerations ;
  uml:id "EAID_75B287C7_9AE3_4d28_8ECD_68CF7049BE6E" .

cim:UnitSymbol.molPermol a cim:UnitSymbol ;
  rdfs:label "molPermol" ;
  rdfs:comment "Concentration, Molar fraction (?), the ratio of the molar amount of a solute divided by the molar amount of the solution."@en ;
  rdfs:isDefinedBy :Package_CIMEnumerations ;
  uml:id "EAID_2E332E4E_01A2_44b3_805D_026A1C392DD7" .

cim:UnitSymbol.none a cim:UnitSymbol ;
  rdfs:label "none" ;
  rdfs:comment "Dimension less quantity, e.g. count, per unit, etc."@en ;
  rdfs:isDefinedBy :Package_CIMEnumerations ;
  uml:id "EAID_D2CE6FE3_01D7_4dd1_B8F7_FF90BE636625" .

cim:UnitSymbol.ohm a cim:UnitSymbol ;
  rdfs:label "ohm" ;
  rdfs:comment "Electric resistance in ohm (V/A)."@en ;
  rdfs:isDefinedBy :Package_CIMEnumerations ;
  uml:id "EAID_0D7094F7_0879_4d34_B08B_DEBC8C333F47" .

cim:UnitSymbol.ohmPerm a cim:UnitSymbol ;
  rdfs:label "ohmPerm" ;
  rdfs:comment "Electric resistance per length in ohm per metre ((V/A)/m)."@en ;
  rdfs:isDefinedBy :Package_CIMEnumerations ;
  uml:id "EAID_7FF254A7_BED8_4c65_995C_C60F5F99FF54" .

cim:UnitSymbol.ohmm a cim:UnitSymbol ;
  rdfs:label "ohmm" ;
  rdfs:comment "resistivity, Ohm metre, (rho)."@en ;
  rdfs:isDefinedBy :Package_CIMEnumerations ;
  uml:id "EAID_AC95BDC8_E2FA_47bc_A37A_04D7248D068B" .

cim:UnitSymbol.onePerHz a cim:UnitSymbol ;
  rdfs:label "onePerHz" ;
  rdfs:comment "Reciprocal of frequency (1/Hz)."@en ;
  rdfs:isDefinedBy :Package_CIMEnumerations ;
  uml:id "EAID_E416F8A6_355A_4667_A64E_E8BA5416F12A" .

cim:UnitSymbol.onePerm a cim:UnitSymbol ;
  rdfs:label "onePerm" ;
  rdfs:comment "Wavenumber, reciprocal metre,  (1/m)."@en ;
  rdfs:isDefinedBy :Package_CIMEnumerations ;
  uml:id "EAID_30EFB7ED_268D_4077_87DC_FAD3D4D1D20E" .

cim:UnitSymbol.ppm a cim:UnitSymbol ;
  rdfs:label "ppm" ;
  rdfs:comment "Concentration in parts per million."@en ;
  rdfs:isDefinedBy :Package_CIMEnumerations ;
  uml:id "EAID_BE0ED943_A3E0_477d_947B_05F076A2A5FD" .

cim:UnitSymbol.rad a cim:UnitSymbol ;
  rdfs:label "rad" ;
  rdfs:comment "Plane angle in radian (m/m)."@en ;
  rdfs:isDefinedBy :Package_CIMEnumerations ;
  uml:id "EAID_E6692373_B332_4cd8_AE2D_D17186894BB3" .

cim:UnitSymbol.radPers a cim:UnitSymbol ;
  rdfs:label "radPers" ;
  rdfs:comment "Angular velocity in radians per second (rad/s)."@en ;
  rdfs:isDefinedBy :Package_CIMEnumerations ;
  uml:id "EAID_A44B7E88_AD3F_4765_894A_8C4E32EAC533" .

cim:UnitSymbol.radPers2 a cim:UnitSymbol ;
  rdfs:label "radPers2" ;
  rdfs:comment "Angular acceleration, radian per second squared."@en ;
  rdfs:isDefinedBy :Package_CIMEnumerations ;
  uml:id "EAID_79216E4F_F72F_44ef_9AAE_4BBE9441712A" .

cim:UnitSymbol.rev a cim:UnitSymbol ;
  rdfs:label "rev" ;
  rdfs:comment "Amount of rotation, Revolutions."@en ;
  rdfs:isDefinedBy :Package_CIMEnumerations ;
  uml:id "EAID_6F1AA7AC_7267_46c1_9A0E_86B9095B2B6B" .

cim:UnitSymbol.rotPers a cim:UnitSymbol ;
  rdfs:label "rotPers" ;
  rdfs:comment "Rotations per second (1/s). See also Hz (1/s)."@en ;
  rdfs:isDefinedBy :Package_CIMEnumerations ;
  uml:id "EAID_ECAF4A79_071B_4634_B2B2_DF2CB571C6DB" .

cim:UnitSymbol.s a cim:UnitSymbol ;
  rdfs:label "s" ;
  rdfs:comment "Time in seconds."@en ;
  rdfs:isDefinedBy :Package_CIMEnumerations ;
  uml:id "EAID_6114A519_3046_45a6_8A51_0DCFB465BCE6" .

cim:UnitSymbol.sPers a cim:UnitSymbol ;
  rdfs:label "sPers" ;
  rdfs:comment "Time, Ratio of time Note: Users may need to supply a prefix such as  to show rates such as s/s"@en ;
  rdfs:isDefinedBy :Package_CIMEnumerations ;
  uml:id "EAID_EC6B9D0A_9C93_4a3f_BF4C_28E0D4F71EF5" .

cim:UnitSymbol.sr a cim:UnitSymbol ;
  rdfs:label "sr" ;
  rdfs:comment "Solid angle in steradian (m2/m2)."@en ;
  rdfs:isDefinedBy :Package_CIMEnumerations ;
  uml:id "EAID_08E268BA_FF87_444c_86E8_73A7EC4FF8D2" .

cim:UnitSymbol.therm a cim:UnitSymbol ;
  rdfs:label "therm" ;
  rdfs:comment "Energy, Therm."@en ;
  rdfs:isDefinedBy :Package_CIMEnumerations ;
  uml:id "EAID_4CA0BAFD_8B17_41ec_9753_0942B31959E8" .

cim:UnitSymbol.tonne a cim:UnitSymbol ;
  rdfs:label "tonne" ;
  rdfs:comment "mass, tonne or metric  ton (1000 kg = 1 Mg)."@en ;
  rdfs:isDefinedBy :Package_CIMEnumerations ;
  uml:id "EAID_A053EE28_60BE_4459_89CF_0EF5CB8FCE30" .

cim:Voltage a rdfs:Datatype ;
  rdfs:label "Voltage" ;
  rdfs:comment "Electrical voltage."@en ;
  owl:equivalentClass xsd:float ;
  rdfs:isDefinedBy :Package_CIMDataTypes ;
  uml:hasMultiplier "k" ;
  uml:hasStereotype uml:cimdatatype ;
  uml:hasUnits "V" ;
  uml:id "EAID_21C26D0F_BD78_444c_A025_61515F1D67B7" .

cim:VoltagePerReactivePower a rdfs:Datatype ;
  rdfs:label "VoltagePerReactivePower" ;
  rdfs:comment "Voltage variation with reactive power"@en ;
  owl:equivalentClass xsd:float ;
  rdfs:isDefinedBy :Package_CIMDataTypes ;
  uml:hasStereotype uml:cimdatatype ;
  uml:hasUnits "VPerVAr" ;
  uml:id "EAID_1DF64161_6CDF_4681_A40A_FAE80E1B8AD9" .

cim:WindGenUnitKind.offshore a cim:WindGenUnitKind ;
  rdfs:label "offshore" ;
  rdfs:comment "The wind generating unit is located offshore."@en ;
  rdfs:isDefinedBy :Package_CIMEnumerations ;
  uml:id "EAID_6AA2C69E_87FC_4e2e_B774_DBA24BA423A8" .

cim:WindGenUnitKind.onshore a cim:WindGenUnitKind ;
  rdfs:label "onshore" ;
  rdfs:comment "The wind generating unit is located onshore."@en ;
  rdfs:isDefinedBy :Package_CIMEnumerations ;
  uml:id "EAID_72FE0A3C_10D8_46e1_9512_E12C33892EE6" .

cim:WindingConnection.A a cim:WindingConnection ;
  rdfs:label "A" ;
  rdfs:comment "Autotransformer common winding"@en ;
  rdfs:isDefinedBy :Package_CIMEnumerations ;
  uml:id "EAID_D7E730D7_F1E1_4b1f_A052_C985EB91EFBC" .

cim:WindingConnection.D a cim:WindingConnection ;
  rdfs:label "D" ;
  rdfs:comment "Delta"@en ;
  rdfs:isDefinedBy :Package_CIMEnumerations ;
  uml:id "EAID_A4A9CBDC_3182_48b4_9709_2458B1B84066" .

cim:WindingConnection.I a cim:WindingConnection ;
  rdfs:label "I" ;
  rdfs:comment "Independent winding, for single-phase connections"@en ;
  rdfs:isDefinedBy :Package_CIMEnumerations ;
  uml:id "EAID_42EC06DE_A1F1_414b_85A6_55B3A11A14EC" .

cim:WindingConnection.Y a cim:WindingConnection ;
  rdfs:label "Y" ;
  rdfs:comment "Wye"@en ;
  rdfs:isDefinedBy :Package_CIMEnumerations ;
  uml:id "EAID_8DE87FC8_1289_49fa_9738_92F17BE0E78A" .

cim:WindingConnection.Yn a cim:WindingConnection ;
  rdfs:label "Yn" ;
  rdfs:comment "Wye, with neutral brought out for grounding."@en ;
  rdfs:isDefinedBy :Package_CIMEnumerations ;
  uml:id "EAID_662B6476_DA64_4379_93BE_06B3DAC31C2B" .

cim:WindingConnection.Z a cim:WindingConnection ;
  rdfs:label "Z" ;
  rdfs:comment "ZigZag"@en ;
  rdfs:isDefinedBy :Package_CIMEnumerations ;
  uml:id "EAID_4C2D41A1_4F47_4561_9CB1_0F8C4C2A35B6" .

cim:WindingConnection.Zn a cim:WindingConnection ;
  rdfs:label "Zn" ;
  rdfs:comment "ZigZag, with neutral brought out for grounding."@en ;
  rdfs:isDefinedBy :Package_CIMEnumerations ;
  uml:id "EAID_CBED0332_D6A9_465c_9F81_3BADD87D81BD" .

cim:WireInsulationKind.asbestosAndVarnishedCambric a cim:WireInsulationKind ;
  rdfs:label "asbestosAndVarnishedCambric" ;
  rdfs:isDefinedBy :Package_CIMEnumerations ;
  uml:id "EAID_E2D397FE_53C0_4362_96E5_163900C3C661" .

cim:WireInsulationKind.beltedPilc a cim:WireInsulationKind ;
  rdfs:label "beltedPilc" ;
  rdfs:isDefinedBy :Package_CIMEnumerations ;
  uml:id "EAID_D234E706_517B_4452_8C7A_209068C4AB5B" .

cim:WireInsulationKind.butyl a cim:WireInsulationKind ;
  rdfs:label "butyl" ;
  rdfs:isDefinedBy :Package_CIMEnumerations ;
  uml:id "EAID_E12301A9_8968_4235_AD10_01C5D076D9C6" .

cim:WireInsulationKind.crosslinkedPolyethylene a cim:WireInsulationKind ;
  rdfs:label "crosslinkedPolyethylene" ;
  rdfs:isDefinedBy :Package_CIMEnumerations ;
  uml:id "EAID_F8F5FADE_221E_47db_9CCF_BF45B3961468" .

cim:WireInsulationKind.ethylenePropyleneRubber a cim:WireInsulationKind ;
  rdfs:label "ethylenePropyleneRubber" ;
  rdfs:isDefinedBy :Package_CIMEnumerations ;
  uml:id "EAID_FAB16BFF_E26A_4ac2_A4EF_5D87ED0D6D8A" .

cim:WireInsulationKind.highMolecularWeightPolyethylene a cim:WireInsulationKind ;
  rdfs:label "highMolecularWeightPolyethylene" ;
  rdfs:isDefinedBy :Package_CIMEnumerations ;
  uml:id "EAID_2A5AC730_5EAA_4dbe_89F7_6926C40CE3AA" .

cim:WireInsulationKind.highPressureFluidFilled a cim:WireInsulationKind ;
  rdfs:label "highPressureFluidFilled" ;
  rdfs:isDefinedBy :Package_CIMEnumerations ;
  uml:id "EAID_31782C28_3342_4e7e_9C16_C767EA054D93" .

cim:WireInsulationKind.lowCapacitanceRubber a cim:WireInsulationKind ;
  rdfs:label "lowCapacitanceRubber" ;
  rdfs:isDefinedBy :Package_CIMEnumerations ;
  uml:id "EAID_961CFE6D_312A_4c78_8787_DD6FF530792B" .

cim:WireInsulationKind.oilPaper a cim:WireInsulationKind ;
  rdfs:label "oilPaper" ;
  rdfs:isDefinedBy :Package_CIMEnumerations ;
  uml:id "EAID_9AE08072_2A33_43af_BE3F_064F8C0B6D16" .

cim:WireInsulationKind.other a cim:WireInsulationKind ;
  rdfs:label "other" ;
  rdfs:isDefinedBy :Package_CIMEnumerations ;
  uml:id "EAID_D633B342_9CA4_4a3c_9018_925E2D8FF1C2" .

cim:WireInsulationKind.ozoneResistantRubber a cim:WireInsulationKind ;
  rdfs:label "ozoneResistantRubber" ;
  rdfs:isDefinedBy :Package_CIMEnumerations ;
  uml:id "EAID_2EB63137_31CC_4de7_836B_7CDF6703A9C7" .

cim:WireInsulationKind.rubber a cim:WireInsulationKind ;
  rdfs:label "rubber" ;
  rdfs:isDefinedBy :Package_CIMEnumerations ;
  uml:id "EAID_2EBA837D_F669_4613_BAEC_5E4EFE0C4E56" .

cim:WireInsulationKind.siliconRubber a cim:WireInsulationKind ;
  rdfs:label "siliconRubber" ;
  rdfs:isDefinedBy :Package_CIMEnumerations ;
  uml:id "EAID_0FEAA298_EF99_4777_998D_84196014FD5B" .

cim:WireInsulationKind.treeResistantHighMolecularWeightPolyethylene a cim:WireInsulationKind ;
  rdfs:label "treeResistantHighMolecularWeightPolyethylene" ;
  rdfs:isDefinedBy :Package_CIMEnumerations ;
  uml:id "EAID_45F5CFFD_B559_451e_8ED1_31ADA97E7135" .

cim:WireInsulationKind.treeRetardantCrosslinkedPolyethylene a cim:WireInsulationKind ;
  rdfs:label "treeRetardantCrosslinkedPolyethylene" ;
  rdfs:isDefinedBy :Package_CIMEnumerations ;
  uml:id "EAID_EDAD013B_EA92_4565_A0D3_5637926526EB" .

cim:WireInsulationKind.unbeltedPilc a cim:WireInsulationKind ;
  rdfs:label "unbeltedPilc" ;
  rdfs:isDefinedBy :Package_CIMEnumerations ;
  uml:id "EAID_B452862B_3CC6_4a8c_8D29_87A2CB7E52AB" .

cim:WireInsulationKind.varnishedCambricCloth a cim:WireInsulationKind ;
  rdfs:label "varnishedCambricCloth" ;
  rdfs:isDefinedBy :Package_CIMEnumerations ;
  uml:id "EAID_33D24022_A36E_4d80_97FA_6A87221C94A2" .

cim:WireInsulationKind.varnishedDacronGlass a cim:WireInsulationKind ;
  rdfs:label "varnishedDacronGlass" ;
  rdfs:isDefinedBy :Package_CIMEnumerations ;
  uml:id "EAID_47E2D409_4615_446d_B62A_1AE66872A80D" .

cim:WireMaterialKind.aaac a cim:WireMaterialKind ;
  rdfs:label "aaac" ;
  rdfs:comment "Aluminum-alloy conductor steel reinforced."@en ;
  rdfs:isDefinedBy :Package_CIMEnumerations ;
  uml:id "EAID_268ED1E9_EC67_4f18_A7DC_0955C9A0AD4D" .

cim:WireMaterialKind.acsr a cim:WireMaterialKind ;
  rdfs:label "acsr" ;
  rdfs:comment "Aluminum conductor steel reinforced."@en ;
  rdfs:isDefinedBy :Package_CIMEnumerations ;
  uml:id "EAID_0FC14A5C_8C14_4a1c_8F99_767018668A79" .

cim:WireMaterialKind.aluminum a cim:WireMaterialKind ;
  rdfs:label "aluminum" ;
  rdfs:isDefinedBy :Package_CIMEnumerations ;
  uml:id "EAID_4B18AEEA_0183_47c7_A880_8130E7DCEFD3" .

cim:WireMaterialKind.aluminumAlloy a cim:WireMaterialKind ;
  rdfs:label "aluminumAlloy" ;
  rdfs:isDefinedBy :Package_CIMEnumerations ;
  uml:id "EAID_0BBB476F_EF99_49fc_8D0B_253412E863A8" .

cim:WireMaterialKind.aluminumAlloySteel a cim:WireMaterialKind ;
  rdfs:label "aluminumAlloySteel" ;
  rdfs:isDefinedBy :Package_CIMEnumerations ;
  uml:id "EAID_E856F4E7_A25B_46c1_A00D_8C9E3E20C11D" .

cim:WireMaterialKind.aluminumSteel a cim:WireMaterialKind ;
  rdfs:label "aluminumSteel" ;
  rdfs:isDefinedBy :Package_CIMEnumerations ;
  uml:id "EAID_1026B016_6E05_4dc6_9C09_4DDB5109DBDA" .

cim:WireMaterialKind.copper a cim:WireMaterialKind ;
  rdfs:label "copper" ;
  rdfs:isDefinedBy :Package_CIMEnumerations ;
  uml:id "EAID_C437F22C_25F5_441e_91FA_1DF52B52982A" .

cim:WireMaterialKind.other a cim:WireMaterialKind ;
  rdfs:label "other" ;
  rdfs:isDefinedBy :Package_CIMEnumerations ;
  uml:id "EAID_D11DA662_4961_4a31_A0D7_4F15BB1653EC" .

cim:WireMaterialKind.steel a cim:WireMaterialKind ;
  rdfs:label "steel" ;
  rdfs:isDefinedBy :Package_CIMEnumerations ;
  uml:id "EAID_B41B166A_4EC4_4b8b_B3E5_020CB40F2C5B" .

cim:WireUsageKind.distribution a cim:WireUsageKind ;
  rdfs:label "distribution" ;
  rdfs:isDefinedBy :Package_CIMEnumerations ;
  uml:id "EAID_B3883D2E_FE70_404f_A707_BC1F61D33C69" .

cim:WireUsageKind.other a cim:WireUsageKind ;
  rdfs:label "other" ;
  rdfs:isDefinedBy :Package_CIMEnumerations ;
  uml:id "EAID_6C7040CB_2E2C_495d_8A01_449C074F2543" .

cim:WireUsageKind.secondary a cim:WireUsageKind ;
  rdfs:label "secondary" ;
  rdfs:isDefinedBy :Package_CIMEnumerations ;
  uml:id "EAID_7E55E71F_42CA_4aa4_9EC2_82A7F9648E86" .

cim:WireUsageKind.transmission a cim:WireUsageKind ;
  rdfs:label "transmission" ;
  rdfs:isDefinedBy :Package_CIMEnumerations ;
  uml:id "EAID_BF36BBDB_FC1D_4924_86A9_D9F754285E55" .

entsoe:LimitTypeKind.highVoltage a entsoe:LimitTypeKind ;
  rdfs:label "highVoltage" ;
  rdfs:comment """Referring to the rating of the equipments, a voltage too high can lead to accelerated ageing or the destruction of the equipment. 
This limit type may or may not have duration."""@en ;
  rdfs:isDefinedBy :Package_EntsoeExtensions ;
  uml:id "EAID_A2487C52_43C7_43ca_8C3D_8118D17045FE" .

entsoe:LimitTypeKind.lowVoltage a entsoe:LimitTypeKind ;
  rdfs:label "lowVoltage" ;
  rdfs:comment """A too low voltage can disturb the normal operation of some protections and transformer equipped with on-load tap changers, electronic power devices or can affect the behaviour of the auxiliaries of generation units.
This limit type may or may not have duration."""@en ;
  rdfs:isDefinedBy :Package_EntsoeExtensions ;
  uml:id "EAID_D8379B00_BAAB_4819_B91E_BACD2110B25C" .

entsoe:LimitTypeKind.patl a entsoe:LimitTypeKind ;
  rdfs:label "patl" ;
  rdfs:comment """The Permanent Admissible Transmission Loading (PATL) is the loading in Amps, MVA or MW that can be accepted by a network branch for an unlimited duration without any risk for the material.
The duration attribute is not used and shall be excluded for the PATL limit type. Hence only one limit value exists for the PATL type."""@en ;
  rdfs:isDefinedBy :Package_EntsoeExtensions ;
  uml:id "EAID_516D15CE_8CA9_4d25_8FDD_F27A89E58B09" .

entsoe:LimitTypeKind.patlt a entsoe:LimitTypeKind ;
  rdfs:label "patlt" ;
  rdfs:comment "Permanent Admissible Transmission Loading Threshold  (PATLT) is a value in engineering units defined for PATL and calculated using percentage less than 100 of the PATL type intended to alert operators of an arising condition. The percentage should be given in the name of the OperationalLimitSet. The aceptableDuration is another way to express the severity of the limit."@en ;
  rdfs:isDefinedBy :Package_EntsoeExtensions ;
  uml:id "EAID_643C64D1_3C4E_49a1_B399_98811CDA33C9" .

entsoe:LimitTypeKind.tatl a entsoe:LimitTypeKind ;
  rdfs:label "tatl" ;
  rdfs:comment """Temporarily Admissible Transmission Loading (TATL) which is the loading in Amps, MVA or MW that can be accepted by a branch for a certain limited duration.
The TATL can be defined in different ways:
<ul>
 <li>as a fixed percentage of the PATL for a given time (for example, 115% of the PATL that can be accepted during 15 minutes),</li>
</ul>
<ul>
 <li>pairs of TATL type and Duration calculated for each line taking into account its particular configuration and conditions of functioning (for example, it can define a TATL acceptable during 20 minutes and another one acceptable during 10 minutes).</li>
</ul>
Such a definition of TATL can depend on the initial operating conditions of the network element (sag situation of a line).
The duration attribute can be used define several TATL limit types. Hence multiple TATL limit values may exist having different durations."""@en ;
  rdfs:isDefinedBy :Package_EntsoeExtensions ;
  uml:id "EAID_372CFE1D_4098_420a_BA32_1A12D5074DD4" .

entsoe:LimitTypeKind.tc a entsoe:LimitTypeKind ;
  rdfs:label "tc" ;
  rdfs:comment """Tripping Current (TC) is the ultimate intensity without any delay. It is defined as the threshold the line will trip without any possible remedial actions.
The tripping of the network element is ordered by protections against short circuits or by overload protections, but in any case, the activation delay of these protections is not compatible with the reaction delay of an operator (less than one minute).
The duration is always zero and the duration attribute may be left out. Hence only one limit value exists for the TC type."""@en ;
  rdfs:isDefinedBy :Package_EntsoeExtensions ;
  uml:id "EAID_5453131E_0F2E_43ab_8AE6_76BAEAE28C73" .

entsoe:LimitTypeKind.tct a entsoe:LimitTypeKind ;
  rdfs:label "tct" ;
  rdfs:comment "Tripping Current Threshold  (TCT) is a value in engineering units defined for TC and calculated using percentage less than 100 of the TC type intended to alert operators of an arising condition. The percentage should be given in the name of the OperationalLimitSet. The aceptableDuration is another way to express the severity of the limit."@en ;
  rdfs:isDefinedBy :Package_EntsoeExtensions ;
  uml:id "EAID_BBCB79E0_9C34_4767_BB0E_DEE92D439726" .

md:URI a rdfs:Datatype ;
  rdfs:label "URI" ;
  rdfs:comment "URI is a string following the rules defined by the W3C/IETF URI Planning Interest Group in a set of RFCs of which one is RFC 3305."@en ;
  rdfs:isDefinedBy :Package_ModelDescription ;
  uml:hasStereotype uml:primitive ;
  uml:id "EAID_FD27B00A_FB5C_4944_9ECA_58BD201E9B7F" .

uml:aggregateOf a uml:Stereotype ;
  rdfs:label "Aggregate Of" .

uml:attribute a uml:Stereotype ;
  rdfs:label "Attribute" .

uml:base a uml:Stereotype ;
  rdfs:label "Base" .

uml:byreference a uml:Stereotype ;
  rdfs:label "By Reference" .

uml:cdpsm a uml:Stereotype ;
  rdfs:label "cdpsm" ;
  uml:id "EAID_D4915636_C3CA_4527_9986_F137EC44B354" .

uml:cimdatatype a uml:Stereotype ;
  rdfs:label "CIMDatatype" ;
  uml:id "EAID_A2D28F4B_4F45_4ba7_8701_D09EC6B89714" .

uml:compositeOf a uml:Stereotype ;
  rdfs:label "Composite Of" .

uml:compound a uml:Stereotype ;
  rdfs:label "Compound", "Compound Datatype" ;
  uml:id "EAID_D3825557_DF84_4b0c_A74A_B6BE103760C1" .

uml:concrete a uml:Stereotype ;
  rdfs:label "Concrete" .

uml:contextualmodel a uml:Stereotype ;
  rdfs:label "ContextualModel" ;
  uml:id "EAID_662AB0FE_6E69_4895_BC28_E41DBF4E9E5D", "EAID_97912E7C_E64C_4e21_82F3_7DC2A50E13E4" .

uml:datatype a uml:Stereotype ;
  rdfs:label "Datatype" .

uml:deprecated a uml:Stereotype ;
  rdfs:label "deprecated" ;
  uml:id "EAID_04E85A9B_E8D0_4f2c_AD38_6B560201A24B" .

uml:description a uml:Stereotype ;
  rdfs:label "Description" ;
  uml:id "EAID_87832818_A93B_476a_AD31_510F1A714138" .

uml:entsoe a uml:Stereotype ;
  rdfs:label "Entsoe", "entsoe" ;
  uml:id "EAID_5E43CDB3_68DA_43a7_BC0A_E49A40791E83", "EAID_7277A622_CDA5_4acf_8D8A_7FD6BAF778CB", "EAID_B7AA0B9A_56E5_48fd_8546_D2D8B064DE88", "EAID_BE2C9710_33C0_4dd8_8103_799A0956E212" .

uml:enum a uml:Stereotype ;
  rdfs:label "enum" ;
  uml:id "EAID_2DB4C97D_A73C_4e3d_945B_DC11C242BB0B", "EAID_60D92F7D_34A8_40c8_AB17_ED9AB8998747" .

uml:enumeration a uml:Stereotype ;
  rdfs:label "Enumeration", "enumeration" ;
  uml:id "XTRA_stereotype_enumeration" .

uml:extendedby a uml:Stereotype ;
  rdfs:label "Extended By" .

uml:extension a uml:Stereotype ;
  rdfs:label "Extension Class", "extension" ;
  uml:id "EAID_08AD788C_24B5_4945_B219_3618A7834048", "EAID_E41FCD65_2FBD_4c6a_9A11_B55DDF063061" .

uml:ofAggregate a uml:Stereotype ;
  rdfs:label "Of Aggregate" .

uml:ofComposite a uml:Stereotype ;
  rdfs:label "Of Composite" .

uml:preserve a uml:Stereotype ;
  rdfs:label "Preserve" .

uml:primitive a uml:Stereotype ;
  rdfs:label "Primitive" ;
  uml:id "EAID_2CBBE568_189E_4185_ABB5_8CA72ACAB81A", "EAID_C80829EC_090C_414c_8DFC_95797736C710" .

uml:union a uml:Stereotype ;
  rdfs:label "Union" .

uml:xmlattribute a uml:Stereotype ;
  rdfs:label "XML Attribute" .

uml:xmlelement a uml:Stereotype ;
  rdfs:label "XML Element" .

xsd:date rdfs:label "Date" ;
  uml:id "eaxmiid3" .

xsd:dateTime rdfs:label "DateTime" ;
  uml:id "eaxmiid1" .

xsd:integer rdfs:label "Integer" ;
  uml:id "eaxmiid4" .

xsd:string rdfs:label "String" ;
  uml:id "eaxmiid0" .


